# baseURI: http://toop.tno.nl/organization
# imports: https://www.w3.org/2009/08/skos-reference/skos.rdf
# prefix: toop

@prefix adms: <http://www.w3.org/ns/adms#> .
@prefix arg: <http://spinrdf.org/arg#> .
@prefix dc: <http://purl.org/dc/elements/1.1/> .
@prefix dcam: <http://purl.org/dc/dcam/> .
@prefix dcat: <http://www.w3.org/ns/dcat#> .
@prefix dct: <http://purl.org/dc/terms/> .
@prefix dcterms: <http://purl.org/dc/terms/> .
@prefix foaf: <http://xmlns.com/foaf/0.1/> .
@prefix gr: <http://purl.org/goodrelations/v1#> .
@prefix nhr: <http://example.register.nl/nationaalhandelsregister#> .
@prefix org: <http://www.w3.org/ns/org#> .
@prefix owl: <http://www.w3.org/2002/07/owl#> .
@prefix owlTime: <http://www.w3.org/2006/time#> .
@prefix prov: <http://www.w3.org/ns/prov#> .
@prefix rdf: <http://www.w3.org/1999/02/22-rdf-syntax-ns#> .
@prefix rdfs: <http://www.w3.org/2000/01/rdf-schema#> .
@prefix rov: <http://www.w3.org/ns/regorg#> .
@prefix schema: <http://schema.org/> .
@prefix skos: <http://www.w3.org/2004/02/skos/core#> .
@prefix sp: <http://spinrdf.org/sp#> .
@prefix spin: <http://spinrdf.org/spin#> .
@prefix spl: <http://spinrdf.org/spl#> .
@prefix toop: <http://toop.tno.nl/organization#> .
@prefix vann: <http://purl.org/vocab/vann/> .
@prefix vcard: <http://www.w3.org/2006/vcard/ns#> .
@prefix voaf: <http://purl.org/vocommons/voaf#> .
@prefix wdrs: <http://www.w3.org/2007/05/powder-s#> .
@prefix wgs: <http://www.w3.org/2003/01/geo/wgs84_pos#> .
@prefix xsd: <http://www.w3.org/2001/XMLSchema#> .

<http://example.register.nl/nationaalhandelsregister>
  owl:versionInfo "Created with TopBraid Composer" ;
.
nhr:KvK-nummer
  rdf:type rdfs:Class ;
  rdfs:comment "The unique official company identifier_"@nl ;
  rdfs:label "Kvk-nummer _"@nl ;
  rdfs:subClassOf adms:Identifier ;
  skos:prefLabel "Kvk-nummer" ;
.
nhr:MaatschappelijkeActiviteit
  rdf:type owl:Class ;
  rdfs:comment "Een MaatschappelijkeActiviteit is een organisatie zonder winstoogmerk maar met een missie die gericht is op het verbeteren of instandhouden van aktiviteiten of bezit met maatschappelijk karakter. "@nl ;
  rdfs:label "Maatschappelijke activiteit_"@nl ;
  rdfs:subClassOf skos:Concept ;
  rdfs:subClassOf [
      rdf:type owl:Restriction ;
      owl:onDataRange nhr:KvK-nummer ;
      owl:onProperty nhr:kvk-nummer ;
      owl:qualifiedCardinality "1"^^xsd:nonNegativeInteger ;
    ] ;
.
nhr:Onderneming
  rdf:type owl:Class ;
  rdfs:comment "Een Onderderming is een organisatie met winstoogmerk. "@nl ;
  rdfs:label "Onderneming_"@nl ;
  rdfs:subClassOf skos:Concept ;
.
nhr:Rechtsvorm
  rdf:type owl:Class ;
  rdfs:comment "De vorm die u kiest voor de uitoefening van uw onderneming, heet rechtsvorm. De rechtsvorm is niet alleen van belang voor aansprakelijkheid, maar is ook van invloed op uw belastingverplichtingen. Zo is een rechtspersoon de eigenaar van de onderneming en daarmee belastingplichtig voor de winst uit onderneming."@nl ;
  rdfs:label "Rechtsvorm_"@nl ;
  rdfs:subClassOf skos:Concept ;
  skos:prefLabel "Rechtsvorm" ;
.
nhr:Status
  rdf:type owl:Class ;
  rdfs:comment "De status van de organisatie. "@nl ;
  rdfs:label "Status_"@nl ;
  rdfs:subClassOf skos:Concept ;
  skos:prefLabel "Status" ;
.
nhr:actief
  rdf:type nhr:Status ;
  rdfs:comment "De organisatie bestaat en is actief. "@nl ;
  rdfs:label "actief_"@nl ;
  skos:prefLabel "actief" ;
.
nhr:besloten_vennootschap
  rdf:type nhr:Rechtsvorm ;
  rdfs:comment "Een bv kunt u alleen of samen met anderen oprichten. Voor de oprichting schakelt u een notaris in. In de notariële akte wordt onder meer vastgelegd hoeveel aandelen elk van de oprichters in de bv krijgt."@nl ;
  rdfs:label "bv_"@nl ;
  skos:prefLabel "bv" ;
.
nhr:beëindigd
  rdf:type nhr:Status ;
  rdfs:comment "De organisatievorm is opgehouden te bestaan. "@nl ;
  rdfs:label "beëindigd_"@nl ;
  skos:prefLabel "beëindigd" ;
.
nhr:commanditaire_vennootschap
  rdf:type nhr:Rechtsvorm ;
  rdfs:comment "Voor een cv gelden grotendeels dezelfde regels als voor een vof. Het verschil is dat een cv behalve de gewone vennoten (de 'beherende' vennoten) ook nog zogenoemde stille vennoten heeft. De stille vennoten brengen geld in de cv in, maar bemoeien zich niet met de verdere gang van zaken van de onderneming. Elke beherende vennoot die aan de eisen voldoet, geldt voor de inkomstenbelasting als ondernemer. Als hij voldoet aan het urencriterium, kan hij dus gebruikmaken van de speciale regelingen voor ondernemers."@nl ;
  rdfs:label "cv_"@nl ;
  skos:prefLabel "cv" ;
.
nhr:eenmanszaak
  rdf:type nhr:Rechtsvorm ;
  rdfs:comment "Bij een eenmanszaak drijft u de onderneming alleen. Dat is het geval als u een zelfstandig beroep uitoefent (bijvoorbeeld notaris of huisarts) of als u de enige eigenaar van uw bedrijf bent. U kunt dus ook een eenmanszaak hebben als u personeel in dienst hebt. "@nl ;
  rdfs:label "eenmanszaak_"@nl ;
  skos:prefLabel "eenmanszaak" ;
.
nhr:handelsnaam
  rdf:type rdf:Property ;
  rdfs:comment "if the company is a business for which holds Handelsnaam.volgnr = 1"@nl ;
  rdfs:domain nhr:MaatschappelijkeActiviteit ;
  rdfs:domain nhr:Onderneming ;
  rdfs:label "handelsnaam_"@nl ;
  rdfs:range xsd:string ;
  rdfs:subPropertyOf rdf:predicate ;
  skos:prefLabel "handelsnaam" ;
.
nhr:heeftStatus
  rdf:type owl:ObjectProperty ;
  rdfs:comment "De huidige formele status van de organisatie. "@nl ;
  rdfs:domain nhr:MaatschappelijkeActiviteit ;
  rdfs:domain nhr:Onderneming ;
  rdfs:label "heeft status_"@nl ;
  rdfs:range nhr:Status ;
  rdfs:subPropertyOf rdf:predicate ;
  skos:prefLabel "heeft status" ;
.
nhr:kvk-nummer
  rdf:type owl:DatatypeProperty ;
  rdfs:comment "Alle bedrijven krijgen bij inschrijving bij de Kamer van Koophandel een KvK-nummer. Bij een bedrijfsoverdracht krijgen ondernemingen een nieuw KvK-nummer, zodat het duidelijk is dat er sprake is van een nieuwe eigenaar. U moet het nieuwe KvK-nummer vermelden op uw bedrijfscorrespondentie, zoals brieven, orders, facturen en offertes. "@nl ;
  rdfs:domain nhr:MaatschappelijkeActiviteit ;
  rdfs:domain nhr:Onderneming ;
  rdfs:label "kvk-nummer_"@nl ;
  rdfs:range nhr:KvK-nummer ;
  rdfs:subPropertyOf skos:notation ;
  skos:prefLabel "kvk-nummer"@nl ;
.
nhr:maatschap
  rdf:type nhr:Rechtsvorm ;
  rdfs:comment "In het geval van een maatschap oefent u een beroep uit in samenwerking met anderen (uw 'maten'), bijvoorbeeld in een artsenpraktijk of een tolkencentrum. U kunt zelf een samenwerkingscontract opstellen of u kunt een deskundige inschakelen."@nl ;
  rdfs:label "maatschap_"@nl ;
  skos:prefLabel "maatschap" ;
.
nhr:naam
  rdf:type rdf:Property ;
  rdfs:comment "if the company is a \"non-natural person\" or a \"societal activity\" for which holds NaamVolgorde.volgorde = 1"@nl ;
  rdfs:domain nhr:MaatschappelijkeActiviteit ;
  rdfs:domain nhr:Onderneming ;
  rdfs:label "naam_"@nl ;
  rdfs:range xsd:string ;
  rdfs:subPropertyOf rdf:predicate ;
  skos:prefLabel "naam" ;
.
nhr:stichting_of_vereniging
  rdf:type nhr:Rechtsvorm ;
  rdfs:comment "Stichtingen en verenigingen worden in bepaalde gevallen ook als onderneming beschouwd. Uw stichting of vereniging betaalt dan over de winst vennootschapsbelasting. "@nl ;
  rdfs:label "stichting of vereniging_"@nl ;
  skos:prefLabel "stichting of vereniging" ;
.
nhr:vennootschap_onder_firma_VOF
  rdf:type nhr:Rechtsvorm ;
  rdfs:comment "Van een vennootschap onder firma (vof) is sprake als u samen met anderen (de firmanten of vennoten) een onderneming begint. U kunt zelf een samenwerkingscontract opstellen of u kunt een deskundige inschakelen. Elke vennoot die aan de eisen voor ondernemerschap voldoet, geldt voor de inkomstenbelasting als ondernemer. En kan hij gebruikmaken van de ondernemersregelingen. "@nl ;
  rdfs:label "vof_"@nl ;
  skos:prefLabel "vof" ;
.
dc:contributor
  rdf:type owl:AnnotationProperty ;
.
dc:creator
  rdf:type owl:AnnotationProperty ;
.
dc:date
  rdf:type owl:AnnotationProperty ;
.
dc:description
  rdf:type owl:AnnotationProperty ;
.
dc:title
  rdf:type owl:AnnotationProperty ;
.
dcterms:
  dcterms:modified "2012-06-14"^^xsd:date ;
  dcterms:publisher <http://purl.org/dc/aboutdcmi#DCMI> ;
  dcterms:title "DCMI Metadata Terms - other"@en ;
.
dcterms:Agent
  rdf:type dcterms:AgentClass ;
  rdf:type rdfs:Class ;
  dcterms:description "Examples of Agent include person, organization, and software agent."@en ;
  dcterms:hasVersion <http://dublincore.org/usage/terms/history/#Agent-001> ;
  dcterms:issued "2008-01-14"^^xsd:date ;
  rdfs:comment "A resource that acts or has the power to act."@en ;
  rdfs:isDefinedBy dcterms: ;
  rdfs:label "Agent"@en ;
  rdfs:subClassOf rdfs:Resource ;
.
dcterms:AgentClass
  rdf:type rdfs:Class ;
  dcterms:description "Examples of Agent Class include groups seen as classes, such as students, women, charities, lecturers."@en ;
  dcterms:hasVersion <http://dublincore.org/usage/terms/history/#AgentClass-003> ;
  dcterms:issued "2008-01-14"^^xsd:date ;
  dcterms:modified "2012-06-14"^^xsd:date ;
  rdfs:comment "A group of agents."@en ;
  rdfs:isDefinedBy dcterms: ;
  rdfs:label "Agent Class"@en ;
  rdfs:subClassOf rdfs:Class ;
.
dcterms:BibliographicResource
  rdf:type rdfs:Class ;
  dcterms:hasVersion <http://dublincore.org/usage/terms/history/#BibliographicResource-001> ;
  dcterms:issued "2008-01-14"^^xsd:date ;
  rdfs:comment "A book, article, or other documentary resource."@en ;
  rdfs:isDefinedBy dcterms: ;
  rdfs:label "Bibliographic Resource"@en ;
  rdfs:subClassOf rdfs:Resource ;
.
dcterms:Box
  rdf:type rdfs:Datatype ;
  dcterms:hasVersion <http://dublincore.org/usage/terms/history/#Box-003> ;
  dcterms:issued "2000-07-11"^^xsd:date ;
  dcterms:modified "2008-01-14"^^xsd:date ;
  rdfs:comment "The set of regions in space defined by their geographic coordinates according to the DCMI Box Encoding Scheme."@en ;
  rdfs:isDefinedBy dcterms: ;
  rdfs:label "DCMI Box"@en ;
  rdfs:seeAlso <http://dublincore.org/documents/dcmi-box/> ;
  rdfs:subClassOf rdfs:Resource ;
.
dcterms:DCMIType
  rdf:type dcam:VocabularyEncodingScheme ;
  dcterms:hasVersion <http://dublincore.org/usage/terms/history/#DCMIType-005> ;
  dcterms:issued "2000-07-11"^^xsd:date ;
  dcterms:modified "2012-06-14"^^xsd:date ;
  rdfs:comment "The set of classes specified by the DCMI Type Vocabulary, used to categorize the nature or genre of the resource."@en ;
  rdfs:isDefinedBy dcterms: ;
  rdfs:label "DCMI Type Vocabulary"@en ;
  rdfs:seeAlso <http://purl.org/dc/dcmitype/> ;
.
dcterms:DDC
  rdf:type dcam:VocabularyEncodingScheme ;
  dcterms:hasVersion <http://dublincore.org/usage/terms/history/#DDC-003> ;
  dcterms:issued "2000-07-11"^^xsd:date ;
  dcterms:modified "2008-01-14"^^xsd:date ;
  rdfs:comment "The set of conceptual resources specified by the Dewey Decimal Classification."@en ;
  rdfs:isDefinedBy dcterms: ;
  rdfs:label "DDC"@en ;
  rdfs:seeAlso <http://www.oclc.org/dewey/> ;
.
dcterms:FileFormat
  rdf:type rdfs:Class ;
  dcterms:description "Examples include the formats defined by the list of Internet Media Types."@en ;
  dcterms:hasVersion <http://dublincore.org/usage/terms/history/#FileFormat-001> ;
  dcterms:issued "2008-01-14"^^xsd:date ;
  rdfs:comment "A digital resource format."@en ;
  rdfs:isDefinedBy dcterms: ;
  rdfs:label "File Format"@en ;
  rdfs:subClassOf dcterms:MediaType ;
.
dcterms:Frequency
  rdf:type rdfs:Class ;
  dcterms:hasVersion <http://dublincore.org/usage/terms/history/#Frequency-001> ;
  dcterms:issued "2008-01-14"^^xsd:date ;
  rdfs:comment "A rate at which something recurs."@en ;
  rdfs:isDefinedBy dcterms: ;
  rdfs:label "Frequency"@en ;
  rdfs:subClassOf rdfs:Resource ;
.
dcterms:IMT
  rdf:type dcam:VocabularyEncodingScheme ;
  dcterms:hasVersion <http://dublincore.org/usage/terms/history/#IMT-004> ;
  dcterms:issued "2000-07-11"^^xsd:date ;
  dcterms:modified "2008-01-14"^^xsd:date ;
  rdfs:comment "The set of media types specified by the Internet Assigned Numbers Authority."@en ;
  rdfs:isDefinedBy dcterms: ;
  rdfs:label "IMT"@en ;
  rdfs:seeAlso <http://www.iana.org/assignments/media-types/> ;
.
dcterms:ISO3166
  rdf:type rdfs:Datatype ;
  dcterms:hasVersion <http://dublincore.org/usage/terms/history/#ISO3166-004> ;
  dcterms:issued "2000-07-11"^^xsd:date ;
  dcterms:modified "2008-01-14"^^xsd:date ;
  rdfs:comment "The set of codes listed in ISO 3166-1 for the representation of names of countries."@en ;
  rdfs:isDefinedBy dcterms: ;
  rdfs:label "ISO 3166"@en ;
  rdfs:seeAlso <http://www.iso.org/iso/en/prods-services/iso3166ma/02iso-3166-code-lists/list-en1.html> ;
  rdfs:subClassOf rdfs:Resource ;
.
dcterms:ISO639-2
  rdf:type rdfs:Datatype ;
  dcterms:hasVersion <http://dublincore.org/usage/terms/history/#ISO639-2-003> ;
  dcterms:issued "2000-07-11"^^xsd:date ;
  dcterms:modified "2008-01-14"^^xsd:date ;
  rdfs:comment "The three-letter alphabetic codes listed in ISO639-2 for the representation of names of languages."@en ;
  rdfs:isDefinedBy dcterms: ;
  rdfs:label "ISO 639-2"@en ;
  rdfs:seeAlso <http://lcweb.loc.gov/standards/iso639-2/langhome.html> ;
  rdfs:subClassOf rdfs:Resource ;
.
dcterms:ISO639-3
  rdf:type rdfs:Datatype ;
  dcterms:hasVersion <http://dublincore.org/usage/terms/history/#ISO639-3-001> ;
  dcterms:issued "2008-01-14"^^xsd:date ;
  rdfs:comment "The set of three-letter codes listed in ISO 639-3 for the representation of names of languages."@en ;
  rdfs:isDefinedBy dcterms: ;
  rdfs:label "ISO 639-3"@en ;
  rdfs:seeAlso <http://www.sil.org/iso639-3/> ;
  rdfs:subClassOf rdfs:Resource ;
.
dcterms:Jurisdiction
  rdf:type rdfs:Class ;
  dcterms:hasVersion <http://dublincore.org/usage/terms/history/#Jurisdiction-001> ;
  dcterms:issued "2008-01-14"^^xsd:date ;
  rdfs:comment "The extent or range of judicial, law enforcement, or other authority."@en ;
  rdfs:isDefinedBy dcterms: ;
  rdfs:label "Jurisdiction"@en ;
  rdfs:subClassOf dcterms:LocationPeriodOrJurisdiction ;
.
dcterms:LCC
  rdf:type dcam:VocabularyEncodingScheme ;
  dcterms:hasVersion <http://dublincore.org/usage/terms/history/#LCC-003> ;
  dcterms:issued "2000-07-11"^^xsd:date ;
  dcterms:modified "2008-01-14"^^xsd:date ;
  rdfs:comment "The set of conceptual resources specified by the Library of Congress Classification."@en ;
  rdfs:isDefinedBy dcterms: ;
  rdfs:label "LCC"@en ;
  rdfs:seeAlso <http://lcweb.loc.gov/catdir/cpso/lcco/lcco.html> ;
.
dcterms:LCSH
  rdf:type dcam:VocabularyEncodingScheme ;
  dcterms:hasVersion <http://dublincore.org/usage/terms/history/#LCSH-003> ;
  dcterms:issued "2000-07-11"^^xsd:date ;
  dcterms:modified "2008-01-14"^^xsd:date ;
  rdfs:comment "The set of labeled concepts specified by the Library of Congress Subject Headings."@en ;
  rdfs:isDefinedBy dcterms: ;
  rdfs:label "LCSH"@en ;
.
dcterms:LicenseDocument
  rdf:type rdfs:Class ;
  dcterms:hasVersion <http://dublincore.org/usage/terms/history/#LicenseDocument-001> ;
  dcterms:issued "2008-01-14"^^xsd:date ;
  rdfs:comment "A legal document giving official permission to do something with a Resource."@en ;
  rdfs:isDefinedBy dcterms: ;
  rdfs:label "License Document"@en ;
  rdfs:subClassOf dcterms:RightsStatement ;
.
dcterms:LinguisticSystem
  rdf:type rdfs:Class ;
  dcterms:description "Examples include written, spoken, sign, and computer languages."@en ;
  dcterms:hasVersion <http://dublincore.org/usage/terms/history/#LinguisticSystem-001> ;
  dcterms:issued "2008-01-14"^^xsd:date ;
  rdfs:comment "A system of signs, symbols, sounds, gestures, or rules used in communication."@en ;
  rdfs:isDefinedBy dcterms: ;
  rdfs:label "Linguistic System"@en ;
  rdfs:subClassOf rdfs:Resource ;
.
dcterms:Location
  rdf:type rdfs:Class ;
  dcterms:hasVersion <http://dublincore.org/usage/terms/history/#Location-001> ;
  dcterms:issued "2008-01-14"^^xsd:date ;
  rdfs:comment "A spatial region or named place."@en ;
  rdfs:isDefinedBy dcterms: ;
  rdfs:label "Location"@en ;
  rdfs:subClassOf dcterms:LocationPeriodOrJurisdiction ;
.
dcterms:LocationPeriodOrJurisdiction
  rdf:type rdfs:Class ;
  dcterms:hasVersion <http://dublincore.org/usage/terms/history/#LocationPeriodOrJurisdiction-001> ;
  dcterms:issued "2008-01-14"^^xsd:date ;
  rdfs:comment "A location, period of time, or jurisdiction."@en ;
  rdfs:isDefinedBy dcterms: ;
  rdfs:label "Location, Period, or Jurisdiction"@en ;
  rdfs:subClassOf rdfs:Resource ;
.
dcterms:MESH
  rdf:type dcam:VocabularyEncodingScheme ;
  dcterms:hasVersion <http://dublincore.org/usage/terms/history/#MESH-003> ;
  dcterms:issued "2000-07-11"^^xsd:date ;
  dcterms:modified "2008-01-14"^^xsd:date ;
  rdfs:comment "The set of labeled concepts specified by the Medical Subject Headings."@en ;
  rdfs:isDefinedBy dcterms: ;
  rdfs:label "MeSH"@en ;
  rdfs:seeAlso <http://www.nlm.nih.gov/mesh/meshhome.html> ;
.
dcterms:MediaType
  rdf:type rdfs:Class ;
  dcterms:hasVersion <http://dublincore.org/usage/terms/history/#MediaType-001> ;
  dcterms:issued "2008-01-14"^^xsd:date ;
  rdfs:comment "A file format or physical medium."@en ;
  rdfs:isDefinedBy dcterms: ;
  rdfs:label "Media Type"@en ;
  rdfs:subClassOf dcterms:MediaTypeOrExtent ;
.
dcterms:MediaTypeOrExtent
  rdf:type rdfs:Class ;
  dcterms:hasVersion <http://dublincore.org/usage/terms/history/#MediaTypeOrExtent-001> ;
  dcterms:issued "2008-01-14"^^xsd:date ;
  rdfs:comment "A media type or extent."@en ;
  rdfs:isDefinedBy dcterms: ;
  rdfs:label "Media Type or Extent"@en ;
  rdfs:subClassOf rdfs:Resource ;
.
dcterms:MethodOfAccrual
  rdf:type rdfs:Class ;
  dcterms:hasVersion <http://dublincore.org/usage/terms/history/#MethodOfAccrual-001> ;
  dcterms:issued "2008-01-14"^^xsd:date ;
  rdfs:comment "A method by which resources are added to a collection."@en ;
  rdfs:isDefinedBy dcterms: ;
  rdfs:label "Method of Accrual"@en ;
  rdfs:subClassOf rdfs:Resource ;
.
dcterms:MethodOfInstruction
  rdf:type rdfs:Class ;
  dcterms:hasVersion <http://dublincore.org/usage/terms/history/#MethodOfInstruction-001> ;
  dcterms:issued "2008-01-14"^^xsd:date ;
  rdfs:comment "A process that is used to engender knowledge, attitudes, and skills."@en ;
  rdfs:isDefinedBy dcterms: ;
  rdfs:label "Method of Instruction"@en ;
  rdfs:subClassOf rdfs:Resource ;
.
dcterms:NLM
  rdf:type dcam:VocabularyEncodingScheme ;
  dcterms:hasVersion <http://dublincore.org/usage/terms/history/#NLM-002> ;
  dcterms:issued "2005-06-13"^^xsd:date ;
  dcterms:modified "2008-01-14"^^xsd:date ;
  rdfs:comment "The set of conceptual resources specified by the National Library of Medicine Classification."@en ;
  rdfs:isDefinedBy dcterms: ;
  rdfs:label "NLM"@en ;
  rdfs:seeAlso <http://wwwcf.nlm.nih.gov/class/> ;
.
dcterms:Period
  rdf:type rdfs:Datatype ;
  dcterms:hasVersion <http://dublincore.org/usage/terms/history/#Period-003> ;
  dcterms:issued "2000-07-11"^^xsd:date ;
  dcterms:modified "2008-01-14"^^xsd:date ;
  rdfs:comment "The set of time intervals defined by their limits according to the DCMI Period Encoding Scheme."@en ;
  rdfs:isDefinedBy dcterms: ;
  rdfs:label "DCMI Period"@en ;
  rdfs:seeAlso <http://dublincore.org/documents/dcmi-period/> ;
  rdfs:subClassOf rdfs:Resource ;
.
dcterms:PeriodOfTime
  rdf:type rdfs:Class ;
  dcterms:hasVersion <http://dublincore.org/usage/terms/history/#PeriodOfTime-001> ;
  dcterms:issued "2008-01-14"^^xsd:date ;
  rdfs:comment "An interval of time that is named or defined by its start and end dates."@en ;
  rdfs:isDefinedBy dcterms: ;
  rdfs:label "Period of Time"@en ;
  rdfs:subClassOf dcterms:LocationPeriodOrJurisdiction ;
.
dcterms:PhysicalMedium
  rdf:type rdfs:Class ;
  dcterms:description "Examples include paper, canvas, or DVD."@en ;
  dcterms:hasVersion <http://dublincore.org/usage/terms/history/#PhysicalMedium-001> ;
  dcterms:issued "2008-01-14"^^xsd:date ;
  rdfs:comment "A physical material or carrier."@en ;
  rdfs:isDefinedBy dcterms: ;
  rdfs:label "Physical Medium"@en ;
  rdfs:subClassOf dcterms:MediaType ;
.
dcterms:PhysicalResource
  rdf:type rdfs:Class ;
  dcterms:hasVersion <http://dublincore.org/usage/terms/history/#PhysicalResource-001> ;
  dcterms:issued "2008-01-14"^^xsd:date ;
  rdfs:comment "A material thing."@en ;
  rdfs:isDefinedBy dcterms: ;
  rdfs:label "Physical Resource"@en ;
  rdfs:subClassOf rdfs:Resource ;
.
dcterms:Point
  rdf:type rdfs:Datatype ;
  dcterms:hasVersion <http://dublincore.org/usage/terms/history/#Point-003> ;
  dcterms:issued "2000-07-11"^^xsd:date ;
  dcterms:modified "2008-01-14"^^xsd:date ;
  rdfs:comment "The set of points in space defined by their geographic coordinates according to the DCMI Point Encoding Scheme."@en ;
  rdfs:isDefinedBy dcterms: ;
  rdfs:label "DCMI Point"@en ;
  rdfs:seeAlso <http://dublincore.org/documents/dcmi-point/> ;
  rdfs:subClassOf rdfs:Resource ;
.
dcterms:Policy
  rdf:type rdfs:Class ;
  dcterms:hasVersion <http://dublincore.org/usage/terms/history/#Policy-001> ;
  dcterms:issued "2008-01-14"^^xsd:date ;
  rdfs:comment "A plan or course of action by an authority, intended to influence and determine decisions, actions, and other matters."@en ;
  rdfs:isDefinedBy dcterms: ;
  rdfs:label "Policy"@en ;
  rdfs:subClassOf rdfs:Resource ;
.
dcterms:ProvenanceStatement
  rdf:type rdfs:Class ;
  dcterms:hasVersion <http://dublincore.org/usage/terms/history/#ProvenanceStatement-001> ;
  dcterms:issued "2008-01-14"^^xsd:date ;
  rdfs:comment "A statement of any changes in ownership and custody of a resource since its creation that are significant for its authenticity, integrity, and interpretation."@en ;
  rdfs:isDefinedBy dcterms: ;
  rdfs:label "Provenance Statement"@en ;
  rdfs:subClassOf rdfs:Resource ;
.
dcterms:RFC1766
  rdf:type rdfs:Datatype ;
  dcterms:hasVersion <http://dublincore.org/usage/terms/history/#RFC1766-003> ;
  dcterms:issued "2000-07-11"^^xsd:date ;
  dcterms:modified "2008-01-14"^^xsd:date ;
  rdfs:comment "The set of tags, constructed according to RFC 1766, for the identification of languages."@en ;
  rdfs:isDefinedBy dcterms: ;
  rdfs:label "RFC 1766"@en ;
  rdfs:seeAlso <http://www.ietf.org/rfc/rfc1766.txt> ;
  rdfs:subClassOf rdfs:Resource ;
.
dcterms:RFC3066
  rdf:type rdfs:Datatype ;
  dcterms:description "RFC 3066 has been obsoleted by RFC 4646."@en ;
  dcterms:hasVersion <http://dublincore.org/usage/terms/history/#RFC3066-002> ;
  dcterms:issued "2002-07-13"^^xsd:date ;
  dcterms:modified "2008-01-14"^^xsd:date ;
  rdfs:comment "The set of tags constructed according to RFC 3066 for the identification of languages."@en ;
  rdfs:isDefinedBy dcterms: ;
  rdfs:label "RFC 3066"@en ;
  rdfs:seeAlso <http://www.ietf.org/rfc/rfc3066.txt> ;
  rdfs:subClassOf rdfs:Resource ;
.
dcterms:RFC4646
  rdf:type rdfs:Datatype ;
  dcterms:description "RFC 4646 obsoletes RFC 3066."@en ;
  dcterms:hasVersion <http://dublincore.org/usage/terms/history/#RFC4646-001> ;
  dcterms:issued "2008-01-14"^^xsd:date ;
  rdfs:comment "The set of tags constructed according to RFC 4646 for the identification of languages."@en ;
  rdfs:isDefinedBy dcterms: ;
  rdfs:label "RFC 4646"@en ;
  rdfs:seeAlso <http://www.ietf.org/rfc/rfc4646.txt> ;
  rdfs:subClassOf rdfs:Resource ;
.
dcterms:RFC5646
  rdf:type rdfs:Datatype ;
  dcterms:description "RFC 5646 obsoletes RFC 4646."@en ;
  dcterms:hasVersion <http://dublincore.org/usage/terms/history/#RFC5646-001> ;
  dcterms:issued "2010-10-11"^^xsd:date ;
  rdfs:comment "The set of tags constructed according to RFC 5646 for the identification of languages."@en ;
  rdfs:isDefinedBy dcterms: ;
  rdfs:label "RFC 5646"@en ;
  rdfs:seeAlso <http://www.ietf.org/rfc/rfc5646.txt> ;
  rdfs:subClassOf rdfs:Resource ;
.
dcterms:RightsStatement
  rdf:type rdfs:Class ;
  dcterms:hasVersion <http://dublincore.org/usage/terms/history/#RightsStatement-001> ;
  dcterms:issued "2008-01-14"^^xsd:date ;
  rdfs:comment "A statement about the intellectual property rights (IPR) held in or over a Resource, a legal document giving official permission to do something with a resource, or a statement about access rights."@en ;
  rdfs:isDefinedBy dcterms: ;
  rdfs:label "Rights Statement"@en ;
  rdfs:subClassOf rdfs:Resource ;
.
dcterms:SizeOrDuration
  rdf:type rdfs:Class ;
  dcterms:description "Examples include a number of pages, a specification of length, width, and breadth, or a period in hours, minutes, and seconds."@en ;
  dcterms:hasVersion <http://dublincore.org/usage/terms/history/#SizeOrDuration-001> ;
  dcterms:issued "2008-01-14"^^xsd:date ;
  rdfs:comment "A dimension or extent, or a time taken to play or execute."@en ;
  rdfs:isDefinedBy dcterms: ;
  rdfs:label "Size or Duration"@en ;
  rdfs:subClassOf dcterms:MediaTypeOrExtent ;
.
dcterms:Standard
  rdf:type rdfs:Class ;
  dcterms:hasVersion <http://dublincore.org/usage/terms/history/#Standard-001> ;
  dcterms:issued "2008-01-14"^^xsd:date ;
  rdfs:comment "A basis for comparison; a reference point against which other things can be evaluated."@en ;
  rdfs:isDefinedBy dcterms: ;
  rdfs:label "Standard"@en ;
  rdfs:subClassOf rdfs:Resource ;
.
dcterms:TGN
  rdf:type dcam:VocabularyEncodingScheme ;
  dcterms:hasVersion <http://dublincore.org/usage/terms/history/#TGN-003> ;
  dcterms:issued "2000-07-11"^^xsd:date ;
  dcterms:modified "2008-01-14"^^xsd:date ;
  rdfs:comment "The set of places specified by the Getty Thesaurus of Geographic Names."@en ;
  rdfs:isDefinedBy dcterms: ;
  rdfs:label "TGN"@en ;
  rdfs:seeAlso <http://www.getty.edu/research/tools/vocabulary/tgn/index.html> ;
.
dcterms:UDC
  rdf:type dcam:VocabularyEncodingScheme ;
  dcterms:hasVersion <http://dublincore.org/usage/terms/history/#UDC-003> ;
  dcterms:issued "2000-07-11"^^xsd:date ;
  dcterms:modified "2008-01-14"^^xsd:date ;
  rdfs:comment "The set of conceptual resources specified by the Universal Decimal Classification."@en ;
  rdfs:isDefinedBy dcterms: ;
  rdfs:label "UDC"@en ;
  rdfs:seeAlso <http://www.udcc.org/> ;
.
dcterms:URI
  rdf:type rdfs:Datatype ;
  dcterms:hasVersion <http://dublincore.org/usage/terms/history/#URI-003> ;
  dcterms:issued "2000-07-11"^^xsd:date ;
  dcterms:modified "2008-01-14"^^xsd:date ;
  rdfs:comment "The set of identifiers constructed according to the generic syntax for Uniform Resource Identifiers as specified by the Internet Engineering Task Force."@en ;
  rdfs:isDefinedBy dcterms: ;
  rdfs:label "URI"@en ;
  rdfs:seeAlso <http://www.ietf.org/rfc/rfc3986.txt> ;
  rdfs:subClassOf rdfs:Resource ;
.
dcterms:W3CDTF
  rdf:type rdfs:Datatype ;
  dcterms:hasVersion <http://dublincore.org/usage/terms/history/#W3CDTF-003> ;
  dcterms:issued "2000-07-11"^^xsd:date ;
  dcterms:modified "2008-01-14"^^xsd:date ;
  rdfs:comment "The set of dates and times constructed according to the W3C Date and Time Formats Specification."@en ;
  rdfs:isDefinedBy dcterms: ;
  rdfs:label "W3C-DTF"@en ;
  rdfs:seeAlso <http://www.w3.org/TR/NOTE-datetime> ;
  rdfs:subClassOf rdfs:Resource ;
.
dcterms:abstract
  rdf:type rdf:Property ;
  dcterms:hasVersion <http://dublincore.org/usage/terms/history/#abstract-003> ;
  dcterms:issued "2000-07-11"^^xsd:date ;
  dcterms:modified "2008-01-14"^^xsd:date ;
  rdfs:comment "A summary of the resource."@en ;
  rdfs:isDefinedBy dcterms: ;
  rdfs:label "Abstract"@en ;
  rdfs:subPropertyOf dc:description ;
  rdfs:subPropertyOf dcterms:description ;
.
dcterms:accessRights
  rdf:type rdf:Property ;
  dcterms:description "Access Rights may include information regarding access or restrictions based on privacy, security, or other policies."@en ;
  dcterms:hasVersion <http://dublincore.org/usage/terms/history/#accessRights-002> ;
  dcterms:issued "2003-02-15"^^xsd:date ;
  dcterms:modified "2008-01-14"^^xsd:date ;
  rdfs:comment "Information about who can access the resource or an indication of its security status."@en ;
  rdfs:isDefinedBy dcterms: ;
  rdfs:label "Access Rights"@en ;
  rdfs:range dcterms:RightsStatement ;
  rdfs:subPropertyOf dc:rights ;
  rdfs:subPropertyOf dcterms:rights ;
.
dcterms:accrualMethod
  rdf:type rdf:Property ;
  dcterms:hasVersion <http://dublincore.org/usage/terms/history/#accrualMethod-003> ;
  dcterms:issued "2005-06-13"^^xsd:date ;
  dcterms:modified "2010-10-11"^^xsd:date ;
  rdfs:comment "The method by which items are added to a collection."@en ;
  rdfs:domain <http://purl.org/dc/dcmitype/Collection> ;
  rdfs:isDefinedBy dcterms: ;
  rdfs:label "Accrual Method"@en ;
  rdfs:range dcterms:MethodOfAccrual ;
.
dcterms:accrualPeriodicity
  rdf:type rdf:Property ;
  dcterms:hasVersion <http://dublincore.org/usage/terms/history/#accrualPeriodicity-003> ;
  dcterms:issued "2005-06-13"^^xsd:date ;
  dcterms:modified "2010-10-11"^^xsd:date ;
  rdfs:comment "The frequency with which items are added to a collection."@en ;
  rdfs:domain <http://purl.org/dc/dcmitype/Collection> ;
  rdfs:isDefinedBy dcterms: ;
  rdfs:label "Accrual Periodicity"@en ;
  rdfs:range dcterms:Frequency ;
.
dcterms:accrualPolicy
  rdf:type rdf:Property ;
  dcterms:hasVersion <http://dublincore.org/usage/terms/history/#accrualPolicy-003> ;
  dcterms:issued "2005-06-13"^^xsd:date ;
  dcterms:modified "2010-10-11"^^xsd:date ;
  rdfs:comment "The policy governing the addition of items to a collection."@en ;
  rdfs:domain <http://purl.org/dc/dcmitype/Collection> ;
  rdfs:isDefinedBy dcterms: ;
  rdfs:label "Accrual Policy"@en ;
  rdfs:range dcterms:Policy ;
.
dcterms:alternative
  rdf:type rdf:Property ;
  dcterms:description "The distinction between titles and alternative titles is application-specific."@en ;
  dcterms:hasVersion <http://dublincore.org/usage/terms/history/#alternative-003> ;
  dcterms:issued "2000-07-11"^^xsd:date ;
  dcterms:modified "2010-10-11"^^xsd:date ;
  rdfs:comment "An alternative name for the resource."@en ;
  rdfs:isDefinedBy dcterms: ;
  rdfs:label "Alternative Title"@en ;
  rdfs:range rdfs:Literal ;
  rdfs:subPropertyOf dc:title ;
  rdfs:subPropertyOf dcterms:title ;
.
dcterms:audience
  rdf:type rdf:Property ;
  dcterms:hasVersion <http://dublincore.org/usage/terms/history/#audience-003> ;
  dcterms:issued "2001-05-21"^^xsd:date ;
  dcterms:modified "2008-01-14"^^xsd:date ;
  rdfs:comment "A class of entity for whom the resource is intended or useful."@en ;
  rdfs:isDefinedBy dcterms: ;
  rdfs:label "Audience"@en ;
  rdfs:range dcterms:AgentClass ;
.
dcterms:available
  rdf:type rdf:Property ;
  dcterms:hasVersion <http://dublincore.org/usage/terms/history/#available-003> ;
  dcterms:issued "2000-07-11"^^xsd:date ;
  dcterms:modified "2008-01-14"^^xsd:date ;
  rdfs:comment "Date (often a range) that the resource became or will become available."@en ;
  rdfs:isDefinedBy dcterms: ;
  rdfs:label "Date Available"@en ;
  rdfs:range rdfs:Literal ;
  rdfs:subPropertyOf dc:date ;
  rdfs:subPropertyOf dcterms:date ;
.
dcterms:bibliographicCitation
  rdf:type rdf:Property ;
  dcterms:description "Recommended practice is to include sufficient bibliographic detail to identify the resource as unambiguously as possible."@en ;
  dcterms:hasVersion <http://dublincore.org/usage/terms/history/#bibliographicCitation-002> ;
  dcterms:issued "2003-02-15"^^xsd:date ;
  dcterms:modified "2008-01-14"^^xsd:date ;
  rdfs:comment "A bibliographic reference for the resource."@en ;
  rdfs:domain dcterms:BibliographicResource ;
  rdfs:isDefinedBy dcterms: ;
  rdfs:label "Bibliographic Citation"@en ;
  rdfs:range rdfs:Literal ;
  rdfs:subPropertyOf dc:identifier ;
  rdfs:subPropertyOf dcterms:identifier ;
.
dcterms:conformsTo
  rdf:type rdf:Property ;
  dcterms:hasVersion <http://dublincore.org/usage/terms/history/#conformsTo-003> ;
  dcterms:issued "2001-05-21"^^xsd:date ;
  dcterms:modified "2008-01-14"^^xsd:date ;
  rdfs:comment "An established standard to which the described resource conforms."@en ;
  rdfs:isDefinedBy dcterms: ;
  rdfs:label "Conforms To"@en ;
  rdfs:range dcterms:Standard ;
  rdfs:subPropertyOf dc:relation ;
  rdfs:subPropertyOf dcterms:relation ;
.
dcterms:contributor
  rdf:type rdf:Property ;
  dcterms:description "Examples of a Contributor include a person, an organization, or a service."@en ;
  dcterms:hasVersion <http://dublincore.org/usage/terms/history/#contributorT-001> ;
  dcterms:issued "2008-01-14"^^xsd:date ;
  dcterms:modified "2010-10-11"^^xsd:date ;
  rdfs:comment "An entity responsible for making contributions to the resource."@en ;
  rdfs:isDefinedBy dcterms: ;
  rdfs:label "Contributor"@en ;
  rdfs:range dcterms:Agent ;
  rdfs:subPropertyOf dc:contributor ;
.
dcterms:coverage
  rdf:type rdf:Property ;
  dcterms:description "Spatial topic and spatial applicability may be a named place or a location specified by its geographic coordinates. Temporal topic may be a named period, date, or date range. A jurisdiction may be a named administrative entity or a geographic place to which the resource applies. Recommended best practice is to use a controlled vocabulary such as the Thesaurus of Geographic Names [TGN]. Where appropriate, named places or time periods can be used in preference to numeric identifiers such as sets of coordinates or date ranges."@en ;
  dcterms:hasVersion <http://dublincore.org/usage/terms/history/#coverageT-001> ;
  dcterms:issued "2008-01-14"^^xsd:date ;
  dcterms:modified "2008-01-14"^^xsd:date ;
  rdfs:comment "The spatial or temporal topic of the resource, the spatial applicability of the resource, or the jurisdiction under which the resource is relevant."@en ;
  rdfs:isDefinedBy dcterms: ;
  rdfs:label "Coverage"@en ;
  rdfs:range dcterms:LocationPeriodOrJurisdiction ;
  rdfs:subPropertyOf dc:coverage ;
.
dcterms:created
  rdf:type rdf:Property ;
  dcterms:hasVersion <http://dublincore.org/usage/terms/history/#created-003> ;
  dcterms:issued "2000-07-11"^^xsd:date ;
  dcterms:modified "2008-01-14"^^xsd:date ;
  rdfs:comment "Date of creation of the resource."@en ;
  rdfs:isDefinedBy dcterms: ;
  rdfs:label "Date Created"@en ;
  rdfs:range rdfs:Literal ;
  rdfs:subPropertyOf dc:date ;
  rdfs:subPropertyOf dcterms:date ;
.
dcterms:creator
  rdf:type rdf:Property ;
  dcterms:description "Examples of a Creator include a person, an organization, or a service."@en ;
  dcterms:hasVersion <http://dublincore.org/usage/terms/history/#creatorT-002> ;
  dcterms:issued "2008-01-14"^^xsd:date ;
  dcterms:modified "2010-10-11"^^xsd:date ;
  rdfs:comment "An entity primarily responsible for making the resource."@en ;
  rdfs:isDefinedBy dcterms: ;
  rdfs:label "Creator"@en ;
  rdfs:range dcterms:Agent ;
  rdfs:subPropertyOf dc:creator ;
  rdfs:subPropertyOf dcterms:contributor ;
  owl:equivalentProperty foaf:maker ;
.
dcterms:date
  rdf:type rdf:Property ;
  dcterms:description "Date may be used to express temporal information at any level of granularity.  Recommended best practice is to use an encoding scheme, such as the W3CDTF profile of ISO 8601 [W3CDTF]."@en ;
  dcterms:hasVersion <http://dublincore.org/usage/terms/history/#dateT-001> ;
  dcterms:issued "2008-01-14"^^xsd:date ;
  dcterms:modified "2008-01-14"^^xsd:date ;
  rdfs:comment "A point or period of time associated with an event in the lifecycle of the resource."@en ;
  rdfs:isDefinedBy dcterms: ;
  rdfs:label "Date"@en ;
  rdfs:range rdfs:Literal ;
  rdfs:subPropertyOf dc:date ;
.
dcterms:dateAccepted
  rdf:type rdf:Property ;
  dcterms:description "Examples of resources to which a Date Accepted may be relevant are a thesis (accepted by a university department) or an article (accepted by a journal)."@en ;
  dcterms:hasVersion <http://dublincore.org/usage/terms/history/#dateAccepted-002> ;
  dcterms:issued "2002-07-13"^^xsd:date ;
  dcterms:modified "2008-01-14"^^xsd:date ;
  rdfs:comment "Date of acceptance of the resource."@en ;
  rdfs:isDefinedBy dcterms: ;
  rdfs:label "Date Accepted"@en ;
  rdfs:range rdfs:Literal ;
  rdfs:subPropertyOf dc:date ;
  rdfs:subPropertyOf dcterms:date ;
.
dcterms:dateCopyrighted
  rdf:type rdf:Property ;
  dcterms:hasVersion <http://dublincore.org/usage/terms/history/#dateCopyrighted-002> ;
  dcterms:issued "2002-07-13"^^xsd:date ;
  dcterms:modified "2008-01-14"^^xsd:date ;
  rdfs:comment "Date of copyright."@en ;
  rdfs:isDefinedBy dcterms: ;
  rdfs:label "Date Copyrighted"@en ;
  rdfs:range rdfs:Literal ;
  rdfs:subPropertyOf dc:date ;
  rdfs:subPropertyOf dcterms:date ;
.
dcterms:dateSubmitted
  rdf:type rdf:Property ;
  dcterms:description "Examples of resources to which a Date Submitted may be relevant are a thesis (submitted to a university department) or an article (submitted to a journal)."@en ;
  dcterms:hasVersion <http://dublincore.org/usage/terms/history/#dateSubmitted-002> ;
  dcterms:issued "2002-07-13"^^xsd:date ;
  dcterms:modified "2008-01-14"^^xsd:date ;
  rdfs:comment "Date of submission of the resource."@en ;
  rdfs:isDefinedBy dcterms: ;
  rdfs:label "Date Submitted"@en ;
  rdfs:range rdfs:Literal ;
  rdfs:subPropertyOf dc:date ;
  rdfs:subPropertyOf dcterms:date ;
.
dcterms:description
  rdf:type rdf:Property ;
  dcterms:description "Description may include but is not limited to: an abstract, a table of contents, a graphical representation, or a free-text account of the resource."@en ;
  dcterms:hasVersion <http://dublincore.org/usage/terms/history/#descriptionT-001> ;
  dcterms:issued "2008-01-14"^^xsd:date ;
  dcterms:modified "2008-01-14"^^xsd:date ;
  rdfs:comment "An account of the resource."@en ;
  rdfs:isDefinedBy dcterms: ;
  rdfs:label "Description"@en ;
  rdfs:subPropertyOf dc:description ;
.
dcterms:educationLevel
  rdf:type rdf:Property ;
  dcterms:hasVersion <http://dublincore.org/usage/terms/history/#educationLevel-002> ;
  dcterms:issued "2002-07-13"^^xsd:date ;
  dcterms:modified "2008-01-14"^^xsd:date ;
  rdfs:comment "A class of entity, defined in terms of progression through an educational or training context, for which the described resource is intended."@en ;
  rdfs:isDefinedBy dcterms: ;
  rdfs:label "Audience Education Level"@en ;
  rdfs:range dcterms:AgentClass ;
  rdfs:subPropertyOf dcterms:audience ;
.
dcterms:extent
  rdf:type rdf:Property ;
  dcterms:hasVersion <http://dublincore.org/usage/terms/history/#extent-003> ;
  dcterms:issued "2000-07-11"^^xsd:date ;
  dcterms:modified "2008-01-14"^^xsd:date ;
  rdfs:comment "The size or duration of the resource."@en ;
  rdfs:isDefinedBy dcterms: ;
  rdfs:label "Extent"@en ;
  rdfs:range dcterms:SizeOrDuration ;
  rdfs:subPropertyOf dc:format ;
  rdfs:subPropertyOf dcterms:format ;
.
dcterms:format
  rdf:type rdf:Property ;
  dcterms:description "Examples of dimensions include size and duration. Recommended best practice is to use a controlled vocabulary such as the list of Internet Media Types [MIME]."@en ;
  dcterms:hasVersion <http://dublincore.org/usage/terms/history/#formatT-001> ;
  dcterms:issued "2008-01-14"^^xsd:date ;
  dcterms:modified "2008-01-14"^^xsd:date ;
  rdfs:comment "The file format, physical medium, or dimensions of the resource."@en ;
  rdfs:isDefinedBy dcterms: ;
  rdfs:label "Format"@en ;
  rdfs:range dcterms:MediaTypeOrExtent ;
  rdfs:subPropertyOf dc:format ;
.
dcterms:hasFormat
  rdf:type rdf:Property ;
  dcterms:hasVersion <http://dublincore.org/usage/terms/history/#hasFormat-003> ;
  dcterms:issued "2000-07-11"^^xsd:date ;
  dcterms:modified "2008-01-14"^^xsd:date ;
  rdfs:comment "A related resource that is substantially the same as the pre-existing described resource, but in another format."@en ;
  rdfs:isDefinedBy dcterms: ;
  rdfs:label "Has Format"@en ;
  rdfs:subPropertyOf dc:relation ;
  rdfs:subPropertyOf dcterms:relation ;
  skos:note "This term is intended to be used with non-literal values as defined in the DCMI Abstract Model (http://dublincore.org/documents/abstract-model/).  As of December 2007, the DCMI Usage Board is seeking a way to express this intention with a formal range declaration."@en ;
.
dcterms:hasPart
  rdf:type rdf:Property ;
  dcterms:hasVersion <http://dublincore.org/usage/terms/history/#hasPart-003> ;
  dcterms:issued "2000-07-11"^^xsd:date ;
  dcterms:modified "2008-01-14"^^xsd:date ;
  rdfs:comment "A related resource that is included either physically or logically in the described resource."@en ;
  rdfs:isDefinedBy dcterms: ;
  rdfs:label "Has Part"@en ;
  rdfs:subPropertyOf dc:relation ;
  rdfs:subPropertyOf dcterms:relation ;
  skos:note "This term is intended to be used with non-literal values as defined in the DCMI Abstract Model (http://dublincore.org/documents/abstract-model/).  As of December 2007, the DCMI Usage Board is seeking a way to express this intention with a formal range declaration."@en ;
.
dcterms:hasVersion
  rdf:type rdf:Property ;
  dcterms:hasVersion <http://dublincore.org/usage/terms/history/#hasVersion-003> ;
  dcterms:issued "2000-07-11"^^xsd:date ;
  dcterms:modified "2008-01-14"^^xsd:date ;
  rdfs:comment "A related resource that is a version, edition, or adaptation of the described resource."@en ;
  rdfs:isDefinedBy dcterms: ;
  rdfs:label "Has Version"@en ;
  rdfs:subPropertyOf dc:relation ;
  rdfs:subPropertyOf dcterms:relation ;
  skos:note "This term is intended to be used with non-literal values as defined in the DCMI Abstract Model (http://dublincore.org/documents/abstract-model/).  As of December 2007, the DCMI Usage Board is seeking a way to express this intention with a formal range declaration."@en ;
.
dcterms:identifier
  rdf:type rdf:Property ;
  dcterms:description "Recommended best practice is to identify the resource by means of a string conforming to a formal identification system. "@en ;
  dcterms:hasVersion <http://dublincore.org/usage/terms/history/#identifierT-001> ;
  dcterms:issued "2008-01-14"^^xsd:date ;
  dcterms:modified "2008-01-14"^^xsd:date ;
  rdfs:comment "An unambiguous reference to the resource within a given context."@en ;
  rdfs:isDefinedBy dcterms: ;
  rdfs:label "Identifier"@en ;
  rdfs:range rdfs:Literal ;
  rdfs:subPropertyOf dc:identifier ;
.
dcterms:instructionalMethod
  rdf:type rdf:Property ;
  dcterms:description "Instructional Method will typically include ways of presenting instructional materials or conducting instructional activities, patterns of learner-to-learner and learner-to-instructor interactions, and mechanisms by which group and individual levels of learning are measured.  Instructional methods include all aspects of the instruction and learning processes from planning and implementation through evaluation and feedback."@en ;
  dcterms:hasVersion <http://dublincore.org/usage/terms/history/#instructionalMethod-002> ;
  dcterms:issued "2005-06-13"^^xsd:date ;
  dcterms:modified "2008-01-14"^^xsd:date ;
  rdfs:comment "A process, used to engender knowledge, attitudes and skills, that the described resource is designed to support."@en ;
  rdfs:isDefinedBy dcterms: ;
  rdfs:label "Instructional Method"@en ;
  rdfs:range dcterms:MethodOfInstruction ;
.
dcterms:isFormatOf
  rdf:type rdf:Property ;
  dcterms:hasVersion <http://dublincore.org/usage/terms/history/#isFormatOf-003> ;
  dcterms:issued "2000-07-11"^^xsd:date ;
  dcterms:modified "2008-01-14"^^xsd:date ;
  rdfs:comment "A related resource that is substantially the same as the described resource, but in another format."@en ;
  rdfs:isDefinedBy dcterms: ;
  rdfs:label "Is Format Of"@en ;
  rdfs:subPropertyOf dc:relation ;
  rdfs:subPropertyOf dcterms:relation ;
  skos:note "This term is intended to be used with non-literal values as defined in the DCMI Abstract Model (http://dublincore.org/documents/abstract-model/).  As of December 2007, the DCMI Usage Board is seeking a way to express this intention with a formal range declaration."@en ;
.
dcterms:isPartOf
  rdf:type rdf:Property ;
  dcterms:hasVersion <http://dublincore.org/usage/terms/history/#isPartOf-003> ;
  dcterms:issued "2000-07-11"^^xsd:date ;
  dcterms:modified "2008-01-14"^^xsd:date ;
  rdfs:comment "A related resource in which the described resource is physically or logically included."@en ;
  rdfs:isDefinedBy dcterms: ;
  rdfs:label "Is Part Of"@en ;
  rdfs:subPropertyOf dc:relation ;
  rdfs:subPropertyOf dcterms:relation ;
  skos:note "This term is intended to be used with non-literal values as defined in the DCMI Abstract Model (http://dublincore.org/documents/abstract-model/).  As of December 2007, the DCMI Usage Board is seeking a way to express this intention with a formal range declaration."@en ;
.
dcterms:isReferencedBy
  rdf:type rdf:Property ;
  dcterms:hasVersion <http://dublincore.org/usage/terms/history/#isReferencedBy-003> ;
  dcterms:issued "2000-07-11"^^xsd:date ;
  dcterms:modified "2008-01-14"^^xsd:date ;
  rdfs:comment "A related resource that references, cites, or otherwise points to the described resource."@en ;
  rdfs:isDefinedBy dcterms: ;
  rdfs:label "Is Referenced By"@en ;
  rdfs:subPropertyOf dc:relation ;
  rdfs:subPropertyOf dcterms:relation ;
  skos:note "This term is intended to be used with non-literal values as defined in the DCMI Abstract Model (http://dublincore.org/documents/abstract-model/).  As of December 2007, the DCMI Usage Board is seeking a way to express this intention with a formal range declaration."@en ;
.
dcterms:isReplacedBy
  rdf:type rdf:Property ;
  dcterms:hasVersion <http://dublincore.org/usage/terms/history/#isReplacedBy-003> ;
  dcterms:issued "2000-07-11"^^xsd:date ;
  dcterms:modified "2008-01-14"^^xsd:date ;
  rdfs:comment "A related resource that supplants, displaces, or supersedes the described resource."@en ;
  rdfs:isDefinedBy dcterms: ;
  rdfs:label "Is Replaced By"@en ;
  rdfs:subPropertyOf dc:relation ;
  rdfs:subPropertyOf dcterms:relation ;
  skos:note "This term is intended to be used with non-literal values as defined in the DCMI Abstract Model (http://dublincore.org/documents/abstract-model/).  As of December 2007, the DCMI Usage Board is seeking a way to express this intention with a formal range declaration."@en ;
.
dcterms:isRequiredBy
  rdf:type rdf:Property ;
  dcterms:hasVersion <http://dublincore.org/usage/terms/history/#isRequiredBy-003> ;
  dcterms:issued "2000-07-11"^^xsd:date ;
  dcterms:modified "2008-01-14"^^xsd:date ;
  rdfs:comment "A related resource that requires the described resource to support its function, delivery, or coherence."@en ;
  rdfs:isDefinedBy dcterms: ;
  rdfs:label "Is Required By"@en ;
  rdfs:subPropertyOf dc:relation ;
  rdfs:subPropertyOf dcterms:relation ;
  skos:note "This term is intended to be used with non-literal values as defined in the DCMI Abstract Model (http://dublincore.org/documents/abstract-model/).  As of December 2007, the DCMI Usage Board is seeking a way to express this intention with a formal range declaration."@en ;
.
dcterms:isVersionOf
  rdf:type rdf:Property ;
  dcterms:description "Changes in version imply substantive changes in content rather than differences in format."@en ;
  dcterms:hasVersion <http://dublincore.org/usage/terms/history/#isVersionOf-003> ;
  dcterms:issued "2000-07-11"^^xsd:date ;
  dcterms:modified "2008-01-14"^^xsd:date ;
  rdfs:comment "A related resource of which the described resource is a version, edition, or adaptation."@en ;
  rdfs:isDefinedBy dcterms: ;
  rdfs:label "Is Version Of"@en ;
  rdfs:subPropertyOf dc:relation ;
  rdfs:subPropertyOf dcterms:relation ;
  skos:note "This term is intended to be used with non-literal values as defined in the DCMI Abstract Model (http://dublincore.org/documents/abstract-model/).  As of December 2007, the DCMI Usage Board is seeking a way to express this intention with a formal range declaration."@en ;
.
dcterms:issued
  rdf:type rdf:Property ;
  dcterms:hasVersion <http://dublincore.org/usage/terms/history/#issued-003> ;
  dcterms:issued "2000-07-11"^^xsd:date ;
  dcterms:modified "2008-01-14"^^xsd:date ;
  rdfs:comment "Date of formal issuance (e.g., publication) of the resource."@en ;
  rdfs:isDefinedBy dcterms: ;
  rdfs:label "Date Issued"@en ;
  rdfs:range rdfs:Literal ;
  rdfs:subPropertyOf dc:date ;
  rdfs:subPropertyOf dcterms:date ;
.
dcterms:language
  rdf:type rdf:Property ;
  dcterms:description "Recommended best practice is to use a controlled vocabulary such as RFC 4646 [RFC4646]."@en ;
  dcterms:hasVersion <http://dublincore.org/usage/terms/history/#languageT-001> ;
  dcterms:issued "2008-01-14"^^xsd:date ;
  dcterms:modified "2008-01-14"^^xsd:date ;
  rdfs:comment "A language of the resource."@en ;
  rdfs:isDefinedBy dcterms: ;
  rdfs:label "Language"@en ;
  rdfs:range dcterms:LinguisticSystem ;
  rdfs:subPropertyOf dc:language ;
.
dcterms:license
  rdf:type rdf:Property ;
  dcterms:hasVersion <http://dublincore.org/usage/terms/history/#license-002> ;
  dcterms:issued "2004-06-14"^^xsd:date ;
  dcterms:modified "2008-01-14"^^xsd:date ;
  rdfs:comment "A legal document giving official permission to do something with the resource."@en ;
  rdfs:isDefinedBy dcterms: ;
  rdfs:label "License"@en ;
  rdfs:range dcterms:LicenseDocument ;
  rdfs:subPropertyOf dc:rights ;
  rdfs:subPropertyOf dcterms:rights ;
.
dcterms:mediator
  rdf:type rdf:Property ;
  dcterms:description "In an educational context, a mediator might be a parent, teacher, teaching assistant, or care-giver."@en ;
  dcterms:hasVersion <http://dublincore.org/usage/terms/history/#mediator-003> ;
  dcterms:issued "2001-05-21"^^xsd:date ;
  dcterms:modified "2008-01-14"^^xsd:date ;
  rdfs:comment "An entity that mediates access to the resource and for whom the resource is intended or useful."@en ;
  rdfs:isDefinedBy dcterms: ;
  rdfs:label "Mediator"@en ;
  rdfs:range dcterms:AgentClass ;
  rdfs:subPropertyOf dcterms:audience ;
.
dcterms:medium
  rdf:type rdf:Property ;
  dcterms:hasVersion <http://dublincore.org/usage/terms/history/#medium-003> ;
  dcterms:issued "2000-07-11"^^xsd:date ;
  dcterms:modified "2008-01-14"^^xsd:date ;
  rdfs:comment "The material or physical carrier of the resource."@en ;
  rdfs:domain dcterms:PhysicalResource ;
  rdfs:isDefinedBy dcterms: ;
  rdfs:label "Medium"@en ;
  rdfs:range dcterms:PhysicalMedium ;
  rdfs:subPropertyOf dc:format ;
  rdfs:subPropertyOf dcterms:format ;
.
dcterms:modified
  rdf:type rdf:Property ;
  dcterms:hasVersion <http://dublincore.org/usage/terms/history/#modified-003> ;
  dcterms:issued "2000-07-11"^^xsd:date ;
  dcterms:modified "2008-01-14"^^xsd:date ;
  rdfs:comment "Date on which the resource was changed."@en ;
  rdfs:isDefinedBy dcterms: ;
  rdfs:label "Date Modified"@en ;
  rdfs:range rdfs:Literal ;
  rdfs:subPropertyOf dc:date ;
  rdfs:subPropertyOf dcterms:date ;
.
dcterms:provenance
  rdf:type rdf:Property ;
  dcterms:description "The statement may include a description of any changes successive custodians made to the resource."@en ;
  dcterms:hasVersion <http://dublincore.org/usage/terms/history/#provenance-002> ;
  dcterms:issued "2004-09-20"^^xsd:date ;
  dcterms:modified "2008-01-14"^^xsd:date ;
  rdfs:comment "A statement of any changes in ownership and custody of the resource since its creation that are significant for its authenticity, integrity, and interpretation."@en ;
  rdfs:isDefinedBy dcterms: ;
  rdfs:label "Provenance"@en ;
  rdfs:range dcterms:ProvenanceStatement ;
.
dcterms:publisher
  rdf:type rdf:Property ;
  dcterms:description "Examples of a Publisher include a person, an organization, or a service."@en ;
  dcterms:hasVersion <http://dublincore.org/usage/terms/history/#publisherT-001> ;
  dcterms:issued "2008-01-14"^^xsd:date ;
  dcterms:modified "2010-10-11"^^xsd:date ;
  rdfs:comment "An entity responsible for making the resource available."@en ;
  rdfs:isDefinedBy dcterms: ;
  rdfs:label "Publisher"@en ;
  rdfs:range dcterms:Agent ;
  rdfs:subPropertyOf dc:publisher ;
.
dcterms:references
  rdf:type rdf:Property ;
  dcterms:hasVersion <http://dublincore.org/usage/terms/history/#references-003> ;
  dcterms:issued "2000-07-11"^^xsd:date ;
  dcterms:modified "2008-01-14"^^xsd:date ;
  rdfs:comment "A related resource that is referenced, cited, or otherwise pointed to by the described resource."@en ;
  rdfs:isDefinedBy dcterms: ;
  rdfs:label "References"@en ;
  rdfs:subPropertyOf dc:relation ;
  rdfs:subPropertyOf dcterms:relation ;
  skos:note "This term is intended to be used with non-literal values as defined in the DCMI Abstract Model (http://dublincore.org/documents/abstract-model/).  As of December 2007, the DCMI Usage Board is seeking a way to express this intention with a formal range declaration."@en ;
.
dcterms:relation
  rdf:type rdf:Property ;
  dcterms:description "Recommended best practice is to identify the related resource by means of a string conforming to a formal identification system. "@en ;
  dcterms:hasVersion <http://dublincore.org/usage/terms/history/#relationT-001> ;
  dcterms:issued "2008-01-14"^^xsd:date ;
  dcterms:modified "2008-01-14"^^xsd:date ;
  rdfs:comment "A related resource."@en ;
  rdfs:isDefinedBy dcterms: ;
  rdfs:label "Relation"@en ;
  rdfs:subPropertyOf dc:relation ;
  skos:note "This term is intended to be used with non-literal values as defined in the DCMI Abstract Model (http://dublincore.org/documents/abstract-model/).  As of December 2007, the DCMI Usage Board is seeking a way to express this intention with a formal range declaration."@en ;
.
dcterms:replaces
  rdf:type rdf:Property ;
  dcterms:hasVersion <http://dublincore.org/usage/terms/history/#replaces-003> ;
  dcterms:issued "2000-07-11"^^xsd:date ;
  dcterms:modified "2008-01-14"^^xsd:date ;
  rdfs:comment "A related resource that is supplanted, displaced, or superseded by the described resource."@en ;
  rdfs:isDefinedBy dcterms: ;
  rdfs:label "Replaces"@en ;
  rdfs:subPropertyOf dc:relation ;
  rdfs:subPropertyOf dcterms:relation ;
  skos:note "This term is intended to be used with non-literal values as defined in the DCMI Abstract Model (http://dublincore.org/documents/abstract-model/).  As of December 2007, the DCMI Usage Board is seeking a way to express this intention with a formal range declaration."@en ;
.
dcterms:requires
  rdf:type rdf:Property ;
  dcterms:hasVersion <http://dublincore.org/usage/terms/history/#requires-003> ;
  dcterms:issued "2000-07-11"^^xsd:date ;
  dcterms:modified "2008-01-14"^^xsd:date ;
  rdfs:comment "A related resource that is required by the described resource to support its function, delivery, or coherence."@en ;
  rdfs:isDefinedBy dcterms: ;
  rdfs:label "Requires"@en ;
  rdfs:subPropertyOf dc:relation ;
  rdfs:subPropertyOf dcterms:relation ;
  skos:note "This term is intended to be used with non-literal values as defined in the DCMI Abstract Model (http://dublincore.org/documents/abstract-model/).  As of December 2007, the DCMI Usage Board is seeking a way to express this intention with a formal range declaration."@en ;
.
dcterms:rights
  rdf:type rdf:Property ;
  dcterms:description "Typically, rights information includes a statement about various property rights associated with the resource, including intellectual property rights."@en ;
  dcterms:hasVersion <http://dublincore.org/usage/terms/history/#rightsT-001> ;
  dcterms:issued "2008-01-14"^^xsd:date ;
  dcterms:modified "2008-01-14"^^xsd:date ;
  rdfs:comment "Information about rights held in and over the resource."@en ;
  rdfs:isDefinedBy dcterms: ;
  rdfs:label "Rights"@en ;
  rdfs:range dcterms:RightsStatement ;
  rdfs:subPropertyOf dc:rights ;
.
dcterms:rightsHolder
  rdf:type rdf:Property ;
  dcterms:hasVersion <http://dublincore.org/usage/terms/history/#rightsHolder-002> ;
  dcterms:issued "2004-06-14"^^xsd:date ;
  dcterms:modified "2008-01-14"^^xsd:date ;
  rdfs:comment "A person or organization owning or managing rights over the resource."@en ;
  rdfs:isDefinedBy dcterms: ;
  rdfs:label "Rights Holder"@en ;
  rdfs:range dcterms:Agent ;
.
dcterms:source
  rdf:type rdf:Property ;
  dcterms:description "The described resource may be derived from the related resource in whole or in part. Recommended best practice is to identify the related resource by means of a string conforming to a formal identification system."@en ;
  dcterms:hasVersion <http://dublincore.org/usage/terms/history/#sourceT-001> ;
  dcterms:issued "2008-01-14"^^xsd:date ;
  dcterms:modified "2008-01-14"^^xsd:date ;
  rdfs:comment "A related resource from which the described resource is derived."@en ;
  rdfs:isDefinedBy dcterms: ;
  rdfs:label "Source"@en ;
  rdfs:subPropertyOf dc:source ;
  rdfs:subPropertyOf dcterms:relation ;
  skos:note "This term is intended to be used with non-literal values as defined in the DCMI Abstract Model (http://dublincore.org/documents/abstract-model/).  As of December 2007, the DCMI Usage Board is seeking a way to express this intention with a formal range declaration."@en ;
.
dcterms:spatial
  rdf:type rdf:Property ;
  dcterms:hasVersion <http://dublincore.org/usage/terms/history/#spatial-003> ;
  dcterms:issued "2000-07-11"^^xsd:date ;
  dcterms:modified "2008-01-14"^^xsd:date ;
  rdfs:comment "Spatial characteristics of the resource."@en ;
  rdfs:isDefinedBy dcterms: ;
  rdfs:label "Spatial Coverage"@en ;
  rdfs:range dcterms:Location ;
  rdfs:subPropertyOf dc:coverage ;
  rdfs:subPropertyOf dcterms:coverage ;
.
dcterms:subject
  rdf:type rdf:Property ;
  dcterms:description "Typically, the subject will be represented using keywords, key phrases, or classification codes. Recommended best practice is to use a controlled vocabulary."@en ;
  dcterms:hasVersion <http://dublincore.org/usage/terms/history/#subjectT-002> ;
  dcterms:issued "2008-01-14"^^xsd:date ;
  dcterms:modified "2012-06-14"^^xsd:date ;
  rdfs:comment "The topic of the resource."@en ;
  rdfs:isDefinedBy dcterms: ;
  rdfs:label "Subject"@en ;
  rdfs:subPropertyOf dc:subject ;
  skos:note "This term is intended to be used with non-literal values as defined in the DCMI Abstract Model (http://dublincore.org/documents/abstract-model/).  As of December 2007, the DCMI Usage Board is seeking a way to express this intention with a formal range declaration."@en ;
.
dcterms:tableOfContents
  rdf:type rdf:Property ;
  dcterms:hasVersion <http://dublincore.org/usage/terms/history/#tableOfContents-003> ;
  dcterms:issued "2000-07-11"^^xsd:date ;
  dcterms:modified "2008-01-14"^^xsd:date ;
  rdfs:comment "A list of subunits of the resource."@en ;
  rdfs:isDefinedBy dcterms: ;
  rdfs:label "Table Of Contents"@en ;
  rdfs:subPropertyOf dc:description ;
  rdfs:subPropertyOf dcterms:description ;
.
dcterms:temporal
  rdf:type rdf:Property ;
  dcterms:hasVersion <http://dublincore.org/usage/terms/history/#temporal-003> ;
  dcterms:issued "2000-07-11"^^xsd:date ;
  dcterms:modified "2008-01-14"^^xsd:date ;
  rdfs:comment "Temporal characteristics of the resource."@en ;
  rdfs:isDefinedBy dcterms: ;
  rdfs:label "Temporal Coverage"@en ;
  rdfs:range dcterms:PeriodOfTime ;
  rdfs:subPropertyOf dc:coverage ;
  rdfs:subPropertyOf dcterms:coverage ;
.
dcterms:title
  rdf:type rdf:Property ;
  dcterms:hasVersion <http://dublincore.org/usage/terms/history/#titleT-002> ;
  dcterms:issued "2008-01-14"^^xsd:date ;
  dcterms:modified "2010-10-11"^^xsd:date ;
  rdfs:comment "A name given to the resource."@en ;
  rdfs:isDefinedBy dcterms: ;
  rdfs:label "Title"@en ;
  rdfs:range rdfs:Literal ;
  rdfs:subPropertyOf dc:title ;
.
dcterms:type
  rdf:type rdf:Property ;
  dcterms:description "Recommended best practice is to use a controlled vocabulary such as the DCMI Type Vocabulary [DCMITYPE]. To describe the file format, physical medium, or dimensions of the resource, use the Format element."@en ;
  dcterms:hasVersion <http://dublincore.org/usage/terms/history/#typeT-001> ;
  dcterms:issued "2008-01-14"^^xsd:date ;
  dcterms:modified "2008-01-14"^^xsd:date ;
  rdfs:comment "The nature or genre of the resource."@en ;
  rdfs:isDefinedBy dcterms: ;
  rdfs:label "Type"@en ;
  rdfs:range rdfs:Class ;
  rdfs:subPropertyOf dc:type ;
.
dcterms:valid
  rdf:type rdf:Property ;
  dcterms:hasVersion <http://dublincore.org/usage/terms/history/#valid-003> ;
  dcterms:issued "2000-07-11"^^xsd:date ;
  dcterms:modified "2008-01-14"^^xsd:date ;
  rdfs:comment "Date (often a range) of validity of a resource."@en ;
  rdfs:isDefinedBy dcterms: ;
  rdfs:label "Date Valid"@en ;
  rdfs:range rdfs:Literal ;
  rdfs:subPropertyOf dc:date ;
  rdfs:subPropertyOf dcterms:date ;
.
gr:BusinessEntity
  rdfs:subClassOf org:FormalOrganization ;
.
<http://spinrdf.org/sp>
  rdfs:comment "An RDF schema to syntactically represent SPARQL queries and update commands as RDF triples." ;
  rdfs:label "SPIN SPARQL Syntax" ;
  owl:versionInfo "1.5.0" ;
.
sp:Aggregation
  rdf:type rdfs:Class ;
  rdfs:comment "Base class of aggregation types (not part of the SPARQL 1.0 standard but supported by ARQ and other engines)." ;
  rdfs:label "Aggregation" ;
  rdfs:subClassOf sp:SystemClass ;
.
sp:AltPath
  rdf:type rdfs:Class ;
  rdfs:comment "An alternative path with the union of sp:path1 and sp:path2." ;
  rdfs:label "Alt path" ;
  rdfs:subClassOf sp:Path ;
.
sp:Asc
  rdf:type rdfs:Class ;
  rdfs:comment "Marker to indicate ascending order." ;
  rdfs:label "Asc" ;
  rdfs:subClassOf sp:OrderByCondition ;
.
sp:Ask
  rdf:type rdfs:Class ;
  rdfs:comment "An ASK query that returns true if the condition in the body is met by at least one result set." ;
  rdfs:label "Ask" ;
  rdfs:subClassOf sp:Query ;
.
sp:Avg
  rdf:type rdfs:Class ;
  rdfs:comment "Represents AVG aggregations." ;
  rdfs:label "AVG" ;
  rdfs:subClassOf sp:Aggregation ;
.
sp:Bind
  rdf:type rdfs:Class ;
  rdfs:comment "A BIND element." ;
  rdfs:label "Bind" ;
  rdfs:subClassOf sp:Element ;
.
sp:Clear
  rdf:type rdfs:Class ;
  rdfs:comment "An Update operation that removes all triples from a specified graph. Must specify the graph using sp:graphIRI, or sp:default, sp:named or sp:all. May have the SILENT flag, encoded using sp:silent." ;
  rdfs:label "Clear" ;
  rdfs:subClassOf sp:Update ;
.
sp:Command
  rdf:type rdfs:Class ;
  rdfs:comment "A shared superclass for sp:Query and sp:Update that can be used to specify that the range of property can be either one." ;
  rdfs:label "Command" ;
  rdfs:subClassOf sp:SystemClass ;
.
sp:Construct
  rdf:type rdfs:Class ;
  rdfs:comment "A CONSTRUCT-type query that can be used to construct new triples from template triples (head) that use variable bindings from the match patterns (body)." ;
  rdfs:label "Construct" ;
  rdfs:subClassOf sp:Query ;
  rdfs:subClassOf spin:Rule ;
.
sp:Count
  rdf:type rdfs:Class ;
  rdfs:comment "Counts the number of times a variable is used. The variable is stored in the variable property. This might be left blank to indicate COUNT(*)." ;
  rdfs:label "COUNT" ;
  rdfs:subClassOf sp:Aggregation ;
.
sp:Create
  rdf:type rdfs:Class ;
  rdfs:comment "An Update operation that creates a new empty graph with a name specified by sp:graphIRI. May have sp:silent set to true." ;
  rdfs:label "Create" ;
  rdfs:subClassOf sp:Update ;
.
sp:Delete
  rdf:type rdfs:Class ;
  rdf:type owl:DeprecatedClass ;
  rdfs:comment """Deprecated - use sp:Modify instead.

Represents a DELETE FROM (part of SPARQL UPDATE language). The graph IRIs are stored in sp:graphIRI. The template patterns to delete are stored in sp:deletePattern. The WHERE clause is represented using sp:where.""" ;
  rdfs:label "Delete" ;
  rdfs:subClassOf sp:Modify ;
.
sp:DeleteData
  rdf:type rdfs:Class ;
  rdfs:comment "An Update operation to delete specific triples. The graph triples are represented using sp:data, which points to an rdf:List of sp:Triples or sp:NamedGraphs." ;
  rdfs:label "Delete data" ;
  rdfs:subClassOf sp:Update ;
.
sp:DeleteWhere
  rdf:type rdfs:Class ;
  rdfs:comment "An Update operation where the triples matched by the WHERE clause (sp:where) will be the triples deleted." ;
  rdfs:label "Delete where" ;
  rdfs:subClassOf sp:Update ;
  rdfs:subClassOf spin:Rule ;
.
sp:Desc
  rdf:type rdfs:Class ;
  rdfs:comment "Marker to indicate descending order." ;
  rdfs:label "Desc" ;
  rdfs:subClassOf sp:OrderByCondition ;
.
sp:Describe
  rdf:type rdfs:Class ;
  rdfs:comment "A DESCRIBE-type Query." ;
  rdfs:label "Describe" ;
  rdfs:subClassOf sp:Query ;
.
sp:Drop
  rdf:type rdfs:Class ;
  rdfs:comment "An Update operation that removes a specified graph from the Graph Store. Must specify the graph using sp:graphIRI, or sp:default, sp:named or sp:all. May have the SILENT flag, encoded using sp:silent." ;
  rdfs:label "Drop" ;
  rdfs:subClassOf sp:Update ;
.
sp:Element
  rdf:type rdfs:Class ;
  rdfs:comment "An abstract base class for all pattern elements." ;
  rdfs:label "Element" ;
  rdfs:subClassOf sp:SystemClass ;
.
sp:ElementGroup
  rdf:type rdfs:Class ;
  rdfs:comment "Abstract base class of group patterns." ;
  rdfs:label "Element group" ;
  rdfs:subClassOf sp:Element ;
.
sp:ElementList
  rdf:type rdfs:Class ;
  rdfs:comment "A list of Elements. This class is never instantiated directly as SPIN will use plain rdf:Lists to store element lists." ;
  rdfs:label "Element list" ;
  rdfs:subClassOf sp:ElementGroup ;
  rdfs:subClassOf rdf:List ;
.
sp:Exists
  rdf:type rdfs:Class ;
  rdfs:comment "An EXISTS element group." ;
  rdfs:label "Exists" ;
  rdfs:subClassOf sp:ElementGroup ;
.
sp:Filter
  rdf:type rdfs:Class ;
  rdfs:comment "A constraint element that evaluates a given expression to true or false." ;
  rdfs:label "Filter" ;
  rdfs:subClassOf sp:Element ;
.
sp:GroupConcat
  rdf:type rdfs:Class ;
  rdfs:comment "Represents GROUP_CONCAT aggregations." ;
  rdfs:label "GROUP_CONCAT" ;
  rdfs:subClassOf sp:Aggregation ;
.
sp:Insert
  rdf:type rdfs:Class ;
  rdf:type owl:DeprecatedClass ;
  rdfs:comment """Deprecated - use sp:Modify instead.

Represents a INSERT INTO (part of SPARQL UPDATE language). The graph IRIs are stored in sp:graphIRI. The template patterns to delete are stored in sp:insertPattern. The WHERE clause is represented using sp:where.""" ;
  rdfs:label "Insert" ;
  rdfs:subClassOf sp:Modify ;
.
sp:InsertData
  rdf:type rdfs:Class ;
  rdfs:comment "An Update operation to insert specific triples. The graph triples are represented using sp:data, which points to an rdf:List of sp:Triples or sp:NamedGraphs." ;
  rdfs:label "Insert data" ;
  rdfs:subClassOf sp:Update ;
.
sp:Let
  rdf:type rdfs:Class ;
  rdf:type owl:DeprecatedClass ;
  rdfs:comment """Deprecated: use sp:Bind instead.

A variable assignment (LET (?<varName> := <expression>)). Not part of the SPARQL 1.0 standard, but (for example) ARQ.""" ;
  rdfs:label "Let" ;
  rdfs:subClassOf sp:Bind ;
.
sp:Load
  rdf:type rdfs:Class ;
  rdfs:comment "A LOAD Update operation. The document to load is specified using sp:document, and the (optional) target graph using sp:into." ;
  rdfs:label "Load" ;
  rdfs:subClassOf sp:Update ;
.
sp:Max
  rdf:type rdfs:Class ;
  rdfs:comment "Represents MAX aggregations." ;
  rdfs:label "MAX" ;
  rdfs:subClassOf sp:Aggregation ;
.
sp:Min
  rdf:type rdfs:Class ;
  rdfs:comment "Represents MIN aggregations." ;
  rdfs:label "MIN" ;
  rdfs:subClassOf sp:Aggregation ;
.
sp:Minus
  rdf:type rdfs:Class ;
  rdfs:comment "A MINUS element group." ;
  rdfs:label "Minus" ;
  rdfs:subClassOf sp:ElementGroup ;
.
sp:ModPath
  rdf:type rdfs:Class ;
  rdfs:comment "A modified path such as rdfs:subClassOf*." ;
  rdfs:label "Mod path" ;
  rdfs:subClassOf sp:Path ;
.
sp:Modify
  rdf:type rdfs:Class ;
  rdfs:comment "Represents a MODIFY (part of SPARQL UPDATE language). The graph IRIs are stored in sp:graphIRI. The template patterns are stored in sp:deletePattern and sp:insertPattern. The WHERE clause is represented using sp:where." ;
  rdfs:label "Modify" ;
  rdfs:subClassOf sp:Update ;
  rdfs:subClassOf spin:Rule ;
.
sp:NamedGraph
  rdf:type rdfs:Class ;
  rdfs:comment "A named Graph element such as GRAPH <uri> {...}." ;
  rdfs:label "Named graph" ;
  rdfs:subClassOf sp:ElementGroup ;
.
sp:NotExists
  rdf:type rdfs:Class ;
  rdfs:comment "A NOT EXISTS element group." ;
  rdfs:label "Not exists" ;
  rdfs:subClassOf sp:ElementGroup ;
.
sp:Optional
  rdf:type rdfs:Class ;
  rdfs:comment "An optional element in a query." ;
  rdfs:label "Optional" ;
  rdfs:subClassOf sp:ElementGroup ;
.
sp:OrderByCondition
  rdf:type rdfs:Class ;
  rdfs:comment "An abstract base class for ascending or descending order conditions. Instances of this class (typically bnodes) must have a value for expression to point to the actual values." ;
  rdfs:label "Order by condition" ;
  rdfs:subClassOf sp:SystemClass ;
.
sp:Path
  rdf:type rdfs:Class ;
  rdfs:comment "The base class of SPARQL property path expressions. Paths are used by sp:TriplePath triple paths." ;
  rdfs:label "Path" ;
  rdfs:subClassOf sp:SystemClass ;
.
sp:Query
  rdf:type rdfs:Class ;
  rdfs:comment "Abstract base class of the various types of supported queries. Common to all types of queries is that they can have a body (\"WHERE clause\")." ;
  rdfs:label "Query" ;
  rdfs:subClassOf sp:Command ;
.
sp:ReverseLinkPath
  rdf:type rdfs:Class ;
  rdfs:label "Reverse link path" ;
  rdfs:subClassOf sp:Path ;
.
sp:ReversePath
  rdf:type rdfs:Class ;
  rdfs:comment "A path with reversed direction." ;
  rdfs:label "Reverse path" ;
  rdfs:subClassOf sp:Path ;
.
sp:Sample
  rdf:type rdfs:Class ;
  rdfs:comment "Represents SAMPLE aggregations" ;
  rdfs:label "SAMPLE" ;
  rdfs:subClassOf sp:Aggregation ;
.
sp:Select
  rdf:type rdfs:Class ;
  rdfs:comment "A SELECT-type query that returns variable bindings as its result." ;
  rdfs:label "Select query" ;
  rdfs:subClassOf sp:Query ;
.
sp:SeqPath
  rdf:type rdfs:Class ;
  rdfs:comment "A sequence of multiple paths." ;
  rdfs:label "Seq path" ;
  rdfs:subClassOf sp:Path ;
.
sp:Service
  rdf:type rdfs:Class ;
  rdfs:comment "A SERVICE call that matches a nested sub-pattern against a SPARQL end point specified by a URI." ;
  rdfs:label "Service" ;
  rdfs:subClassOf sp:ElementGroup ;
.
sp:SubQuery
  rdf:type rdfs:Class ;
  rdfs:comment "A nested SELECT query inside of an element list. The query is stored in sp:query." ;
  rdfs:label "Sub query" ;
  rdfs:subClassOf sp:Element ;
.
sp:Sum
  rdf:type rdfs:Class ;
  rdfs:comment "Represents sum aggregations, e.g. SELECT SUM(?varName)..." ;
  rdfs:label "SUM" ;
  rdfs:subClassOf sp:Aggregation ;
.
sp:SystemClass
  rdf:type rdfs:Class ;
  rdfs:comment "An \"artificial\" root class that groups all SP classes. This makes them look much less overwhelming in UI tools. Typical end users don't need to see those classes anyway." ;
  rdfs:label "SP System class" ;
  rdfs:subClassOf rdfs:Resource ;
.
sp:Triple
  rdf:type rdfs:Class ;
  rdfs:comment "A base class for TriplePattern and TripleTemplate. This basically specifies that subject, predicate and object must be present." ;
  rdfs:label "Triple" ;
  rdfs:subClassOf sp:Tuple ;
.
sp:TriplePath
  rdf:type rdfs:Class ;
  rdfs:comment "Similar to a TriplePattern, but with a path expression as its predicate. For example, this can be used to express transitive sub-class relationships (?subClass rdfs:subClassOf* ?superClass)." ;
  rdfs:label "Triple path" ;
  rdfs:subClassOf sp:Element ;
  rdfs:subClassOf sp:Tuple ;
.
sp:TriplePattern
  rdf:type rdfs:Class ;
  rdfs:comment "A triple pattern used in the body of a query." ;
  rdfs:label "Triple pattern" ;
  rdfs:subClassOf sp:Element ;
  rdfs:subClassOf sp:Triple ;
.
sp:TripleTemplate
  rdf:type rdfs:Class ;
  rdfs:comment "A prototypical triple used as template in the head of a Construct query. May contain variables." ;
  rdfs:label "Triple template" ;
  rdfs:subClassOf sp:Triple ;
.
sp:Tuple
  rdf:type rdfs:Class ;
  rdfs:comment "Abstract base class for things that have subject and object." ;
  rdfs:label "Tuple" ;
  rdfs:subClassOf sp:SystemClass ;
.
sp:Union
  rdf:type rdfs:Class ;
  rdfs:comment "A UNION group." ;
  rdfs:label "Union" ;
  rdfs:subClassOf sp:ElementGroup ;
.
sp:Update
  rdf:type rdfs:Class ;
  rdfs:comment "Abstract base class to group the various SPARQL UPDATE commands." ;
  rdfs:label "Update" ;
  rdfs:subClassOf sp:Command ;
.
sp:Values
  rdf:type rdfs:Class ;
  rdfs:comment "A VALUES element. sp:varNames points to an rdf:List of strings for the variables, sp:values to an rdf:List of rdf:Lists with nodes for each variable, in the order defined by the variables list." ;
  rdfs:label "Values" ;
  rdfs:subClassOf sp:Element ;
.
sp:Variable
  rdf:type rdfs:Class ;
  rdfs:comment "A variable mentioned in a Triple or expression. Variables are often blank nodes with the variable name stored in ts:name. Variables can also be supplied with a URI in which case the system will attempt to reuse the same variable instance across multiple query definitions." ;
  rdfs:label "Variable" ;
  rdfs:subClassOf sp:SystemClass ;
.
sp:all
  rdf:type rdf:Property ;
  rdfs:comment "Used in DROP and CLEAR." ;
  rdfs:label "all" ;
  rdfs:range xsd:boolean ;
  rdfs:subPropertyOf sp:systemProperty ;
.
sp:arg
  rdf:type rdf:Property ;
  rdfs:comment "Abstract superproperty for the enumerated arg1, arg2 etc." ;
  rdfs:label "arg" ;
.
sp:arg1
  rdf:type rdf:Property ;
  rdfs:comment "The first argument of a function call." ;
  rdfs:label "arg1" ;
  rdfs:subPropertyOf sp:arg ;
.
sp:arg2
  rdf:type rdf:Property ;
  rdfs:comment "The second argument of a function call." ;
  rdfs:label "arg2" ;
  rdfs:subPropertyOf sp:arg ;
.
sp:arg3
  rdf:type rdf:Property ;
  rdfs:comment "The third argument of a function call." ;
  rdfs:label "arg3" ;
  rdfs:subPropertyOf sp:arg ;
.
sp:arg4
  rdf:type rdf:Property ;
  rdfs:comment "The forth argument of a function call." ;
  rdfs:label "arg4" ;
  rdfs:subPropertyOf sp:arg ;
.
sp:arg5
  rdf:type rdf:Property ;
  rdfs:comment "The fifth argument of a function call. Further arguments are not common in SPARQL, therefore no sp:arg6, etc are defined here. However, they can be created if needed." ;
  rdfs:label "arg5" ;
  rdfs:subPropertyOf sp:arg ;
.
sp:as
  rdf:type rdf:Property ;
  rdfs:comment "Points to a Variable used in an AS statement such as COUNT aggregates." ;
  rdfs:label "as" ;
  rdfs:range sp:Variable ;
  rdfs:subPropertyOf sp:systemProperty ;
.
sp:bindings
  rdf:type rdf:Property ;
  rdfs:comment "The actual bindings of a sp:Values element." ;
  rdfs:domain sp:Values ;
  rdfs:label "bindings" ;
  rdfs:range rdf:List ;
  rdfs:subPropertyOf sp:systemProperty ;
.
sp:default
  rdf:type rdf:Property ;
  rdfs:comment "Used in DROP and CLEAR." ;
  rdfs:label "default" ;
  rdfs:range xsd:boolean ;
  rdfs:subPropertyOf sp:systemProperty ;
.
sp:deletePattern
  rdf:type rdf:Property ;
  rdfs:comment "Points to a list of sp:TripleTemplates and sp:NamedGraphs in a modify operation." ;
  rdfs:domain sp:Update ;
  rdfs:label "delete pattern" ;
  rdfs:range rdf:List ;
  rdfs:subPropertyOf sp:systemProperty ;
.
sp:distinct
  rdf:type rdf:Property ;
  rdfs:comment "A marker property to indicate that a Select query is of type SELECT DISTINCT." ;
  rdfs:domain sp:Select ;
  rdfs:label "distinct" ;
  rdfs:range xsd:boolean ;
  rdfs:subPropertyOf sp:systemProperty ;
.
sp:document
  rdf:type rdf:Property ;
  rdfs:comment "The URI of the document to load using a LOAD Update operation." ;
  rdfs:domain sp:Load ;
  rdfs:label "document" ;
  rdfs:range rdfs:Resource ;
  rdfs:subPropertyOf sp:systemProperty ;
.
sp:elements
  rdf:type rdf:Property ;
  rdfs:comment "Points to an ElementList, for example in an Optional element." ;
  rdfs:label "elements" ;
  rdfs:range sp:ElementList ;
  rdfs:subPropertyOf sp:systemProperty ;
.
sp:expression
  rdf:type rdf:Property ;
  rdfs:comment "Points to an expression, for example in a Filter or Assignment." ;
  rdfs:label "expression" ;
  rdfs:subPropertyOf sp:systemProperty ;
.
sp:from
  rdf:type rdf:Property ;
  rdfs:comment "Specifies an RDF Dataset used by a Query (FROM syntax in SPARQL). Values of this property must be URI resources." ;
  rdfs:domain sp:Query ;
  rdfs:label "from" ;
  rdfs:range rdfs:Resource ;
  rdfs:subPropertyOf sp:systemProperty ;
.
sp:fromNamed
  rdf:type rdf:Property ;
  rdfs:comment "Specifies a named RDF Dataset used by a Query (FROM NAMED syntax in SPARQL). Values of this property must be URI resources." ;
  rdfs:domain sp:Query ;
  rdfs:label "from named" ;
  rdfs:range rdfs:Resource ;
  rdfs:subPropertyOf sp:systemProperty ;
.
sp:graphIRI
  rdf:type rdf:Property ;
  rdfs:comment "Points to graph names (IRIs) in various sp:Update operations." ;
  rdfs:label "graph IRI" ;
  rdfs:range rdfs:Resource ;
  rdfs:subPropertyOf sp:systemProperty ;
.
sp:graphNameNode
  rdf:type rdf:Property ;
  rdfs:comment "The name (URI or Variable) of a NamedGraph." ;
  rdfs:domain sp:NamedGraph ;
  rdfs:label "graph name node" ;
  rdfs:range rdfs:Resource ;
  rdfs:subPropertyOf sp:systemProperty ;
.
sp:groupBy
  rdf:type rdf:Property ;
  rdfs:comment "Points from a Query to the list of GROUP BY expressions." ;
  rdfs:domain sp:Select ;
  rdfs:label "group by" ;
  rdfs:range rdf:List ;
  rdfs:subPropertyOf sp:systemProperty ;
.
sp:having
  rdf:type rdf:Property ;
  rdfs:comment "Points from a SELECT query to a list of HAVING expressions." ;
  rdfs:domain sp:Select ;
  rdfs:label "having" ;
  rdfs:range rdf:List ;
  rdfs:subPropertyOf sp:systemProperty ;
.
sp:insertPattern
  rdf:type rdf:Property ;
  rdfs:comment "Points to a list of sp:TripleTemplates or sp:NamedGraphs in a modify command." ;
  rdfs:domain sp:Modify ;
  rdfs:label "insert pattern" ;
  rdfs:range rdf:List ;
  rdfs:subPropertyOf sp:systemProperty ;
.
sp:into
  rdf:type rdf:Property ;
  rdfs:comment "The (optional) target of a LOAD Update operation." ;
  rdfs:domain sp:Load ;
  rdfs:label "into" ;
  rdfs:range rdfs:Resource ;
  rdfs:subPropertyOf sp:systemProperty ;
.
sp:limit
  rdf:type rdf:Property ;
  rdfs:comment "The LIMIT solution modifier of a Query." ;
  rdfs:domain sp:Query ;
  rdfs:label "limit" ;
  rdfs:range xsd:long ;
  rdfs:subPropertyOf sp:systemProperty ;
.
sp:modMax
  rdf:type rdf:Property ;
  rdfs:domain sp:ModPath ;
  rdfs:label "mod max" ;
  rdfs:range xsd:integer ;
  rdfs:subPropertyOf sp:systemProperty ;
.
sp:modMin
  rdf:type rdf:Property ;
  rdfs:domain sp:ModPath ;
  rdfs:label "mod min" ;
  rdfs:range xsd:integer ;
  rdfs:subPropertyOf sp:systemProperty ;
.
sp:named
  rdf:type rdf:Property ;
  rdfs:comment "Used in DROP and CLEAR." ;
  rdfs:label "named" ;
  rdfs:range xsd:boolean ;
  rdfs:subPropertyOf sp:systemProperty ;
.
sp:node
  rdf:type rdf:Property ;
  rdfs:domain sp:ReverseLinkPath ;
  rdfs:label "node" ;
  rdfs:subPropertyOf sp:systemProperty ;
.
sp:object
  rdf:type rdf:Property ;
  rdfs:comment "An RDF Node or Variable describing the object of a triple." ;
  rdfs:domain sp:Tuple ;
  rdfs:label "object" ;
  rdfs:subPropertyOf sp:systemProperty ;
.
sp:offset
  rdf:type rdf:Property ;
  rdfs:comment "The OFFSET solution modifier of a Query." ;
  rdfs:domain sp:Query ;
  rdfs:label "offset" ;
  rdfs:range xsd:long ;
  rdfs:subPropertyOf sp:systemProperty ;
.
sp:orderBy
  rdf:type rdf:Property ;
  rdfs:comment "Links a query with an ORDER BY clause where the values are rdf:List containing OrderByConditions or expressions. While the domain of this property is sp:Query, only Describe and Select queries can have values of it." ;
  rdfs:domain sp:Query ;
  rdfs:label "order by" ;
  rdfs:range rdf:List ;
  rdfs:subPropertyOf sp:systemProperty ;
.
sp:path
  rdf:type rdf:Property ;
  rdfs:comment "Points from a TriplePath to its path." ;
  rdfs:domain sp:TriplePath ;
  rdfs:label "path" ;
  rdfs:range sp:Path ;
  rdfs:subPropertyOf sp:systemProperty ;
.
sp:path1
  rdf:type rdf:Property ;
  rdfs:comment "The first child path of a property path. Used by sp:AltPath and sp:SeqPath." ;
  rdfs:label "path1" ;
  rdfs:range sp:Path ;
  rdfs:subPropertyOf sp:systemProperty ;
.
sp:path2
  rdf:type rdf:Property ;
  rdfs:comment "The second child path of a property path. Used by sp:AltPath and sp:SeqPath." ;
  rdfs:label "path2" ;
  rdfs:range sp:Path ;
  rdfs:subPropertyOf sp:systemProperty ;
.
sp:predicate
  rdf:type rdf:Property ;
  rdfs:comment "A resource or Variable describing the predicate of a triple." ;
  rdfs:domain sp:Triple ;
  rdfs:label "predicate" ;
  rdfs:range rdfs:Resource ;
  rdfs:subPropertyOf sp:systemProperty ;
.
sp:query
  rdf:type rdf:Property ;
  rdfs:comment "Links a SubQuery resource with the nested Query." ;
  rdfs:domain sp:SubQuery ;
  rdfs:label "query" ;
  rdfs:range sp:Query ;
  rdfs:subPropertyOf sp:systemProperty ;
.
sp:reduced
  rdf:type rdf:Property ;
  rdfs:comment "A property with true to indicate that a Select query has a REDUCED flag." ;
  rdfs:domain sp:Select ;
  rdfs:label "reduced" ;
  rdfs:range xsd:boolean ;
  rdfs:subPropertyOf sp:systemProperty ;
.
sp:resultNodes
  rdf:type rdf:Property ;
  rdfs:comment "Contains the result nodes (URI resources or Variables) of a Describe query." ;
  rdfs:domain sp:Describe ;
  rdfs:label "result nodes" ;
  rdfs:range rdf:List ;
  rdfs:subPropertyOf sp:systemProperty ;
.
sp:resultVariables
  rdf:type rdf:Property ;
  rdfs:comment "An rdf:List of variables that are returned by a Select query." ;
  rdfs:domain sp:Select ;
  rdfs:label "result variables" ;
  rdfs:range rdf:List ;
  rdfs:subPropertyOf sp:systemProperty ;
.
sp:separator
  rdf:type rdf:Property ;
  rdfs:comment "Stores the separator=\"...\" value of a GROUP_CONCAT (sp:GroupConcat) aggregation." ;
  rdfs:domain sp:GroupConcat ;
  rdfs:label "separator" ;
  rdfs:range xsd:string ;
  rdfs:subPropertyOf sp:systemProperty ;
.
sp:serviceURI
  rdf:type rdf:Property ;
  rdfs:comment "Used by sp:Service to specify the URI of the SPARQL end point to invoke. Must point to a URI node." ;
  rdfs:domain sp:Service ;
  rdfs:label "service URI" ;
  rdfs:range rdfs:Resource ;
  rdfs:subPropertyOf sp:systemProperty ;
.
sp:silent
  rdf:type rdf:Property ;
  rdfs:label "silent" ;
  rdfs:range xsd:boolean ;
  rdfs:subPropertyOf sp:systemProperty ;
.
sp:subPath
  rdf:type rdf:Property ;
  rdfs:comment "The child path of a property path expression. This is used by ReversePath and ModPath." ;
  rdfs:label "sub path" ;
  rdfs:subPropertyOf sp:systemProperty ;
.
sp:subject
  rdf:type rdf:Property ;
  rdfs:comment "A resource or Variable describing the subject of a triple." ;
  rdfs:domain sp:Tuple ;
  rdfs:label "subject" ;
  rdfs:range rdfs:Resource ;
  rdfs:subPropertyOf sp:systemProperty ;
.
sp:systemProperty
  rdf:type rdf:Property ;
  rdfs:comment "An abstract base proprerty that groups together the SP system properties. Users typically don't need to see them anyway." ;
  rdfs:label "SP system property" ;
.
sp:templates
  rdf:type rdf:Property ;
  rdfs:comment "Points to a list of TripleTemplates that form the head of a Construct query." ;
  rdfs:domain sp:Construct ;
  rdfs:label "templates" ;
  rdfs:range rdf:List ;
  rdfs:subPropertyOf sp:systemProperty ;
.
sp:text
  rdf:type rdf:Property ;
  rdfs:comment "Can be attached to sp:Queries to store a textual representation of the query. This can be useful for tools that do not have a complete SPIN Syntax parser available." ;
  rdfs:label "text" ;
  rdfs:range xsd:string ;
  rdfs:subPropertyOf sp:systemProperty ;
.
sp:using
  rdf:type rdf:Property ;
  rdfs:domain sp:Modify ;
  rdfs:label "using" ;
  rdfs:range rdfs:Resource ;
  rdfs:subPropertyOf sp:systemProperty ;
.
sp:usingNamed
  rdf:type rdf:Property ;
  rdfs:domain sp:Modify ;
  rdfs:label "using named" ;
  rdfs:range rdfs:Resource ;
  rdfs:subPropertyOf sp:systemProperty ;
.
sp:values
  rdf:type rdf:Property ;
  rdfs:comment "The VALUES block at the end of a query. The object may just be an untyped blank node, i.e. the sp:Values type triple is optional." ;
  rdfs:domain sp:Query ;
  rdfs:label "values" ;
  rdfs:range sp:Values ;
  rdfs:subPropertyOf sp:systemProperty ;
.
sp:varName
  rdf:type rdf:Property ;
  rdfs:comment "The name of a Variable." ;
  rdfs:domain sp:Variable ;
  rdfs:label "varName" ;
  rdfs:range xsd:string ;
  rdfs:subPropertyOf sp:systemProperty ;
.
sp:varNames
  rdf:type rdf:Property ;
  rdfs:comment "The names of the variables (xsd:strings) of the variables declared for a VALUES element." ;
  rdfs:domain sp:Values ;
  rdfs:label "var names" ;
  rdfs:range rdf:List ;
  rdfs:subPropertyOf sp:systemProperty ;
.
sp:variable
  rdf:type rdf:Property ;
  rdfs:comment "The variable of a Bind element." ;
  rdfs:domain sp:Bind ;
  rdfs:label "variable" ;
  rdfs:range sp:Variable ;
  rdfs:subPropertyOf sp:systemProperty ;
.
sp:where
  rdf:type rdf:Property ;
  rdfs:comment "The WHERE clause of a Query." ;
  rdfs:label "where" ;
  rdfs:range sp:ElementList ;
  rdfs:subPropertyOf sp:systemProperty ;
.
sp:with
  rdf:type rdf:Property ;
  rdfs:domain sp:Modify ;
  rdfs:label "with" ;
  rdfs:range rdfs:Resource ;
  rdfs:subPropertyOf sp:systemProperty ;
.
<http://spinrdf.org/spin>
  rdfs:comment "An RDF Schema that can be used to attach constraints and rules to RDFS classes, and to encapsulate reusable SPARQL queries into functions and templates." ;
  rdfs:label "SPIN Modeling Vocabulary" ;
  owl:versionInfo "1.4" ;
.
spin:AskTemplate
  rdf:type rdfs:Class ;
  spin:constraint [
      rdf:type spl:Attribute ;
      spl:maxCount 1 ;
      spl:minCount 0 ;
      spl:predicate spin:body ;
      spl:valueType sp:Ask ;
      rdfs:comment "The ASK query wrapped by this template." ;
    ] ;
  rdfs:comment "A SPIN template that wraps an ASK query." ;
  rdfs:label "Ask template" ;
  rdfs:subClassOf spin:Template ;
.
spin:AskTemplates
  rdf:type spin:AskTemplate ;
  spin:abstract "true"^^xsd:boolean ;
  rdfs:comment "Suggested abstract base class for all AskTemplates." ;
  rdfs:label "Ask templates" ;
  rdfs:subClassOf spin:Templates ;
.
spin:Column
  rdf:type rdfs:Class ;
  rdfs:comment "Provides metadata about a column in the result set of a (SPARQL) query, for example of the body queries of SPIN templates. Columns can define human-readable labels that serve as column titles, using rdfs:label." ;
  rdfs:label "Column" ;
  rdfs:subClassOf rdfs:Resource ;
.
spin:ConstraintViolation
  rdf:type rdfs:Class ;
  rdfs:comment "An object that can be created by spin:constraints to provide information about a constraint violation." ;
  rdfs:label "Constraint violation" ;
  rdfs:subClassOf rdfs:Resource ;
.
spin:ConstraintViolationLevel
  rdf:type rdfs:Class ;
  rdfs:comment "The type of the supported levels of constraint violations, including spin:Error and spin:Warning." ;
  rdfs:label "Constraint violation level" ;
  rdfs:subClassOf rdfs:Resource ;
.
spin:ConstructTemplate
  rdf:type rdfs:Class ;
  spin:constraint [
      rdf:type spl:Attribute ;
      spl:maxCount 1 ;
      spl:minCount 0 ;
      spl:predicate spin:body ;
      spl:valueType sp:Construct ;
      rdfs:comment "The CONSTRUCT query wrapped by this template." ;
    ] ;
  rdfs:label "Construct template" ;
  rdfs:subClassOf spin:Template ;
.
spin:ConstructTemplates
  rdf:type spin:ConstructTemplate ;
  spin:abstract "true"^^xsd:boolean ;
  rdfs:comment "Suggested abstract base class for all ConstructTemplates." ;
  rdfs:label "Construct templates" ;
  rdfs:subClassOf spin:Templates ;
.
spin:Error
  rdf:type spin:ConstraintViolationLevel ;
  rdfs:comment "Indicates that the associated constraint violation is an error that should be fixed." ;
  rdfs:label "Error" ;
.
spin:Fatal
  rdf:type spin:ConstraintViolationLevel ;
  rdfs:comment "Indicates that the associated constraint violation is a severe error that must be fixed. Constraint checking engines may decide to stop further evaluation once a fatal error has been detected." ;
  rdfs:label "Fatal" ;
.
spin:Function
  rdf:type rdfs:Class ;
  spin:constraint [
      rdf:type spl:Attribute ;
      spl:maxCount 1 ;
      spl:minCount 0 ;
      spl:predicate spin:body ;
      rdfs:comment "the body of the function" ;
    ] ;
  rdfs:comment "Metaclass for functions that can be used in SPARQL expressions (e.g. FILTER or BIND). The function themselves are classes that are instances of this metaclass. Function calls are instances of the function classes, with property values for the arguments." ;
  rdfs:label "Function" ;
  rdfs:subClassOf spin:Module ;
.
spin:Functions
  rdf:type spin:Function ;
  spin:abstract "true"^^xsd:boolean ;
  rdfs:comment "An abstract base class for all defined functions. This class mainly serves as a shared root so that the various instances of the Function metaclass are grouped together." ;
  rdfs:label "Functions" ;
  rdfs:subClassOf spin:Modules ;
.
spin:Info
  rdf:type spin:ConstraintViolationLevel ;
  rdfs:comment "Indicates that the associated constraint violation is a not a problem. This level can be used for diagnostic and debugging purposes." ;
  rdfs:label "Info" ;
.
spin:LibraryOntology
  rdf:type rdfs:Class ;
  rdfs:comment "A marker class that can be attached to base URIs (ontologies) to instruct SPIN engines that this ontology only contains a library of SPIN declarations. Library Ontologies should be ignored by SPIN inference engines even if they have been imported by a domain model. For example, a SPIN version of OWL RL may contain all the OWL RL axioms, attached to owl:Thing, but nothing else. However, when executed, these axioms should not be executed over themselves, because we don't want the system to reason about the SPIN triples to speed up things." ;
  rdfs:label "Library ontology" ;
  rdfs:subClassOf owl:Ontology ;
.
spin:MagicProperties
  rdf:type spin:MagicProperty ;
  spin:abstract "true"^^xsd:boolean ;
  rdfs:comment "An abstract superclass that can be used to group all spin:MagicProperty instances under a single parent class." ;
  rdfs:label "Magic properties" ;
  rdfs:subClassOf spin:Functions ;
  rdfs:subPropertyOf spin:systemProperty ;
.
spin:MagicProperty
  rdf:type rdfs:Class ;
  rdfs:label "Magic property" ;
  rdfs:subClassOf spin:Function ;
  rdfs:subClassOf rdf:Property ;
.
spin:Module
  rdf:type rdfs:Class ;
  rdfs:comment "An abstract building block of a SPARQL system. A Module can take Arguments as input and applies them on an input RDF Graph. The Arguments should be declared as spin:constraints." ;
  rdfs:label "Module" ;
  rdfs:subClassOf rdfs:Class ;
.
spin:Modules
  rdf:type rdfs:Class ;
  spin:constructor [
      rdf:type spl:ConstructDefaultValues ;
    ] ;
  rdfs:comment "An \"artificial\" parent class for all Functions and Templates." ;
  rdfs:label "Modules" ;
  rdfs:subClassOf rdfs:Resource ;
.
spin:Rule
  rdf:type rdfs:Class ;
  rdfs:comment "Groups together the kinds of SPARQL commands that can appear as SPIN rules and constructors: CONSTRUCT, DELETE WHERE and DELETE/INSERT. This class is never to be instantiated directly." ;
  rdfs:label "Rule" ;
  rdfs:subClassOf sp:Command ;
.
spin:RuleProperty
  rdf:type rdfs:Class ;
  rdfs:comment "The metaclass of spin:rule and its subproperties. spin:RuleProperties can have additional metadata attached to them." ;
  rdfs:label "Rule property" ;
  rdfs:subClassOf rdf:Property ;
.
spin:SelectTemplate
  rdf:type rdfs:Class ;
  spin:constraint [
      rdf:type spl:Attribute ;
      spl:maxCount 1 ;
      spl:minCount 0 ;
      spl:predicate spin:body ;
      spl:valueType sp:Select ;
      rdfs:comment "The SELECT query wrapped by this template." ;
    ] ;
  rdfs:comment "A SPIN template that wraps a SELECT query." ;
  rdfs:label "Select template" ;
  rdfs:subClassOf spin:TableDataProvider ;
  rdfs:subClassOf spin:Template ;
.
spin:SelectTemplates
  rdf:type spin:SelectTemplate ;
  spin:abstract "true"^^xsd:boolean ;
  rdfs:comment "Suggested abstract base class for all SelectTemplates." ;
  rdfs:label "Select templates" ;
  rdfs:subClassOf spin:Templates ;
.
spin:TableDataProvider
  rdf:type rdfs:Class ;
  rdfs:comment """An abstraction of objects that can produce tabular data. This serves as a base class of spin:SelectTemplate, because SELECT queries can produce tables with columns for each result variable. However, other types of TableDataProviders are conceivable by other frameworks, and this class may prove as a useful shared foundation.

TableDataProviders can link to definitions of columns via spin:column, and these definitions can inform rendering engines.""" ;
  rdfs:label "Table data provider" ;
  rdfs:subClassOf rdfs:Class ;
.
spin:Template
  rdf:type rdfs:Class ;
  spin:constraint [
      rdf:type spl:Attribute ;
      spl:maxCount 1 ;
      spl:minCount 0 ;
      spl:predicate spin:body ;
      rdfs:comment "the body of the Template" ;
    ] ;
  rdfs:comment "The metaclass of SPIN templates. Templates are classes that are instances of this class. A template represents a reusable SPARQL query or update request that can be parameterized with arguments. Templates can be instantiated in places where normally a SPARQL query or update request is used, in particular as spin:rules and spin:constraints." ;
  rdfs:label "Template" ;
  rdfs:subClassOf spin:Module ;
.
spin:Templates
  rdf:type spin:Template ;
  spin:abstract "true"^^xsd:boolean ;
  rdfs:comment "Suggested abstract base class for all Templates." ;
  rdfs:label "Templates" ;
  rdfs:subClassOf spin:Modules ;
.
spin:UpdateTemplate
  rdf:type rdfs:Class ;
  spin:constraint [
      rdf:type spl:Attribute ;
      spl:maxCount 1 ;
      spl:minCount 0 ;
      spl:predicate spin:body ;
      spl:valueType sp:Update ;
      rdfs:comment "The UPDATE command wrapped by this template." ;
    ] ;
  rdfs:comment "A SPIN template that has an UPDATE command as its body." ;
  rdfs:label "Update template" ;
  rdfs:subClassOf spin:Template ;
.
spin:UpdateTemplates
  rdf:type spin:UpdateTemplate ;
  spin:abstract "true"^^xsd:boolean ;
  rdfs:comment "Suggested abstract base class for all UpdateTemplates." ;
  rdfs:label "Update templates" ;
  rdfs:subClassOf spin:Templates ;
.
spin:Warning
  rdf:type spin:ConstraintViolationLevel ;
  rdfs:comment "Indicates that the associated constraint violation is a problem that may not have to be fixed but may lead to issues in the future." ;
  rdfs:label "Warning" ;
.
spin:_arg1
  rdf:type sp:Variable ;
  sp:varName "arg1" ;
.
spin:_arg2
  rdf:type sp:Variable ;
  sp:varName "arg2" ;
.
spin:_arg3
  rdf:type sp:Variable ;
  sp:varName "arg3" ;
.
spin:_arg4
  rdf:type sp:Variable ;
  sp:varName "arg4" ;
.
spin:_arg5
  rdf:type sp:Variable ;
  sp:varName "arg5" ;
.
spin:_this
  rdf:type sp:Variable ;
  sp:varName "this" ;
  rdfs:comment "A system variable representing the current context instance in a rule or constraint." ;
  rdfs:label "_this" ;
.
spin:abstract
  rdf:type rdf:Property ;
  rdfs:comment "Can be set to true to indicate that this module shall not be instantiated. Abstract modules are only there to organize other modules into hierarchies." ;
  rdfs:domain spin:Module ;
  rdfs:label "abstract" ;
  rdfs:range xsd:boolean ;
  rdfs:subPropertyOf spin:systemProperty ;
.
spin:ask
  rdf:type spin:Function ;
  rdfs:comment """Executes a given ASK query and returns its boolean result. The first argument must point to an sp:Ask or a SPIN template call that has an ASK query as its body. All subsequent argument can come in pairs, with the first one being a variable name and the second its binding.

Example:

    BIND (spin:ask(?query, \"this\", owl:Thing) AS ?result) .

will execute the sp:Ask behind ?query with the variable ?this pre-bound to owl:Thing.""" ;
  rdfs:label "ask" ;
  rdfs:subClassOf spin:Functions ;
.
spin:body
  rdf:type rdf:Property ;
  rdfs:comment "The body of a Function or Template. This points to a Query instance. For Functions, this is limited to either ASK or SELECT type queries. If the body is the ASK function then the return value is xsd:boolean. Otherwise, the SELECT query must have a single return variable. The first binding of this SELECT query will be returned as result of the function call." ;
  rdfs:label "body" ;
  rdfs:range sp:Command ;
  rdfs:subPropertyOf spin:systemProperty ;
.
spin:cachable
  rdf:type rdf:Property ;
  rdfs:comment "Can be set to true to instruct the SPIN engine that it may cache the results of all calls to the associated function. Functions should only be marked as cachable if the same combination of input arguments always returns the same result. Functions that query a graph or other background data that may change over time should not be cached. Caching can significantly improve performance of frequently needed functions." ;
  rdfs:domain spin:Function ;
  rdfs:label "cachable" ;
  rdfs:range xsd:boolean ;
  rdfs:subPropertyOf spin:systemProperty ;
.
spin:column
  rdf:type rdf:Property ;
  rdfs:comment "Can link a TableDataProvider (esp. SelectTemplate) with one or more columns that provide metadata for rendering purposes. Columns can be sorted by their spin:columnIndex (which must align with the ordering of variables in the SELECT query starting with 0). Not all result variables of the underlying query need to have a matching spin:Column." ;
  rdfs:domain spin:TableDataProvider ;
  rdfs:label "column" ;
  rdfs:range spin:Column ;
  rdfs:subPropertyOf spin:systemProperty ;
.
spin:columnIndex
  rdf:type rdf:Property ;
  rdfs:comment "The index of a column (from left to right) starting at 0." ;
  rdfs:domain spin:Column ;
  rdfs:label "column index" ;
  rdfs:range xsd:integer ;
  rdfs:subPropertyOf spin:systemProperty ;
.
spin:columnType
  rdf:type rdf:Property ;
  rdfs:comment "The datatype or resource type of a spin:Column. For example this is useful as metadata to inform a rendering engine that numeric columns (e.g. xsd:float) need to be right-aligned." ;
  rdfs:domain spin:Column ;
  rdfs:label "column type" ;
  rdfs:range rdfs:Class ;
  rdfs:subPropertyOf spin:systemProperty ;
.
spin:columnWidth
  rdf:type rdf:Property ;
  rdfs:comment "The preferred width of the associated Column, for display purposes. Values in pixels (rendering engines may multiply the values depending on resolution)." ;
  rdfs:domain spin:Column ;
  rdfs:label "column width" ;
  rdfs:range xsd:integer ;
  rdfs:subPropertyOf spin:systemProperty ;
.
spin:command
  rdf:type rdf:Property ;
  rdfs:comment "Can be used to link a resource with a SPARQL query or update request (sp:Command)." ;
  rdfs:label "command" ;
  rdfs:range sp:Command ;
.
spin:constraint
  rdf:type rdf:Property ;
  rdfs:comment "Links a class with constraints on its instances. The values of this property are \"axioms\" expressed as CONSTRUCT or ASK queries where the variable ?this refers to the instances of the surrounding class. ASK queries must evaluate to false for each member of this class - returning true means that the instance ?this violates the constraint. CONSTRUCT queries must create instances of spin:ConstraintViolation to provide details on the reason for the violation." ;
  rdfs:domain rdfs:Class ;
  rdfs:label "constraint" ;
  rdfs:subPropertyOf spin:query ;
.
spin:construct
  rdf:type spin:MagicProperty ;
  rdfs:comment """Evaluates a given sp:Construct or SPIN template call (first argument on the left hand side) and binds the resulting triples to the variables on the right hand side.

Example:

    (?query \"this\" owl:Thing) spin:construct (?s ?p ?o)

will execute the sp:Construct ?query using the binding of owl:Thing to ?this. The resulting triples will be bound to ?s, ?p and ?o. If any of ?s ?p ?o are bound, it will only return the matching triples.""" ;
  rdfs:label "construct" ;
  rdfs:subClassOf spin:MagicProperties ;
.
spin:constructViolations
  rdf:type spin:MagicProperty ;
  spin:constraint [
      rdf:type spl:Argument ;
      spl:predicate sp:arg1 ;
      spl:valueType rdfs:Resource ;
      rdfs:comment "The instance to check." ;
    ] ;
  spin:constraint [
      rdf:type spl:Argument ;
      spl:predicate sp:arg2 ;
      spl:valueType rdfs:Class ;
      rdfs:comment "The class that this type is validated against." ;
    ] ;
  rdfs:comment """Takes an instance (?arg1) and a class definition (?arg2) and returns all constraint violations for that instance as triples. This magic property basically runs its own constraint checker for defining meta-constraints, and can also be used to classify instances.

Example:

    CONSTRUCT {
        ?s ?p ?o .
    }
    WHERE {
        (my:Person my:OldPerson) spin:constructViolations (?s ?p ?o) .
    }""" ;
  rdfs:label "construct violations" ;
  rdfs:subClassOf spin:MagicProperties ;
.
spin:constructor
  rdf:type rdf:Property ;
  rdfs:comment "Can be used to attach a \"constructor\" to a class. A constructor is a SPARQL CONSTRUCT query or INSERT/DELETE Update operation that can add initial values to the current instance. At execution time, the variable ?this is bound to the current instance. Tools can call constructors of a class and its superclasses when an instance of a class has been created. Constructors will also be used to initialize resources that have received a new rdf:type triple as a result of spin:rules firing." ;
  rdfs:domain rdfs:Class ;
  rdfs:label "constructor" ;
  rdfs:range spin:Rule ;
  rdfs:subPropertyOf spin:command ;
.
spin:eval
  rdf:type spin:Function ;
  rdfs:comment "Evaluates a given SPIN expression or SELECT or ASK query, and returns its result. The first argument must be the expression in SPIN RDF syntax. All other arguments must come in pairs: first a property name, and then a value. These name/value pairs will be pre-bound variables for the execution of the expression." ;
  rdfs:label "eval" ;
  rdfs:subClassOf spin:Functions ;
.
spin:evalInGraph
  rdf:type spin:Function ;
  rdfs:comment "Evaluates a given SPIN expression or SELECT or ASK query, and returns its result. The first argument must be the expression in SPIN RDF syntax. This RDF representation of this expression is expected to be in the currently active query graph. The second argument is the URI of a graph that the actual query shall be evaluated against. All other arguments must come in pairs: first a property name, and then a value. These name/value pairs will be pre-bound variables for the execution of the expression." ;
  rdfs:label "eval in graph" ;
  rdfs:subClassOf spin:Functions ;
.
spin:fix
  rdf:type rdf:Property ;
  rdfs:comment "Can be used to link a ConstraintViolation with one or more UPDATE Templates that would help fix the violation." ;
  rdfs:domain spin:ConstraintViolation ;
  rdfs:label "fix" ;
  rdfs:range spin:UpdateTemplate ;
  rdfs:subPropertyOf spin:systemProperty ;
.
spin:imports
  rdf:type owl:OntologyProperty ;
  rdfs:comment "Can be used to link an RDF graph (usually the instance of owl:Ontology) with a SPIN library to define constraints. SPIN-aware tools should include the definitions from those libraries for constraint checking. Using such libraries is a simpler alternative than explicitly importing them using owl:imports, because it does not force all the SPIN triples into the RDF model." ;
  rdfs:domain owl:Ontology ;
  rdfs:label "imports" ;
  rdfs:range owl:Ontology ;
  rdfs:subPropertyOf spin:systemProperty ;
.
spin:inverseBody
  rdf:type rdf:Property ;
  rdfs:comment "The inverse body of a magic property - used to provide a more optimized query if there is one result variable (on the right). The values must be instances of Select and must return SELECT ?arg1 etc. The WHERE clause can access the variable ?object to refer to the provided value on the right hand side of the magic property." ;
  rdfs:domain spin:MagicProperty ;
  rdfs:label "inverse body" ;
  rdfs:range sp:Select ;
  rdfs:subPropertyOf spin:systemProperty ;
.
spin:labelTemplate
  rdf:type rdf:Property ;
  rdfs:comment "A template string for displaying instantiations of a module in human-readable form. The template may contain the argument variable names in curly braces to support substitution. For example, \"The number of values of the {?arg1} property.\"" ;
  rdfs:domain spin:Template ;
  rdfs:label "label template" ;
  rdfs:range xsd:string ;
  rdfs:subPropertyOf spin:systemProperty ;
.
spin:nextRuleProperty
  rdf:type rdf:Property ;
  rdfs:comment "Can be used to link two sub-properties of spin:rule (or spin:rule itself) to instruct the SPIN engine to execute one set of rules before another one. The values of the subject property will be executed before those of the object property." ;
  rdfs:domain spin:RuleProperty ;
  rdfs:label "next rule property" ;
  rdfs:range spin:RuleProperty ;
  rdfs:subPropertyOf spin:systemProperty ;
.
spin:private
  rdf:type rdf:Property ;
  rdfs:comment "Can be set to true to indicate that a SPIN function or template is only meant to be used as a helper of other modules, but not directly. Among others, this allows user interfaces to filter out private modules. Furthermore, it tells potential users of this module that they should avoid using this module, as it may not be stable." ;
  rdfs:domain spin:Module ;
  rdfs:label "private" ;
  rdfs:range xsd:boolean ;
  rdfs:subPropertyOf spin:systemProperty ;
.
spin:query
  rdf:type rdf:Property ;
  rdfs:comment "Can be used to point from any resource to a Query." ;
  rdfs:label "query" ;
  rdfs:range sp:Query ;
  rdfs:subPropertyOf spin:command ;
.
spin:returnType
  rdf:type rdf:Property ;
  rdfs:comment "The return type of a Function, e.g. xsd:string." ;
  rdfs:domain spin:Function ;
  rdfs:label "return type" ;
  rdfs:range rdfs:Class ;
  rdfs:subPropertyOf spin:systemProperty ;
.
spin:rule
  rdf:type spin:RuleProperty ;
  rdfs:comment "An inferencing rule attached to a class. Rules are expressed as CONSTRUCT queries or INSERT/DELETE operations where the variable ?this will be bound to the current instance of the class. These inferences can be used to derive new values from existing values at the instance." ;
  rdfs:domain rdfs:Class ;
  rdfs:label "rule" ;
  rdfs:range spin:Rule ;
  rdfs:subPropertyOf spin:command ;
.
spin:rulePropertyMaxIterationCount
  rdf:type rdf:Property ;
  rdfs:comment "Can be attached to spin:rule (or subclasses thereof) to instruct a SPIN rules engine that it shall only execute the rules max times. If no value is specified, then the rules will be executed with no specific limit." ;
  rdfs:domain spin:RuleProperty ;
  rdfs:label "rule property max iteration count" ;
  rdfs:range xsd:integer ;
  rdfs:subPropertyOf spin:systemProperty ;
.
spin:select
  rdf:type spin:MagicProperty ;
  rdfs:comment """Executes a given SELECT or ASK query (or a corresponding SPIN template call) and binds its result rows to the variables specified on the right hand side. May also pre-bind variables for the query execution, using name-value pairs on the left hand side.

Example:

    (?query \"this\" owl:Thing) spin:select (?a ?b)

will execute the sp:Select or sp:Ask that ?query points to and pre-bind ?this with the value of owl:Thing for the execution of the query. The first result variable of the query's result set will be bound to ?a, the second to ?b etc. If the nodes on the right are bound (or constants) then it will match with the values from the result set.

Note that the first argument on the left hand side can be an instance of a SPIN template (but not the template itself). If you need to execute a template, retrieve its spin:body first.""" ;
  rdfs:label "select" ;
  rdfs:subClassOf spin:MagicProperties ;
.
spin:symbol
  rdf:type rdf:Property ;
  rdfs:comment "The symbol of a function, e.g. \"=\" for the eq function." ;
  rdfs:domain spin:Function ;
  rdfs:label "symbol" ;
  rdfs:range xsd:string ;
  rdfs:subPropertyOf spin:systemProperty ;
.
spin:systemProperty
  rdf:type rdf:Property ;
  rdfs:comment "An \"abstract\" base property that groups together those system properties that the user will hardly ever need to see in property trees. This property may be dropped in future versions of this ontology - right now it's mainly here for convenience." ;
  rdfs:label "system property" ;
.
spin:thisUnbound
  rdf:type rdf:Property ;
  rdfs:comment "Can be set to true for SPIN rules and constraints that do not require pre-binding the variable ?this with all members of the associated class. This flag should only be set to true if the WHERE clause is sufficiently strong to only bind instances of the associated class, or its subclasses. In those cases, the engine can greatly improve performance of query execution, because it does not need to add clauses to narrow down the WHERE clause." ;
  rdfs:domain sp:Construct ;
  rdfs:label "this unbound" ;
  rdfs:range xsd:boolean ;
  rdfs:subPropertyOf spin:systemProperty ;
.
spin:update
  rdf:type rdf:Property ;
  rdfs:comment "Can be used to point from any resource to an Update." ;
  rdfs:label "update" ;
  rdfs:range sp:Update ;
  rdfs:subPropertyOf spin:command ;
.
spin:violatesConstraints
  rdf:type spin:Function ;
  spin:returnType xsd:boolean ;
  rdfs:comment "Checks whether a given instance (?arg1) violates any of the constraints defined for a given class (?arg2)." ;
  rdfs:label "violates constraints" ;
  rdfs:subClassOf spin:Functions ;
.
spin:violationDetail
  rdf:type rdf:Property ;
  rdfs:comment "Links a (parent) spin:ConstraintViolation with one or more (child) spin:ConstraintViolations that provide details on the parent violation. This is commonly used in conjunction with spin:constructViolations to indicate that certain violations have triggered the parent violation." ;
  rdfs:domain spin:ConstraintViolation ;
  rdfs:label "violation detail" ;
  rdfs:range spin:ConstraintViolation ;
  rdfs:subPropertyOf spin:systemProperty ;
.
spin:violationLevel
  rdf:type rdf:Property ;
  rdfs:comment "An optional attribute of ConstraintViolations to point at a violation level (such as Error and Warning). Defaults to spin:Error." ;
  rdfs:domain spin:ConstraintViolation ;
  rdfs:label "violation level" ;
  rdfs:range spin:ConstraintViolationLevel ;
  rdfs:subPropertyOf spin:systemProperty ;
.
spin:violationPath
  rdf:type rdf:Property ;
  rdfs:comment "An optional attribute of ConstraintViolations to provide a path expression from the root resource to the value that is invalid. If this is a URI then the path represents the predicate of a subject/predicate combination. Otherwise it should be a blank node of type sp:Path." ;
  rdfs:domain spin:ConstraintViolation ;
  rdfs:label "violation path" ;
  rdfs:range rdfs:Resource ;
  rdfs:subPropertyOf spin:systemProperty ;
.
spin:violationRoot
  rdf:type rdf:Property ;
  rdfs:comment "The root resource of the violation (often ?this in the constraint body)." ;
  rdfs:domain spin:ConstraintViolation ;
  rdfs:label "violation root" ;
  rdfs:range rdfs:Resource ;
  rdfs:subPropertyOf spin:systemProperty ;
.
spin:violationSource
  rdf:type rdf:Property ;
  rdfs:comment "Can be used to link a spin:ConstraintViolation with the query or template call that caused it. This property is typically filled in automatically by the constraint checking engine and does not need to be set manually. However, it can be useful to learn more about the origin of a violation." ;
  rdfs:domain spin:ConstraintViolation ;
  rdfs:label "violation source" ;
  rdfs:range rdfs:Resource ;
  rdfs:subPropertyOf spin:systemProperty ;
.
spin:violationValue
  rdf:type rdf:Property ;
  rdfs:comment "An optional attribute of ConstraintViolations to point at a specific RDF node that caused the violation. Should be accessible from the root via the violationPath." ;
  rdfs:domain spin:ConstraintViolation ;
  rdfs:label "violation value" ;
  rdfs:subPropertyOf spin:systemProperty ;
.
<http://toop.tno.nl/organization>
  rdf:type owl:Ontology ;
  spin:imports <http://topbraid.org/spin/owlrl-all> ;
  spin:imports <http://topbraid.org/spin/rdfsplus> ;
  spin:imports <http://topbraid.org/spin/skosspin> ;
  spin:imports <http://topbraid.org/spin/spinowl> ;
  owl:imports <https://www.w3.org/2009/08/skos-reference/skos.rdf> ;
  owl:versionIRI <http://ec.toop.org/ns/2017/12/organization> ;
  owl:versionInfo "$Date: 2017/12/27 16:31:41$" ;
.
toop:Address_card1
  rdf:type vcard:Address ;
  rdfs:comment "" ;
  rdfs:label "Address card1_"@nl ;
  skos:prefLabel "Address card1" ;
.
toop:CompanyCode
  rdf:type owl:Class ;
  rdfs:comment "The unique official company identifier_ "@en ;
  rdfs:label "Company code_"@en ;
  rdfs:subClassOf adms:Identifier ;
  owl:equivalentClass nhr:KvK-nummer ;
  skos:prefLabel "Company code" ;
.
toop:Foundation
  rdf:type rdfs:Class ;
  rdf:type owl:Class ;
  rdfs:comment "Represents the event that resulted in the foundation of the organization "@en ;
  rdfs:label "Foundation"@en ;
  rdfs:subClassOf org:ChangeEvent ;
  skos:prefLabel "Foundation" ;
.
toop:MyCompCode-Id123456
  rdf:type adms:Identifier ;
  toop:legalStatusEffectiveDate "2017-10-23"^^xsd:date ;
  toop:registrationAuthority toop:NL-KvK ;
  rdfs:comment "My company code, as instance of toop:CompanyCode class, representing the unique official company identifier as laid down by the registration authority_"@en ;
  rdfs:label "MyCompCode-Id123456_"@en ;
  adms:schemeAgency "NL-KvK Kamer van Koophandel"@nl ;
.
toop:MyHasMainSite
  rdf:type toop:Site ;
  rdfs:comment "" ;
  rdfs:label "MyHasMainSite"@nl ;
  skos:prefLabel "MyHasMainSite" ;
.
toop:MyOrganization_0
  rdf:type vcard:Organization ;
  rdfs:comment "The vCard describing the main site of the company or legal person."@en ;
  rdfs:label "Mijn Organization_0"@nl ;
  skos:prefLabel "MyOrganization_0" ;
.
toop:MyOrganization_1
  rdf:type vcard:Organization ;
  rdfs:comment "" ;
  rdfs:label "MijnOrganization 1_"@nl ;
  skos:prefLabel "My Organization 1" ;
.
toop:MyOrganization_2
  rdf:type vcard:Organization ;
  rdfs:comment "" ;
  rdfs:label "Mijn Organization 2_"@nl ;
  skos:prefLabel "My Organization 2" ;
.
toop:MyRegOrg_1
  rdf:type toop:RegisteredOrganization ;
  toop:companyName "My Own Company (legal name)" ;
  toop:hasMainSite toop:MyHasMainSite ;
  rdfs:comment "My organization as instance from the toop:RegisteredOrganization Class" ;
  rdfs:label "Mijn reg org klas 1_"@nl ;
  skos:prefLabel "My organization as instance from the toop:RegisteredOrganization Class" ;
.
toop:NL-KvK
  rdf:type dcterms:Agent ;
  rdfs:comment "De Kamer van Koophandel is de autoriteit voor Nederland voor het registreren van ondermeer bedrijven"@nl ;
  rdfs:comment "The Dutch Chamber of Commerce, acting as registration authority for The Netherlands"@en ;
  rdfs:label "NL-Kv k_"@en ;
.
toop:RegisteredOrganization
  rdf:type rdfs:Class ;
  rdf:type owl:Class ;
  spin:query [
      rdf:type sp:Select ;
      sp:resultVariables (
          [
            sp:varName "s" ;
          ]
          [
            sp:varName "p" ;
          ]
          [
            sp:varName "v" ;
          ]
        ) ;
      sp:where (
          [
            rdf:type sp:Union ;
            sp:elements (
                (
                  [
                    sp:object [
                        sp:varName "o" ;
                      ] ;
                    sp:predicate rdfs:subClassOf ;
                    sp:subject [
                        sp:varName "s" ;
                      ] ;
                  ]
                  [
                    rdf:type sp:Filter ;
                    sp:expression [
                        rdf:type sp:eq ;
                        sp:arg1 [
                            sp:varName "s" ;
                          ] ;
                        sp:arg2 toop:RegisteredOrganization ;
                      ] ;
                  ]
                  [
                    sp:object [
                        sp:varName "p" ;
                      ] ;
                    sp:predicate owl:onProperty ;
                    sp:subject [
                        sp:varName "o" ;
                      ] ;
                  ]
                  [
                    sp:object [
                        sp:varName "v" ;
                      ] ;
                    sp:predicate owl:someValuesFrom ;
                    sp:subject [
                        sp:varName "o" ;
                      ] ;
                  ]
                )
                (
                  [
                    sp:object [
                        sp:varName "o" ;
                      ] ;
                    sp:predicate rdfs:subClassOf ;
                    sp:subject [
                        sp:varName "s" ;
                      ] ;
                  ]
                  [
                    rdf:type sp:Filter ;
                    sp:expression [
                        rdf:type sp:eq ;
                        sp:arg1 [
                            sp:varName "s" ;
                          ] ;
                        sp:arg2 toop:RegisteredOrganization ;
                      ] ;
                  ]
                  [
                    sp:object [
                        sp:varName "p" ;
                      ] ;
                    sp:predicate owl:onProperty ;
                    sp:subject [
                        sp:varName "o" ;
                      ] ;
                  ]
                  [
                    sp:object [
                        sp:varName "v" ;
                      ] ;
                    sp:predicate owl:cardinality ;
                    sp:subject [
                        sp:varName "o" ;
                      ] ;
                  ]
                )
              ) ;
          ]
        ) ;
    ] ;
  rdfs:comment "The TOOP Registered Orginization class represents an organization that has gained legal status by one of the European member states. It is a direct subclass of the rov:RegisteredOrganization class."@en ;
  rdfs:label "Registered organization"@en ;
  rdfs:subClassOf rov:RegisteredOrganization ;
  rdfs:subClassOf [
      rdf:type owl:Restriction ;
      owl:cardinality "1"^^xsd:nonNegativeInteger ;
      owl:onProperty toop:companyName ;
    ] ;
  rdfs:subClassOf [
      rdf:type owl:Restriction ;
      owl:cardinality "1"^^xsd:nonNegativeInteger ;
      owl:onProperty toop:companyType ;
    ] ;
  rdfs:subClassOf [
      rdf:type owl:Restriction ;
      owl:cardinality "1"^^xsd:nonNegativeInteger ;
      owl:onProperty toop:registrationDate ;
    ] ;
  rdfs:subClassOf [
      rdf:type owl:Restriction ;
      owl:onProperty toop:companyCode ;
      owl:someValuesFrom toop:CompanyCode ;
    ] ;
.
toop:Registration
  rdf:type rdfs:Class ;
  rdf:type owl:Class ;
  rdfs:comment "Represents the event that resulted in the registration of the organization."@en ;
  rdfs:label "Registration"@en ;
  rdfs:subClassOf org:ChangeEvent ;
  skos:prefLabel "Registration" ;
.
toop:SSNumber
  rdf:type rdfs:Class ;
  rdfs:comment "The social security number of the company_"@en ;
  rdfs:label "SSNumber"@en ;
  rdfs:subClassOf adms:Identifier ;
  skos:prefLabel "SSNumber" ;
.
toop:Site
  rdf:type rdfs:Class ;
  rdf:type owl:Class ;
  rdfs:comment "Represents an office or other premise at which the organization is located. Many organizations are spread across multiple sites and many sites will host multiple locations."@en ;
  rdfs:label "Site"@en ;
  rdfs:subClassOf org:Site ;
  skos:prefLabel "Site" ;
.
toop:VATNumber
  rdf:type rdfs:Class ;
  rdfs:comment "The value added tax number of the company"@en ;
  rdfs:label "VATNumber"@en ;
  rdfs:subClassOf adms:Identifier ;
  skos:prefLabel "VATNumber" ;
.
toop:activityDeclaration
  rdf:type rdf:Property ;
  rdfs:comment "The description of the main activity of the company as free text description recorded on the registry. This tag should be used to give a description of the company activity in the local language. This should be used in conjunction with the CompanyNaceCode."@en ;
  rdfs:label "activity declaration"@en ;
  rdfs:subPropertyOf dcterms:description ;
  skos:prefLabel "activity declaration" ;
.
toop:companyCode
  rdf:type owl:ObjectProperty ;
  rdfs:comment "The description of the main code of the company as unique identifier recorded in the registry. This tag should be used to give an identifier of the company in the local language. This should be used in conjunction with the CompanyNaceCode"@en ;
  rdfs:label "company code"@en ;
  skos:prefLabel "company code" ;
.
toop:companyNaceCode
  rdf:type owl:ObjectProperty ;
  rdfs:comment "The description of the main activity of the company as free text description recorded on the registry. This tag should be used to give a description of the company activity in the local language. This should be used in conjunction with the CompanyNaceCode"@en ;
  rdfs:label "company NACE code"@en ;
  rdfs:subPropertyOf rov:orgActivity ;
  skos:prefLabel "company NACE code" ;
.
toop:companyName
  rdf:type owl:DatatypeProperty ;
  rdfs:comment "The official current company name as stored in the business register_"@en ;
  rdfs:label "company name" ;
  owl:equivalentProperty rov:legalName ;
.
toop:companyType
  rdf:type rdf:Property ;
  rdf:type owl:ObjectProperty ;
  rdfs:comment "The legal type of the company_"@en ;
  rdfs:label "company type"@en ;
  owl:equivalentProperty rov:orgType ;
  skos:prefLabel "company type" ;
.
toop:foundationDate
  rdf:type owl:DatatypeProperty ;
  rdfs:comment "Represents the date at which the company started. "@en ;
  rdfs:domain toop:Foundation ;
  rdfs:label "foundation date"@en ;
  rdfs:subPropertyOf prov:startedAtTime ;
  skos:prefLabel "foundation date" ;
.
toop:hasMainSite
  rdf:type owl:ObjectProperty ;
  rdfs:comment "The main site of the company or legal person."@en ;
  rdfs:domain toop:RegisteredOrganization ;
  rdfs:label "has main site"@nl ;
  rdfs:range toop:Site ;
  rdfs:subPropertyOf org:hasPrimarySite ;
  skos:prefLabel "has main site" ;
.
toop:legalStatusEffectiveDate
  rdf:type rdf:Property ;
  rdfs:comment "The date at which the current legal status became effective_"@en ;
  rdfs:domain toop:CompanyCode ;
  rdfs:label "legal status effective date"@en ;
  rdfs:subPropertyOf dcterms:issued ;
  skos:prefLabel "legal status effective date" ;
.
toop:registrationAuthority
  rdf:type owl:ObjectProperty ;
  rdfs:comment "The reference to the official register that has registered the company"@en ;
  rdfs:domain toop:CompanyCode ;
  rdfs:label "registration authority"@en ;
  owl:equivalentProperty dcterms:creator ;
  skos:prefLabel "registration authority" ;
.
toop:registrationDate
  rdf:type owl:DatatypeProperty ;
  rdfs:comment "Represents the date at which the company started. "@en ;
  rdfs:domain toop:Registration ;
  rdfs:label "registration date"@en ;
  rdfs:range xsd:date ;
  rdfs:subPropertyOf prov:startedAtTime ;
  skos:prefLabel "registration date" ;
.
toop:registrationNumber
  rdf:type owl:DatatypeProperty ;
  rdfs:comment "The number of the company as recorded on the register. In some jurisdictions, the number on the register may be different from the official company number. This field must be populated in all service requests even when the RegistrationNumber is the same as the CompanyCode "@en ;
  rdfs:label "registration number"@en ;
  owl:equivalentProperty org:identifier ;
  skos:prefLabel "registration number" ;
.
toop:siteAddress
  rdf:type owl:ObjectProperty ;
  rdfs:comment "Represents the postal address and the visiting address of the company. "@en ;
  rdfs:domain toop:Site ;
  rdfs:label "siteAddress"@en ;
  rdfs:range vcard:Organization ;
  rdfs:subPropertyOf org:siteAddress ;
  skos:prefLabel "siteAddress" ;
.
toop:websiteURL
  rdf:type owl:ObjectProperty ;
  rdfs:comment "ISSUE: currently, TBC's local import for vcard seems incomplete - vcard:has* are missing"@en ;
  rdfs:comment "Represents the website URL of the company."@en ;
  rdfs:comment "Represents the website address of the company."@en ;
  rdfs:domain toop:Site ;
  rdfs:label "websiteAddress"@en ;
  rdfs:label "websiteURL"@en ;
  rdfs:range dcterms:URI ;
  rdfs:subPropertyOf org:siteAddress ;
  skos:prefLabel "websiteAddress" ;
  skos:prefLabel "websiteURL" ;
.
rdfs:comment
  rdf:type owl:AnnotationProperty ;
  rdfs:comment ""@en ;
  rdfs:isDefinedBy <http://www.w3.org/ns/prov-o#> ;
.
rdfs:isDefinedBy
  rdf:type owl:AnnotationProperty ;
.
rdfs:label
  rdf:type owl:AnnotationProperty ;
  rdfs:comment ""@en ;
  rdfs:isDefinedBy <http://www.w3.org/ns/prov-o#> ;
.
rdfs:seeAlso
  rdf:type owl:AnnotationProperty ;
  rdfs:comment ""@en ;
.
owl:Thing
  rdf:type owl:Class ;
.
owl:versionInfo
  rdf:type owl:AnnotationProperty ;
.
<http://www.w3.org/2004/02/skos/core>
  dcterms:contributor "Dave Beckett" ;
  dcterms:contributor "Nikki Rogers" ;
  dcterms:contributor "Participants in W3C's Semantic Web Deployment Working Group." ;
  dcterms:creator "Alistair Miles" ;
  dcterms:creator "Sean Bechhofer" ;
  dcterms:description "An RDF vocabulary for describing the basic structure and content of concept schemes such as thesauri, classification schemes, subject heading lists, taxonomies, 'folksonomies', other types of controlled vocabulary, and also concept schemes embedded in glossaries and terminologies."@en ;
  dcterms:title "SKOS Vocabulary"@en ;
  rdfs:label "SKOS Core RDF vocabulary" ;
  rdfs:seeAlso <http://www.w3.org/TR/skos-reference/> ;
  owl:versionInfo "Modified by TopQuadrant to assert three rdfs:subClassOf owl:Thing triples." ;
.
skos:Collection
  rdf:type owl:Class ;
  rdfs:isDefinedBy <http://www.w3.org/2004/02/skos/core> ;
  rdfs:label "Collection"@en ;
  rdfs:subClassOf owl:Thing ;
  owl:disjointWith skos:Concept ;
  owl:disjointWith skos:ConceptScheme ;
  skos:definition "A meaningful collection of concepts."@en ;
  skos:scopeNote "Labelled collections can be used where you would like a set of concepts to be displayed under a 'node label' in the hierarchy."@en ;
.
skos:Concept
  rdf:type owl:Class ;
  rdfs:isDefinedBy <http://www.w3.org/2004/02/skos/core> ;
  rdfs:label "Concept"@en ;
  rdfs:subClassOf owl:Thing ;
  skos:definition "An idea or notion; a unit of thought."@en ;
.
skos:ConceptScheme
  rdf:type owl:Class ;
  rdfs:isDefinedBy <http://www.w3.org/2004/02/skos/core> ;
  rdfs:label "Concept Scheme"@en ;
  rdfs:subClassOf owl:Thing ;
  owl:disjointWith skos:Concept ;
  skos:definition "A set of concepts, optionally including statements about semantic relationships between those concepts."@en ;
  skos:example "Thesauri, classification schemes, subject heading lists, taxonomies, 'folksonomies', and other types of controlled vocabulary are all examples of concept schemes. Concept schemes are also embedded in glossaries and terminologies."@en ;
  skos:scopeNote "A concept scheme may be defined to include concepts from different sources."@en ;
.
skos:OrderedCollection
  rdf:type owl:Class ;
  rdfs:isDefinedBy <http://www.w3.org/2004/02/skos/core> ;
  rdfs:label "Ordered Collection"@en ;
  rdfs:subClassOf skos:Collection ;
  skos:definition "An ordered collection of concepts, where both the grouping and the ordering are meaningful."@en ;
  skos:scopeNote "Ordered collections can be used where you would like a set of concepts to be displayed in a specific order, and optionally under a 'node label'."@en ;
.
skos:altLabel
  rdf:type rdf:Property ;
  rdf:type owl:AnnotationProperty ;
  rdfs:comment "The range of skos:altLabel is the class of RDF plain literals."@en ;
  rdfs:comment "skos:prefLabel, skos:altLabel and skos:hiddenLabel are pairwise disjoint properties."@en ;
  rdfs:isDefinedBy <http://www.w3.org/2004/02/skos/core> ;
  rdfs:label "alternative label"@en ;
  rdfs:subPropertyOf rdfs:label ;
  skos:definition "An alternative lexical label for a resource."@en ;
  skos:example "Acronyms, abbreviations, spelling variants, and irregular plural/singular forms may be included among the alternative labels for a concept. Mis-spelled terms are normally included as hidden labels (see skos:hiddenLabel)."@en ;
.
skos:broadMatch
  rdf:type rdf:Property ;
  rdf:type owl:ObjectProperty ;
  rdfs:isDefinedBy <http://www.w3.org/2004/02/skos/core> ;
  rdfs:label "has broader match"@en ;
  rdfs:subPropertyOf skos:broader ;
  rdfs:subPropertyOf skos:mappingRelation ;
  owl:inverseOf skos:narrowMatch ;
  skos:definition "skos:broadMatch is used to state a hierarchical mapping link between two conceptual resources in different concept schemes."@en ;
.
skos:broader
  rdf:type rdf:Property ;
  rdf:type owl:ObjectProperty ;
  rdfs:comment "Broader concepts are typically rendered as parents in a concept hierarchy (tree)."@en ;
  rdfs:isDefinedBy <http://www.w3.org/2004/02/skos/core> ;
  rdfs:label "has broader"@en ;
  rdfs:subPropertyOf skos:broaderTransitive ;
  owl:inverseOf skos:narrower ;
  skos:definition "Relates a concept to a concept that is more general in meaning."@en ;
  skos:scopeNote "By convention, skos:broader is only used to assert an immediate (i.e. direct) hierarchical link between two conceptual resources."@en ;
.
skos:broaderTransitive
  rdf:type rdf:Property ;
  rdf:type owl:ObjectProperty ;
  rdf:type owl:TransitiveProperty ;
  rdfs:isDefinedBy <http://www.w3.org/2004/02/skos/core> ;
  rdfs:label "has broader transitive"@en ;
  rdfs:subPropertyOf skos:semanticRelation ;
  owl:inverseOf skos:narrowerTransitive ;
  skos:definition "skos:broaderTransitive is a transitive superproperty of skos:broader." ;
  skos:scopeNote "By convention, skos:broaderTransitive is not used to make assertions. Rather, the properties can be used to draw inferences about the transitive closure of the hierarchical relation, which is useful e.g. when implementing a simple query expansion algorithm in a search application."@en ;
.
skos:changeNote
  rdf:type rdf:Property ;
  rdf:type owl:AnnotationProperty ;
  rdfs:isDefinedBy <http://www.w3.org/2004/02/skos/core> ;
  rdfs:label "change note"@en ;
  rdfs:subPropertyOf skos:note ;
  skos:definition "A note about a modification to a concept."@en ;
.
skos:closeMatch
  rdf:type rdf:Property ;
  rdf:type owl:ObjectProperty ;
  rdf:type owl:SymmetricProperty ;
  rdfs:isDefinedBy <http://www.w3.org/2004/02/skos/core> ;
  rdfs:label "has close match"@en ;
  rdfs:subPropertyOf skos:mappingRelation ;
  skos:definition "skos:closeMatch is used to link two concepts that are sufficiently similar that they can be used interchangeably in some information retrieval applications. In order to avoid the possibility of \"compound errors\" when combining mappings across more than two concept schemes, skos:closeMatch is not declared to be a transitive property."@en ;
.
skos:definition
  rdf:type rdf:Property ;
  rdf:type owl:AnnotationProperty ;
  rdfs:isDefinedBy <http://www.w3.org/2004/02/skos/core> ;
  rdfs:label "definition"@en ;
  rdfs:subPropertyOf skos:note ;
  skos:definition "A statement or formal explanation of the meaning of a concept."@en ;
.
skos:editorialNote
  rdf:type rdf:Property ;
  rdf:type owl:AnnotationProperty ;
  rdfs:isDefinedBy <http://www.w3.org/2004/02/skos/core> ;
  rdfs:label "editorial note"@en ;
  rdfs:subPropertyOf skos:note ;
  skos:definition "A note for an editor, translator or maintainer of the vocabulary."@en ;
.
skos:exactMatch
  rdf:type rdf:Property ;
  rdf:type owl:ObjectProperty ;
  rdf:type owl:SymmetricProperty ;
  rdf:type owl:TransitiveProperty ;
  rdfs:comment "skos:exactMatch is disjoint with each of the properties skos:broadMatch and skos:relatedMatch."@en ;
  rdfs:isDefinedBy <http://www.w3.org/2004/02/skos/core> ;
  rdfs:label "has exact match"@en ;
  rdfs:subPropertyOf skos:closeMatch ;
  skos:definition "skos:exactMatch is used to link two concepts, indicating a high degree of confidence that the concepts can be used interchangeably across a wide range of information retrieval applications. skos:exactMatch is a transitive property, and is a sub-property of skos:closeMatch."@en ;
.
skos:example
  rdf:type rdf:Property ;
  rdf:type owl:AnnotationProperty ;
  rdfs:isDefinedBy <http://www.w3.org/2004/02/skos/core> ;
  rdfs:label "example"@en ;
  rdfs:subPropertyOf skos:note ;
  skos:definition "An example of the use of a concept."@en ;
.
skos:hasTopConcept
  rdf:type rdf:Property ;
  rdf:type owl:ObjectProperty ;
  rdfs:domain skos:ConceptScheme ;
  rdfs:isDefinedBy <http://www.w3.org/2004/02/skos/core> ;
  rdfs:label "has top concept"@en ;
  rdfs:range skos:Concept ;
  owl:inverseOf skos:topConceptOf ;
  skos:definition "Relates, by convention, a concept scheme to a concept which is topmost in the broader/narrower concept hierarchies for that scheme, providing an entry point to these hierarchies."@en ;
.
skos:hiddenLabel
  rdf:type rdf:Property ;
  rdf:type owl:AnnotationProperty ;
  rdfs:comment "The range of skos:hiddenLabel is the class of RDF plain literals."@en ;
  rdfs:comment "skos:prefLabel, skos:altLabel and skos:hiddenLabel are pairwise disjoint properties."@en ;
  rdfs:isDefinedBy <http://www.w3.org/2004/02/skos/core> ;
  rdfs:label "hidden label"@en ;
  rdfs:subPropertyOf rdfs:label ;
  skos:definition "A lexical label for a resource that should be hidden when generating visual displays of the resource, but should still be accessible to free text search operations."@en ;
.
skos:historyNote
  rdf:type rdf:Property ;
  rdf:type owl:AnnotationProperty ;
  rdfs:isDefinedBy <http://www.w3.org/2004/02/skos/core> ;
  rdfs:label "history note"@en ;
  rdfs:subPropertyOf skos:note ;
  skos:definition "A note about the past state/use/meaning of a concept."@en ;
.
skos:inScheme
  rdf:type rdf:Property ;
  rdf:type owl:ObjectProperty ;
  rdfs:isDefinedBy <http://www.w3.org/2004/02/skos/core> ;
  rdfs:label "is in scheme"@en ;
  rdfs:range skos:ConceptScheme ;
  skos:definition "Relates a resource (for example a concept) to a concept scheme in which it is included."@en ;
  skos:scopeNote "A concept may be a member of more than one concept scheme."@en ;
.
skos:mappingRelation
  rdf:type rdf:Property ;
  rdf:type owl:ObjectProperty ;
  rdfs:comment "These concept mapping relations mirror semantic relations, and the data model defined below is similar (with the exception of skos:exactMatch) to the data model defined for semantic relations. A distinct vocabulary is provided for concept mapping relations, to provide a convenient way to differentiate links within a concept scheme from links between concept schemes. However, this pattern of usage is not a formal requirement of the SKOS data model, and relies on informal definitions of best practice."@en ;
  rdfs:isDefinedBy <http://www.w3.org/2004/02/skos/core> ;
  rdfs:label "is in mapping relation with"@en ;
  rdfs:subPropertyOf skos:semanticRelation ;
  skos:definition "Relates two concepts coming, by convention, from different schemes, and that have comparable meanings"@en ;
.
skos:member
  rdf:type rdf:Property ;
  rdf:type owl:ObjectProperty ;
  rdfs:domain skos:Collection ;
  rdfs:isDefinedBy <http://www.w3.org/2004/02/skos/core> ;
  rdfs:label "has member"@en ;
  rdfs:range [
      rdf:type owl:Class ;
      owl:unionOf (
          skos:Concept
          skos:Collection
        ) ;
    ] ;
  skos:definition "Relates a collection to one of its members."@en ;
.
skos:memberList
  rdf:type rdf:Property ;
  rdf:type owl:FunctionalProperty ;
  rdf:type owl:ObjectProperty ;
  rdfs:comment """For any resource, every item in the list given as the value of the
      skos:memberList property is also a value of the skos:member property."""@en ;
  rdfs:domain skos:OrderedCollection ;
  rdfs:isDefinedBy <http://www.w3.org/2004/02/skos/core> ;
  rdfs:label "has member list"@en ;
  rdfs:range rdf:List ;
  skos:definition "Relates an ordered collection to the RDF list containing its members."@en ;
.
skos:narrowMatch
  rdf:type rdf:Property ;
  rdf:type owl:ObjectProperty ;
  rdfs:isDefinedBy <http://www.w3.org/2004/02/skos/core> ;
  rdfs:label "has narrower match"@en ;
  rdfs:subPropertyOf skos:mappingRelation ;
  rdfs:subPropertyOf skos:narrower ;
  owl:inverseOf skos:broadMatch ;
  skos:definition "skos:narrowMatch is used to state a hierarchical mapping link between two conceptual resources in different concept schemes."@en ;
.
skos:narrower
  rdf:type rdf:Property ;
  rdf:type owl:ObjectProperty ;
  rdfs:comment "Narrower concepts are typically rendered as children in a concept hierarchy (tree)."@en ;
  rdfs:isDefinedBy <http://www.w3.org/2004/02/skos/core> ;
  rdfs:label "has narrower"@en ;
  rdfs:subPropertyOf skos:narrowerTransitive ;
  owl:inverseOf skos:broader ;
  skos:definition "Relates a concept to a concept that is more specific in meaning."@en ;
  skos:scopeNote "By convention, skos:broader is only used to assert an immediate (i.e. direct) hierarchical link between two conceptual resources."@en ;
.
skos:narrowerTransitive
  rdf:type rdf:Property ;
  rdf:type owl:ObjectProperty ;
  rdf:type owl:TransitiveProperty ;
  rdfs:isDefinedBy <http://www.w3.org/2004/02/skos/core> ;
  rdfs:label "has narrower transitive"@en ;
  rdfs:subPropertyOf skos:semanticRelation ;
  owl:inverseOf skos:broaderTransitive ;
  skos:definition "skos:narrowerTransitive is a transitive superproperty of skos:narrower." ;
  skos:scopeNote "By convention, skos:narrowerTransitive is not used to make assertions. Rather, the properties can be used to draw inferences about the transitive closure of the hierarchical relation, which is useful e.g. when implementing a simple query expansion algorithm in a search application."@en ;
.
skos:notation
  rdf:type rdf:Property ;
  rdf:type owl:DatatypeProperty ;
  rdfs:isDefinedBy <http://www.w3.org/2004/02/skos/core> ;
  rdfs:label "notation"@en ;
  skos:definition "A notation, also known as classification code, is a string of characters such as \"T58.5\" or \"303.4833\" used to uniquely identify a concept within the scope of a given concept scheme."@en ;
  skos:scopeNote "By convention, skos:notation is used with a typed literal in the object position of the triple."@en ;
.
skos:note
  rdf:type rdf:Property ;
  rdf:type owl:AnnotationProperty ;
  rdfs:isDefinedBy <http://www.w3.org/2004/02/skos/core> ;
  rdfs:label "note"@en ;
  skos:definition "A general note, for any purpose."@en ;
  skos:scopeNote "This property may be used directly, or as a super-property for more specific note types."@en ;
.
skos:prefLabel
  rdf:type rdf:Property ;
  rdf:type owl:AnnotationProperty ;
  rdfs:comment "A resource has no more than one value of skos:prefLabel per language tag."@en ;
  rdfs:comment "The range of skos:prefLabel is the class of RDF plain literals."@en ;
  rdfs:comment """skos:prefLabel, skos:altLabel and skos:hiddenLabel are pairwise
      disjoint properties."""@en ;
  rdfs:isDefinedBy <http://www.w3.org/2004/02/skos/core> ;
  rdfs:label "preferred label"@en ;
  rdfs:subPropertyOf rdfs:label ;
  skos:definition "The preferred lexical label for a resource, in a given language."@en ;
.
skos:related
  rdf:type rdf:Property ;
  rdf:type owl:ObjectProperty ;
  rdf:type owl:SymmetricProperty ;
  rdfs:comment "skos:related is disjoint with skos:broaderTransitive"@en ;
  rdfs:isDefinedBy <http://www.w3.org/2004/02/skos/core> ;
  rdfs:label "has related"@en ;
  rdfs:subPropertyOf skos:semanticRelation ;
  skos:definition "Relates a concept to a concept with which there is an associative semantic relationship."@en ;
.
skos:relatedMatch
  rdf:type rdf:Property ;
  rdf:type owl:ObjectProperty ;
  rdf:type owl:SymmetricProperty ;
  rdfs:isDefinedBy <http://www.w3.org/2004/02/skos/core> ;
  rdfs:label "has related match"@en ;
  rdfs:subPropertyOf skos:mappingRelation ;
  rdfs:subPropertyOf skos:related ;
  skos:definition "skos:relatedMatch is used to state an associative mapping link between two conceptual resources in different concept schemes."@en ;
.
skos:scopeNote
  rdf:type rdf:Property ;
  rdf:type owl:AnnotationProperty ;
  rdfs:isDefinedBy <http://www.w3.org/2004/02/skos/core> ;
  rdfs:label "scope note"@en ;
  rdfs:subPropertyOf skos:note ;
  skos:definition "A note that helps to clarify the meaning and/or the use of a concept."@en ;
.
skos:semanticRelation
  rdf:type rdf:Property ;
  rdf:type owl:ObjectProperty ;
  rdfs:domain skos:Concept ;
  rdfs:isDefinedBy <http://www.w3.org/2004/02/skos/core> ;
  rdfs:label "is in semantic relation with"@en ;
  rdfs:range skos:Concept ;
  skos:definition "Links a concept to a concept related by meaning."@en ;
  skos:scopeNote "This property should not be used directly, but as a super-property for all properties denoting a relationship of meaning between concepts."@en ;
.
skos:topConceptOf
  rdf:type rdf:Property ;
  rdf:type owl:ObjectProperty ;
  rdfs:domain skos:Concept ;
  rdfs:isDefinedBy <http://www.w3.org/2004/02/skos/core> ;
  rdfs:label "is top concept in scheme"@en ;
  rdfs:range skos:ConceptScheme ;
  rdfs:subPropertyOf skos:inScheme ;
  owl:inverseOf skos:hasTopConcept ;
  skos:definition "Relates a concept to the concept scheme that it is a top level concept of."@en ;
.
<http://www.w3.org/2006/vcard/ns>
  dc:creator "Brian Suda" ;
  dc:creator "Harry Halpin" ;
  dc:creator "Norman Walsh" ;
  dc:creator "Renato Iannella" ;
  dc:date "2010-01-20" ;
  dc:description "This ontology models and represents vCards in RDF using current best practices." ;
  dc:title "An Ontology for vCards" ;
  rdfs:seeAlso "http://tools.ietf.org/html/rfc2426" ;
  rdfs:seeAlso "http://www.w3.org/Submission/vcard-rdf/" ;
.
vcard:Address
  rdf:type owl:Class ;
  rdfs:comment "Resources that are vCard Addresses" ;
  rdfs:label "vCard Address Class" ;
  rdfs:subClassOf owl:Thing ;
  rdfs:subClassOf [
      rdf:type owl:Restriction ;
      owl:onProperty vcard:country-name ;
      owl:someValuesFrom rdfs:Literal ;
    ] ;
  rdfs:subClassOf [
      rdf:type owl:Restriction ;
      owl:onProperty vcard:extended-address ;
      owl:someValuesFrom rdfs:Literal ;
    ] ;
  rdfs:subClassOf [
      rdf:type owl:Restriction ;
      owl:onProperty vcard:locality ;
      owl:someValuesFrom rdfs:Literal ;
    ] ;
  rdfs:subClassOf [
      rdf:type owl:Restriction ;
      owl:onProperty vcard:post-office-box ;
      owl:someValuesFrom rdfs:Literal ;
    ] ;
  rdfs:subClassOf [
      rdf:type owl:Restriction ;
      owl:onProperty vcard:postal-code ;
      owl:someValuesFrom rdfs:Literal ;
    ] ;
  rdfs:subClassOf [
      rdf:type owl:Restriction ;
      owl:onProperty vcard:region ;
      owl:someValuesFrom rdfs:Literal ;
    ] ;
  rdfs:subClassOf [
      rdf:type owl:Restriction ;
      owl:onProperty vcard:street-address ;
      owl:someValuesFrom rdfs:Literal ;
    ] ;
  owl:disjointWith vcard:Email ;
  owl:disjointWith vcard:Label ;
  owl:disjointWith vcard:Tel ;
.
vcard:BBS
  rdf:type owl:Class ;
  rdfs:comment "Bulletin Board System Communications" ;
  rdfs:label "Bulletin Board System" ;
  rdfs:subClassOf vcard:Tel ;
.
vcard:Car
  rdf:type owl:Class ;
  rdfs:comment "Car Telephone" ;
  rdfs:label "Car Phone" ;
  rdfs:subClassOf vcard:Tel ;
.
vcard:Cell
  rdf:type owl:Class ;
  rdfs:comment "Cellular or Mobile Telephone" ;
  rdfs:label "Cellular Telephone" ;
  rdfs:subClassOf vcard:Tel ;
.
vcard:Dom
  rdf:type owl:Class ;
  rdfs:comment "Information related to a Domestic Address or Label" ;
  rdfs:label "Domestic" ;
  rdfs:subClassOf owl:Thing ;
  rdfs:subClassOf [
      rdf:type owl:Class ;
      owl:unionOf (
          vcard:Address
          vcard:Label
        ) ;
    ] ;
.
vcard:Email
  rdf:type owl:Class ;
  rdfs:comment "Resources that are vCard Email Addresses" ;
  rdfs:label "Email" ;
  rdfs:subClassOf owl:Thing ;
  owl:disjointWith vcard:Label ;
  owl:disjointWith vcard:Tel ;
.
vcard:Fax
  rdf:type owl:Class ;
  rdfs:comment "Fax Communications" ;
  rdfs:label "Fax" ;
  rdfs:subClassOf vcard:Tel ;
.
vcard:Home
  rdf:type owl:Class ;
  rdfs:comment "Information related to a Home Address, Label, or Telephone" ;
  rdfs:label "Home" ;
  rdfs:subClassOf owl:Thing ;
  rdfs:subClassOf [
      rdf:type owl:Class ;
      owl:unionOf (
          vcard:Address
          vcard:Label
          vcard:Tel
        ) ;
    ] ;
.
vcard:ISDN
  rdf:type owl:Class ;
  rdfs:comment "ISDN Communications" ;
  rdfs:label "ISDN" ;
  rdfs:subClassOf vcard:Tel ;
.
vcard:Internet
  rdf:type owl:Class ;
  rdfs:comment "Internet Email" ;
  rdfs:label "Internet" ;
  rdfs:subClassOf vcard:Email ;
.
vcard:Intl
  rdf:type owl:Class ;
  rdfs:comment "Information related to an International Address or Label" ;
  rdfs:label "International" ;
  rdfs:subClassOf owl:Thing ;
  rdfs:subClassOf [
      rdf:type owl:Class ;
      owl:unionOf (
          vcard:Address
          vcard:Label
        ) ;
    ] ;
.
vcard:Label
  rdf:type owl:Class ;
  rdfs:comment "Resources that are vCard Labels" ;
  rdfs:label "Label" ;
  rdfs:subClassOf owl:Thing ;
  owl:disjointWith vcard:Tel ;
.
vcard:Location
  rdf:type owl:Class ;
  rdfs:comment "Resources that are vCard geographic locations" ;
  rdfs:label "vCard Geographic Location Class" ;
  rdfs:subClassOf owl:Thing ;
  rdfs:subClassOf [
      rdf:type owl:Restriction ;
      owl:onProperty vcard:latitude ;
      owl:someValuesFrom rdfs:Literal ;
    ] ;
  rdfs:subClassOf [
      rdf:type owl:Restriction ;
      owl:onProperty vcard:longitude ;
      owl:someValuesFrom rdfs:Literal ;
    ] ;
.
vcard:Modem
  rdf:type owl:Class ;
  rdfs:comment "Modem Communications" ;
  rdfs:label "Modem" ;
  rdfs:subClassOf vcard:Tel ;
.
vcard:Msg
  rdf:type owl:Class ;
  rdfs:comment "Voice Message Communications" ;
  rdfs:label "Voice Messenger" ;
  rdfs:subClassOf vcard:Tel ;
.
vcard:Name
  rdf:type owl:Class ;
  rdfs:comment "Resources that are vCard personal names" ;
  rdfs:label "vCard Name Class" ;
  rdfs:subClassOf owl:Thing ;
  rdfs:subClassOf [
      rdf:type owl:Restriction ;
      owl:onProperty vcard:additional-name ;
      owl:someValuesFrom rdfs:Literal ;
    ] ;
  rdfs:subClassOf [
      rdf:type owl:Restriction ;
      owl:onProperty vcard:family-name ;
      owl:someValuesFrom rdfs:Literal ;
    ] ;
  rdfs:subClassOf [
      rdf:type owl:Restriction ;
      owl:onProperty vcard:given-name ;
      owl:someValuesFrom rdfs:Literal ;
    ] ;
  rdfs:subClassOf [
      rdf:type owl:Restriction ;
      owl:onProperty vcard:honorific-prefix ;
      owl:someValuesFrom rdfs:Literal ;
    ] ;
  rdfs:subClassOf [
      rdf:type owl:Restriction ;
      owl:onProperty vcard:honorific-suffix ;
      owl:someValuesFrom rdfs:Literal ;
    ] ;
.
vcard:Organization
  rdf:type owl:Class ;
  rdfs:comment "Resources that are vCard organizations" ;
  rdfs:label "vCard Organization Class" ;
  rdfs:subClassOf owl:Thing ;
  rdfs:subClassOf [
      rdf:type owl:Restriction ;
      owl:onProperty vcard:organization-name ;
      owl:someValuesFrom rdfs:Literal ;
    ] ;
  rdfs:subClassOf [
      rdf:type owl:Restriction ;
      owl:onProperty vcard:organization-unit ;
      owl:someValuesFrom rdfs:Literal ;
    ] ;
.
vcard:PCS
  rdf:type owl:Class ;
  rdfs:comment "Personal Communications Service" ;
  rdfs:label "Personal Communications Service" ;
  rdfs:subClassOf vcard:Tel ;
.
vcard:Pager
  rdf:type owl:Class ;
  rdfs:comment "Pager Communications" ;
  rdfs:label "Pager Device" ;
  rdfs:subClassOf vcard:Tel ;
.
vcard:Parcel
  rdf:type owl:Class ;
  rdfs:comment "Information related to a Parcel Address or Label" ;
  rdfs:label "Parcel" ;
  rdfs:subClassOf owl:Thing ;
  rdfs:subClassOf [
      rdf:type owl:Class ;
      owl:unionOf (
          vcard:Address
          vcard:Label
        ) ;
    ] ;
.
vcard:Postal
  rdf:type owl:Class ;
  rdfs:comment "Information related to a Postal Address or Label" ;
  rdfs:label "Postal" ;
  rdfs:subClassOf owl:Thing ;
  rdfs:subClassOf [
      rdf:type owl:Class ;
      owl:unionOf (
          vcard:Address
          vcard:Label
        ) ;
    ] ;
.
vcard:Pref
  rdf:type owl:Class ;
  rdfs:comment "Information related to a Preferred Address, Email, Label, or Telephone" ;
  rdfs:label "Preferred" ;
  rdfs:subClassOf owl:Thing ;
  rdfs:subClassOf [
      rdf:type owl:Class ;
      owl:unionOf (
          vcard:Address
          vcard:Email
          vcard:Label
          vcard:Tel
        ) ;
    ] ;
.
vcard:Tel
  rdf:type owl:Class ;
  rdfs:comment "Resources that are vCard Telephony communication mechanisms" ;
  rdfs:comment "Telephone" ;
  rdfs:subClassOf owl:Thing ;
.
vcard:VCard
  rdf:type owl:Class ;
  rdfs:comment "Resources that are vCards and the URIs that denote these vCards can also be the same URIs that denote people/orgs" ;
  rdfs:label "vCard Class" ;
  rdfs:subClassOf owl:Thing ;
.
vcard:Video
  rdf:type owl:Class ;
  rdfs:comment "Video Communications" ;
  rdfs:label "Video" ;
  rdfs:subClassOf vcard:Tel ;
.
vcard:Voice
  rdf:type owl:Class ;
  rdfs:comment "Voice Communications" ;
  rdfs:label "Voice" ;
  rdfs:subClassOf vcard:Tel ;
.
vcard:Work
  rdf:type owl:Class ;
  rdfs:comment "Information related to a Work Address, Label, or Telephone" ;
  rdfs:label "Work" ;
  rdfs:subClassOf owl:Thing ;
  rdfs:subClassOf [
      rdf:type owl:Class ;
      owl:unionOf (
          vcard:Address
          vcard:Email
          vcard:Label
          vcard:Tel
        ) ;
    ] ;
.
vcard:X400
  rdf:type owl:Class ;
  rdfs:comment "X.400 Email" ;
  rdfs:label "X.400" ;
  rdfs:subClassOf vcard:Email ;
.
vcard:additional-name
  rdf:type owl:DatatypeProperty ;
  rdfs:comment "An additional part of a person's name" ;
  rdfs:domain vcard:Name ;
  rdfs:label "additional name" ;
.
vcard:adr
  rdf:type owl:ObjectProperty ;
  rdfs:comment "A postal or street address of a person" ;
  rdfs:domain vcard:VCard ;
  rdfs:label "address" ;
  rdfs:range vcard:Address ;
.
vcard:agent
  rdf:type owl:ObjectProperty ;
  rdfs:comment "A person that acts as one's agent" ;
  rdfs:domain vcard:VCard ;
  rdfs:label "agent" ;
  rdfs:range vcard:VCard ;
.
vcard:bday
  rdf:type owl:DatatypeProperty ;
  rdfs:comment "The birthday of a person" ;
  rdfs:domain vcard:VCard ;
  rdfs:label "birthday" ;
  rdfs:range [
      rdf:type rdfs:Datatype ;
      owl:unionOf (
          xsd:date
          xsd:dateTime
        ) ;
    ] ;
.
vcard:category
  rdf:type owl:DatatypeProperty ;
  rdfs:comment "A category of a vCard" ;
  rdfs:domain vcard:VCard ;
  rdfs:label "category" ;
.
vcard:class
  rdf:type owl:DatatypeProperty ;
  rdfs:comment "A class (e.g., public, private, etc.) of a vCard" ;
  rdfs:domain vcard:VCard ;
  rdfs:label "class" ;
.
vcard:country-name
  rdf:type owl:DatatypeProperty ;
  rdfs:comment "The country of a postal address" ;
  rdfs:domain vcard:Address ;
  rdfs:label "country" ;
.
vcard:email
  rdf:type owl:ObjectProperty ;
  rdfs:comment "An email address" ;
  rdfs:domain vcard:VCard ;
  rdfs:label "email" ;
.
vcard:extended-address
  rdf:type owl:DatatypeProperty ;
  rdfs:comment "The extended address of a postal address" ;
  rdfs:domain vcard:Address ;
  rdfs:label "extended" ;
.
vcard:family-name
  rdf:type owl:DatatypeProperty ;
  rdfs:comment "A family name part of a person's name" ;
  rdfs:domain vcard:Name ;
  rdfs:label "family name" ;
.
vcard:fn
  rdf:type owl:DatatypeProperty ;
  rdfs:comment "A formatted name of a person" ;
  rdfs:domain vcard:VCard ;
  rdfs:label "formatted name" ;
.
vcard:geo
  rdf:type owl:ObjectProperty ;
  rdfs:comment "A geographic location associated with a person" ;
  rdfs:domain vcard:VCard ;
  rdfs:label "geographic location" ;
  rdfs:range vcard:Location ;
.
vcard:given-name
  rdf:type owl:DatatypeProperty ;
  rdfs:comment "A given name part of a person's name" ;
  rdfs:domain vcard:Name ;
  rdfs:label "given name" ;
.
vcard:honorific-prefix
  rdf:type owl:DatatypeProperty ;
  rdfs:comment "An honorific prefix part of a person's name" ;
  rdfs:domain vcard:Name ;
  rdfs:label "honorific prefix" ;
.
vcard:honorific-suffix
  rdf:type owl:DatatypeProperty ;
  rdfs:comment "An honorific suffix part of a person's name" ;
  rdfs:domain vcard:Name ;
  rdfs:label "honorific suffix" ;
.
vcard:key
  rdf:type owl:ObjectProperty ;
  rdfs:comment "A key (e.g, PKI key) of a person" ;
  rdfs:domain vcard:VCard ;
  rdfs:label "key" ;
.
vcard:label
  rdf:type owl:DatatypeProperty ;
  rdfs:comment "The formatted version of a postal address (a string with embedded line breaks, punctuation, etc.)" ;
  rdfs:domain vcard:Address ;
  rdfs:label "address label" ;
.
vcard:latitude
  rdf:type owl:DatatypeProperty ;
  rdfs:comment "The latitude of the location of the vCard object" ;
  rdfs:domain vcard:Location ;
  rdfs:label "geographic latitude" ;
  rdfs:range xsd:float ;
.
vcard:locality
  rdf:type owl:DatatypeProperty ;
  rdfs:comment "The locality (e.g., city) of a postal address" ;
  rdfs:domain vcard:Address ;
  rdfs:label "locality" ;
.
vcard:logo
  rdf:type owl:ObjectProperty ;
  rdfs:comment "A logo associated with a person or their organization" ;
  rdfs:domain vcard:VCard ;
  rdfs:label "logo" ;
.
vcard:longitude
  rdf:type owl:DatatypeProperty ;
  rdfs:comment "The longitude of the location of the vCard object" ;
  rdfs:domain vcard:Location ;
  rdfs:label "geographic longitude" ;
  rdfs:range xsd:float ;
.
vcard:mailer
  rdf:type owl:DatatypeProperty ;
  rdfs:comment "A mailer associated with a vCard" ;
  rdfs:domain vcard:VCard ;
  rdfs:label "mailer" ;
.
vcard:n
  rdf:type owl:ObjectProperty ;
  rdfs:comment "The components of the name of a person" ;
  rdfs:domain vcard:VCard ;
  rdfs:label "name" ;
  rdfs:range vcard:Name ;
.
vcard:nickname
  rdf:type owl:DatatypeProperty ;
  rdfs:comment "The nickname of a person" ;
  rdfs:domain vcard:VCard ;
  rdfs:label "nickname" ;
.
vcard:note
  rdf:type owl:DatatypeProperty ;
  rdfs:comment "Notes about a person on a vCard" ;
  rdfs:domain vcard:VCard ;
  rdfs:label "notes" ;
.
vcard:org
  rdf:type owl:ObjectProperty ;
  rdfs:comment "An organization associated with a person" ;
  rdfs:domain vcard:VCard ;
  rdfs:label "organization" ;
  rdfs:range vcard:Organization ;
.
vcard:organization-name
  rdf:type owl:DatatypeProperty ;
  rdfs:comment "The name of an organization" ;
  rdfs:domain vcard:Organization ;
  rdfs:label "name" ;
.
vcard:organization-unit
  rdf:type owl:DatatypeProperty ;
  rdfs:comment "The name of a unit within an organization" ;
  rdfs:domain vcard:Organization ;
  rdfs:label "unit" ;
.
vcard:photo
  rdf:type owl:ObjectProperty ;
  rdfs:comment "A photograph of a person" ;
  rdfs:domain vcard:VCard ;
  rdfs:label "photo" ;
.
vcard:post-office-box
  rdf:type owl:DatatypeProperty ;
  rdfs:comment "The post office box of a postal address" ;
  rdfs:domain vcard:Address ;
  rdfs:label "P.O. Box" ;
.
vcard:postal-code
  rdf:type owl:DatatypeProperty ;
  rdfs:comment "The postal code (e.g., U.S. ZIP code) of a postal address" ;
  rdfs:domain vcard:Address ;
  rdfs:label "postal code" ;
.
vcard:prodid
  rdf:type owl:DatatypeProperty ;
  rdfs:comment "The Identifier for the product that created the vCard object" ;
  rdfs:domain vcard:VCard ;
  rdfs:label "prodid" ;
.
vcard:region
  rdf:type owl:DatatypeProperty ;
  rdfs:comment "The region (e.g., state or province) of a postal address" ;
  rdfs:domain vcard:Address ;
  rdfs:label "region" ;
.
vcard:rev
  rdf:type owl:DatatypeProperty ;
  rdfs:comment "The timestamp of a revision of a vCard" ;
  rdfs:domain vcard:VCard ;
  rdfs:label "revision" ;
  rdfs:range [
      rdf:type rdfs:Datatype ;
      owl:unionOf (
          xsd:date
          xsd:dateTime
        ) ;
    ] ;
.
vcard:role
  rdf:type owl:DatatypeProperty ;
  rdfs:comment "A role a person plays within an organization" ;
  rdfs:domain vcard:VCard ;
  rdfs:label "role" ;
.
vcard:sort-string
  rdf:type owl:DatatypeProperty ;
  rdfs:comment "A version of a person's name suitable for collation" ;
  rdfs:domain vcard:VCard ;
  rdfs:label "sort" ;
.
vcard:sound
  rdf:type owl:ObjectProperty ;
  rdfs:comment "A sound (e.g., a greeting or pronounciation) of a person" ;
  rdfs:domain vcard:VCard ;
  rdfs:label "sound" ;
.
vcard:street-address
  rdf:type owl:DatatypeProperty ;
  rdfs:comment "The street address of a postal address" ;
  rdfs:domain vcard:Address ;
  rdfs:label "street" ;
.
vcard:tel
  rdf:type owl:ObjectProperty ;
  rdfs:comment "A telephone number of a person" ;
  rdfs:domain vcard:VCard ;
  rdfs:label "phone" ;
.
vcard:title
  rdf:type owl:DatatypeProperty ;
  rdfs:comment "A person's title" ;
  rdfs:domain vcard:VCard ;
  rdfs:label "title" ;
.
vcard:tz
  rdf:type owl:DatatypeProperty ;
  rdfs:comment "A timezone associated with a person" ;
  rdfs:domain vcard:VCard ;
  rdfs:label "timezone" ;
.
vcard:uid
  rdf:type owl:DatatypeProperty ;
  rdfs:comment "A UID of a person's vCard" ;
  rdfs:domain vcard:VCard ;
  rdfs:label "uid" ;
.
vcard:url
  rdf:type owl:ObjectProperty ;
  rdfs:comment "A URL associated with a person" ;
  rdfs:domain vcard:VCard ;
  rdfs:label "url" ;
.
<http://www.w3.org/TR/2013/NOTE-vocab-adms-20130528/adms20130520.png>
  rdfs:label "Asset Description Metadata Schema (ADMS) UML Class Diagram" ;
.
<http://www.w3.org/TR/2013/NOTE-vocab-regorg-20130528/>
  dcterms:title "Registered Organization Vocabulary" ;
.
<http://www.w3.org/TR/2013/NOTE-vocab-regorg-20130528/regorg20130508.png>
  rdfs:label "Registered Organization vocabulary UML Class Diagram" ;
.
<http://www.w3.org/TR/vocab-adms/>
  dcterms:title "Asset Description Metadata Schema (ADMS)" ;
.
<http://www.w3.org/ns/adms>
  rdf:type <http://labs.mondeca.com/vocab/voaf#Vocabulary> ;
  dcterms:abstract "ADMS is a profile of DCAT, used to describe semantic assets (or just 'Assets'), defined as highly reusable metadata (e.g. xml schemata, generic data models) and reference data (e.g. code lists, taxonomies, dictionaries, vocabularies) that are used for eGovernment system development." ;
  dcterms:creator [
      schema:affiliation [
          foaf:homepage <http://ies.jrc.ec.europa.eu/DE> ;
          foaf:name "European Commission, Joint Research Centre " ;
        ] ;
      rdfs:seeAlso <http://andrea-perego.name/foaf/#me> ;
      foaf:homepage <http://andrea-perego.name/> ;
      foaf:name "Andrea Perego" ;
    ] ;
  dcterms:creator [
      schema:affiliation [
          foaf:homepage <http://ies.jrc.ec.europa.eu/DE> ;
          foaf:name "European Commission, Joint Research Centre " ;
        ] ;
      rdfs:seeAlso <http://andrea-perego.name/foaf/#me> ;
      foaf:homepage <http://andrea-perego.name/> ;
      foaf:name "Andrea Perego" ;
    ] ;
  dcterms:creator [
      schema:affiliation [
          foaf:homepage <http://www.w3.org/> ;
          foaf:name "W3C/ERCIM" ;
        ] ;
      rdfs:seeAlso <http://philarcher.org/foaf.rdf#me> ;
      foaf:homepage <http://www.w3.org/People/all#phila> ;
      foaf:name "Phil Archer" ;
    ] ;
  dcterms:creator [
      schema:affiliation [
          foaf:homepage <http://www.w3.org/> ;
          foaf:name "W3C/ERCIM" ;
        ] ;
      rdfs:seeAlso <http://philarcher.org/foaf.rdf#me> ;
      foaf:homepage <http://www.w3.org/People/all#phila> ;
      foaf:name "Phil Archer" ;
    ] ;
  dcterms:creator [
      rdfs:seeAlso <http://makxdekkers.com/makxdekkers.rdf#me> ;
      foaf:homepage <http://makxdekkers.com/> ;
      foaf:name "Makx Dekkers" ;
    ] ;
  dcterms:creator [
      rdfs:seeAlso <http://makxdekkers.com/makxdekkers.rdf#me> ;
      foaf:homepage <http://makxdekkers.com/> ;
      foaf:name "Makx Dekkers" ;
    ] ;
  dcterms:description """This is the RDF encoding of the 
      <a xmlns=\"http://www.w3.org/ns/adms#\" href=\"http://www.w3.org/TR/vocab-adms/\">Asset Description Metadata Schema</a>, 
      originally developed under the European Union's <a xmlns=\"http://www.w3.org/ns/adms#\" href=\"http://ec.europa.eu/isa/\">ISA Programme</a> 
      and further developed by the W3C <a xmlns=\"http://www.w3.org/ns/adms#\" href=\"http://www.w3.org/2011/gld/\">Government Linked Data Working Group</a>. It re-uses terms 
      from several other vocabularies, notably Dublin Core, with elements of SKOS, FOAF 
      and more.
    """^^rdf:XMLLiteral ;
  dcterms:modified "2013-05-24"^^xsd:date ;
  dcterms:modified "2013-12-21"^^xsd:date ;
  dcterms:modified "2015-07-22"^^xsd:date ;
  vann:preferredNamespacePrefix "adms" ;
  vann:preferredNamespaceUri "http://www.w3.org/ns/adms#" ;
  voaf:specializes <http://www.w3.org/dcat> ;
  rdfs:comment "This file specifies the set of RDF classes and properties used in ADMS"@en ;
  rdfs:label "Asset Description Metadata Schema (ADMS)"@en ;
  owl:versionInfo "21 December 2013 - with correction to URI of the schema cf. using the namespace"@en ;
  wdrs:describedby <http://www.w3.org/TR/vocab-adms/> ;
  foaf:depiction <http://www.w3.org/TR/2013/NOTE-vocab-adms-20130528/adms20130520.png> ;
  foaf:maker [
      foaf:name "Government Linked Data WG, based on output from the ADMS Working Group" ;
      foaf:page <http://www.w3.org/2011/gld/> ;
    ] ;
  foaf:maker [
      foaf:name "Government Linked Data WG, based on output from the ADMS Working Group" ;
      foaf:page <http://www.w3.org/2011/gld/> ;
    ] ;
.
adms:Asset
  rdf:type rdfs:Class ;
  dcterms:identifier "adms:Asset" ;
  rdfs:comment "An Asset is an abstract entity that reflects the intellectual content of the asset and represents those characteristics of the asset that are independent of its physical embodiment. This abstract entity combines the FRBR entities work (a distinct intellectual or artistic creation) and expression (the intellectual or artistic realization of a work). Assets can be versioned. Every time the intellectual content of an asset changes, the result is considered to be a new asset that can be linked to previous and next versions of the Asset. The physical embodiment of an Asset is called an Asset Distribution. A particular Asset may have zero or more Asset Distributions."@en ;
  rdfs:isDefinedBy <http://www.w3.org/TR/vocab-adms/> ;
  rdfs:label "Asset"@en ;
  rdfs:subClassOf rdfs:Resource ;
  rdfs:subClassOf dcat:Dataset ;
.
adms:AssetDistribution
  rdf:type rdfs:Class ;
  dcterms:identifier "adms:AssetDistribution" ;
  rdfs:comment "An Asset Distribution represents a particular physical embodiment of an Asset, which is an example of the FRBR entity manifestation (the physical embodiment of an expression of a work). An Asset Distribution is typically a downloadable computer file (but in principle it could also be a paper document) that implements the intellectual content of an Asset. A particular Asset Distribution is associated with one and only one Asset, while all Distributions of an Asset share the same intellectual content in different physical formats. Asset Distributions themselves are not versioned."@en ;
  rdfs:isDefinedBy <http://www.w3.org/TR/vocab-adms/> ;
  rdfs:label "Asset Distribution"@en ;
  rdfs:subClassOf rdfs:Resource ;
  rdfs:subClassOf dcat:Distribution ;
.
adms:AssetRepository
  rdf:type rdfs:Class ;
  dcterms:identifier "adms:AssetRepository" ;
  rdfs:comment "An Asset Repository is a system or service that provides facilities for storage and maintenance of descriptions of Assets and Asset Distributions, and functionality that allows users to search and access these descriptions. An Asset Repository will typically contain descriptions of several Assets and related Asset Distributions."@en ;
  rdfs:isDefinedBy <http://www.w3.org/TR/vocab-adms/> ;
  rdfs:label "Asset Repository"@en ;
  rdfs:subClassOf rdfs:Resource ;
  rdfs:subClassOf dcat:Catalog ;
.
adms:Identifier
  rdf:type rdfs:Class ;
  dcterms:identifier "adms:Identifier" ;
  rdfs:comment """This class is based on the UN/CEFACT 
    Identifier complex type defined in See Section 5.8 of Core Components Data Type Catalogue Version 3.1 (http://www.unece.org/fileadmin/DAM/cefact/codesfortrade/CCTS/CCTS-DTCatalogueVersion3p1.pdf)
    In RDF this is expressed using the following properties:
    - the content string should be provided using skos:notation, datatyped with the identifier scheme (inclduing the version number if appropriate);
    - use dcterms:creator to link to a class describing the agency that manages the identifier scheme or adms:schemaAgency to provide the name as a literal.
    Although not part of the ADMS conceptual model, it may be useful to provide further properties to the Identifier class such as
    dcterms:created to provide the date on which the identifier was issued."""^^rdf:XMLLiteral ;
  rdfs:isDefinedBy <http://www.w3.org/TR/vocab-adms/> ;
  rdfs:label "Identifier"@en ;
  rdfs:subClassOf rdfs:Resource ;
.
adms:identifier
  rdf:type rdf:Property ;
  rdf:type owl:ObjectProperty ;
  dcterms:identifier "adms:identifier" ;
  rdfs:comment """adms:identifier is used to link any resource to 
      an instance of adms:Identifier which is its range. N.B. it is not appropriate to use 
      dcterms:identifer to link to the Identifier class as its range is rdfs:Literal.
      ADMS uses this to provide any identifier for the Asset."""^^rdf:XMLLiteral ;
  rdfs:isDefinedBy <http://www.w3.org/TR/vocab-adms/> ;
  rdfs:label "identifier"@en ;
  rdfs:range adms:Identifier ;
.
adms:includedAsset
  rdf:type rdf:Property ;
  rdf:type owl:ObjectProperty ;
  dcterms:identifier "adms:includedAsset" ;
  rdfs:comment "Links to an Asset that is contained in the Asset being described, e.g. when there are several vocabularies defined in a single document."@en ;
  rdfs:domain adms:Asset ;
  rdfs:isDefinedBy <http://www.w3.org/TR/vocab-adms/> ;
  rdfs:label "included asset"@en ;
  rdfs:range adms:Asset ;
.
adms:interoperabilityLevel
  rdf:type rdf:Property ;
  rdf:type owl:ObjectProperty ;
  dcterms:identifier "adms:interoperabilityLevel" ;
  rdfs:comment "Links an Asset to its adms:InteroperabilityLevel. Since this is encoded using skos:Concept, that is the defined range for this property."^^rdf:XMLLiteral ;
  rdfs:domain adms:Asset ;
  rdfs:isDefinedBy <http://www.w3.org/TR/vocab-adms/> ;
  rdfs:label "interoperability level"@en ;
  rdfs:range skos:Concept ;
.
adms:last
  rdf:type rdf:Property ;
  rdf:type owl:ObjectProperty ;
  dcterms:identifier "adms:last" ;
  rdfs:comment "A link to the current or latest version of the Asset." ;
  rdfs:isDefinedBy <http://www.w3.org/TR/vocab-adms/> ;
  rdfs:label "last"@en ;
  rdfs:subPropertyOf <http://www.w3.org/1999/xhtml/vocab#last> ;
.
adms:next
  rdf:type rdf:Property ;
  rdf:type owl:ObjectProperty ;
  dcterms:identifier "adms:next" ;
  rdfs:comment "A link to the next version of the Asset." ;
  rdfs:isDefinedBy <http://www.w3.org/TR/vocab-adms/> ;
  rdfs:label "next"@en ;
  rdfs:subPropertyOf <http://www.w3.org/1999/xhtml/vocab#next> ;
.
adms:prev
  rdf:type rdf:Property ;
  rdf:type owl:ObjectProperty ;
  dcterms:identifier "adms:prev" ;
  rdfs:comment "A link to the previous version of the Asset." ;
  rdfs:isDefinedBy <http://www.w3.org/TR/vocab-adms/> ;
  rdfs:label "prev"@en ;
  rdfs:subPropertyOf <http://www.w3.org/1999/xhtml/vocab#prev> ;
.
adms:representationTechnique
  rdf:type rdf:Property ;
  rdf:type owl:ObjectProperty ;
  dcterms:identifier "adms:representationTechnique" ;
  rdfs:comment "Links an adms:AssetDistribution to a skos:Concept that is its adms:RepresentationTechnique."^^rdf:XMLLiteral ;
  rdfs:isDefinedBy <http://www.w3.org/TR/vocab-adms/> ;
  rdfs:label "representation technique"@en ;
  rdfs:range skos:Concept ;
.
adms:sample
  rdf:type rdf:Property ;
  rdf:type owl:ObjectProperty ;
  dcterms:identifier "adms:sample" ;
  rdfs:comment "Links to a sample of an Asset (which is itself an Asset)."@en ;
  rdfs:domain adms:Asset ;
  rdfs:isDefinedBy <http://www.w3.org/TR/vocab-adms/> ;
  rdfs:label "sample"@en ;
  rdfs:range adms:Asset ;
.
adms:schemeAgency
  rdf:type rdf:Property ;
  rdf:type owl:DatatypeProperty ;
  dcterms:identifier "adms:schemeAgency" ;
  rdfs:comment "The name of the agency responsible for issuing the identifier"@en ;
  rdfs:domain adms:Identifier ;
  rdfs:isDefinedBy <http://www.w3.org/TR/vocab-adms/> ;
  rdfs:label "scheme agency"@en ;
  rdfs:range rdfs:Literal ;
.
adms:status
  rdf:type rdf:Property ;
  rdf:type owl:ObjectProperty ;
  dcterms:identifier "adms:status" ;
  rdfs:comment """Links to the status of the Asset or Asset Distribution 
      in the context of a particular workflow process. Since Status is defined using a skos:Concept, 
      that is the defined range for this property."""^^rdf:XMLLiteral ;
  rdfs:isDefinedBy <http://www.w3.org/TR/vocab-adms/> ;
  rdfs:label "status"@en ;
  rdfs:range skos:Concept ;
.
adms:supportedSchema
  rdf:type rdf:Property ;
  rdf:type owl:ObjectProperty ;
  dcterms:identifier "adms:supportedSchema" ;
  rdfs:comment "A schema according to which the Asset Repository can provide data about its content, e.g. ADMS"@en ;
  rdfs:isDefinedBy <http://www.w3.org/TR/vocab-adms/> ;
  rdfs:label "supported schema"@en ;
  rdfs:range adms:Asset ;
.
adms:translation
  rdf:type rdf:Property ;
  rdf:type owl:ObjectProperty ;
  dcterms:identifier "adms:translation" ;
  rdfs:comment "Links Assets that are translations of each other."@en ;
  rdfs:isDefinedBy <http://www.w3.org/TR/vocab-adms/> ;
  rdfs:label "translation"@en ;
.
adms:versionNotes
  rdf:type rdf:Property ;
  rdf:type owl:DatatypeProperty ;
  dcterms:identifier "adms:versionNotes" ;
  rdfs:comment "A description of changes between this version and the previous version of the Asset."@en ;
  rdfs:isDefinedBy <http://www.w3.org/TR/vocab-adms/> ;
  rdfs:label "version notes"@en ;
  rdfs:range rdfs:Literal ;
.
org:
  dcterms:contributor [
      foaf:homepage <http://www.asahi-net.or.jp/~ax2s-kmtn/> ;
      foaf:name "Shuji Kamitsuna" ;
    ] ;
  dcterms:contributor [
      foaf:mbox "antonio.maccioni@agid.gov.it" ;
      foaf:name "Antonio Maccioni" ;
    ] ;
  dcterms:contributor [
      foaf:mbox "dave@epimorphics.com" ;
      foaf:name "Dave Reynolds" ;
    ] ;
  dcterms:contributor [
      foaf:mbox "dguardiola@quinode.fr" ;
      foaf:name "Dominique Guardiola" ;
    ] ;
  dcterms:contributor [
      foaf:mbox "emontiel@fi.upm.es" ;
      foaf:name "Elena Montiel Ponsoda" ;
    ] ;
  dcterms:contributor [
      foaf:mbox "giorgia.lodi@agid.gov.it" ;
      foaf:name "Giorgia Lodi" ;
    ] ;
  dcterms:contributor [
      foaf:mbox "lupe@fi.upm.es" ;
      foaf:name "Guadalupe Aguado de Cea" ;
    ] ;
  dcterms:contributor [
      foaf:mbox "mpoveda@fi.upm.es" ;
      foaf:name "María Poveda Villalón" ;
    ] ;
  dcterms:contributor [
      foaf:mbox "ogiraldo@fi.upm.es" ;
      foaf:name "Olga Ximena Giraldo" ;
    ] ;
  dcterms:created "2010-05-28"^^xsd:date ;
  dcterms:license <http://www.opendatacommons.org/licenses/pddl/1.0/> ;
  dcterms:modified "2010-06-09"^^xsd:date ;
  dcterms:modified "2010-10-08"^^xsd:date ;
  dcterms:modified "2012-09-30"^^xsd:date ;
  dcterms:modified "2012-10-06"^^xsd:date ;
  dcterms:modified "2013-02-15"^^xsd:date ;
  dcterms:modified "2013-12-16"^^xsd:date ;
  dcterms:modified "2014-01-02"^^xsd:date ;
  dcterms:modified "2014-01-25"^^xsd:date ;
  dcterms:modified "2014-02-05"^^xsd:date ;
  dcterms:modified "2014-04-12"^^xsd:date ;
  dcterms:title "Core organization ontology"@en ;
  dcterms:title "Ontologia delle organizzazioni"@it ;
  dcterms:title "Ontologie des organisations"@fr ;
  dcterms:title "Ontología de organizaciones"@es ;
  rdfs:comment "Vocabolario per descrivere strutture organizzative, le quali possono essere specializzate in una vasta varietà di tipi di organizzazione"@it ;
  rdfs:comment "Vocabulario para describir organizaciones, adaptable a una amplia variedad de ellas."@es ;
  rdfs:comment "Vocabulary for describing organizational structures, specializable to a broad variety of types of organization."@en ;
  rdfs:label "Core organization ontology"@en ;
  rdfs:label "Ontologia delle organizzazioni"@it ;
  rdfs:label "Ontologie des organisations"@fr ;
  rdfs:label "Ontología de organizaciones"@es ;
  rdfs:seeAlso <http://www.w3.org/TR/vocab-org/> ;
  owl:versionInfo "0.8" ;
.
org:ChangeEvent
  rdf:type rdfs:Class ;
  rdf:type owl:Class ;
  rdfs:comment "Evento que da como resultado un cambio sustancial en la organización, por ejemplo, una fusión o una reestructuración total. Está pensado para situaciones en las que la organización resultante es lo suficientemente distinta de las organizaciones originales, tiene una identidad distinta y una URI también distinta. Se deberían definir subtipos de eventos mediante vocabularios específicos (Extension vocabularies) para referirse a categorías de eventos específicos. El momento o periodo en el que el evento ocurre se debería expresar mediante las propiedades `prov:startAtTime` y `prov:endedAtTime`, y una descripción del mismo se debería incluir mediante el uso de la propiedad `dct:description`."@es ;
  rdfs:comment "Rappresenta un evento risultato essere un importante cambiamento per un'organizzazione come ad esempio una fusione o una riorganizzazione. È pensato per quelle situazioni in cui l'organizzazione risultante si distingue da quella originale sufficientemente da essere rappresentata con una URI differente. Le estensioni del vocabolario dovrebbero definire le sotto-classi per esprimere particolari categorie di eventi. L'istante o l'intervallo in cui l'evento accade dovrebbe essere espresso tramite `prov:startAtTime` e`prov:endedAtTime`. Una descrizione dovrebbe essere fornita attraverso `dct:description`."@it ;
  rdfs:comment "Represents an event which resulted in a major change to an organization such as a merger or complete restructuring. It is intended for situations where the resulting organization is sufficient distinct from the original organizations that it has a distinct identity and distinct URI. Extension vocabularies should define sub-classes of this to denote particular categories of event. The instant or interval at which the event occurred should be given by `prov:startAtTime` and `prov:endedAtTime`, a description should be given by `dct:description`. "@en ;
  rdfs:comment "Représente un Évènement impliquant un changement majeur dans l'Organisation, comme une fusion ou une restructuration. Prévu pour des situations ou l'organisation finale est suffisamment différente des Organisations originales pour qu'elle ait une identité et une URI distinctes. Des vocabulaires d'extension devraient définir des sous-classes de celle-ci pour annoter les différentes catégories d'Évènemenents. Le moment ou l'intervalle de l'Évènement devrait être indiqué avec `prov:startAtTime` et `prov:endedAtTime`, et une description avec la classe `dct:description`. "@fr ;
  rdfs:comment "合併や完全な再編などの組織に大きな変化をもたらした出来事を表わします。これは、結果として作成される組織と元の組織とが、別のアイデンティティーと別のURIを持つに足るほど異なる状況を対象としています。"@ja ;
  rdfs:isDefinedBy <http://www.w3.org/ns/org> ;
  rdfs:label "Change Event"@en ;
  rdfs:label "Evento di cambiamento"@it ;
  rdfs:label "evento de cambio"@es ;
  rdfs:label "Évènement"@fr ;
  rdfs:subClassOf prov:Activity ;
.
org:FormalOrganization
  rdf:type rdfs:Class ;
  rdf:type owl:Class ;
  rdfs:comment "An Organization which is recognized in the world at large, in particular in legal jurisdictions, with associated rights and responsibilities. Examples include a Corporation, Charity, Government or Church. Note that this is a super class of `gr:BusinessEntity` and it is recommended to use the GoodRelations vocabulary to denote Business classifications such as DUNS or NAICS."@en ;
  rdfs:comment "Organización reconocida a nivel mundial, en particular en jurisdicciones legales, con derechos y responsabilidades asociadas. Algunos ejemplos son: organización corporativa, organización benéfica, organización gubernamental, organización religiosa. Se debe tener en cuenta que ésta es una superclase de `gr:BusinessEntity` y que se recomienda el uso del vocabulario GoodRelations para referirse a clasificaciones de negocios tales como DUNS o NAICS."@es ;
  rdfs:comment "Un'organizzazione che è riconosciuta a livello mondiale o, in generale, all'interno di una qualche giurisdizione, e che quindi possiede diritti e responsabilità. Ad esempio aziende, enti governativi, associazioni di volontariato. Si noti che questa è una superclasse di `gr:BusinessEntity` e che quindi è raccomandabile usare il vocabolario GoodRelations per esprimere classificazioni di tipo industriale e commerciale come DUNS e NAICS."@it ;
  rdfs:comment "Une Organisation reconnue, en particulier par les juridictions locales, ayant des droits et des responsabilités. Exemples : entreprises, association à but non-lucratif, collectivité, église. Notez que c'est une super-classe de `gr:BusinessEntity` et qu'il est recommandé d'utiliser le vocabulaire GoodRelations pour indiquer les classifications économiques comme le code NACE."@fr ;
  rdfs:comment "関連する権利と責任を有する（特に法的管轄区域において）世界中に広く認識されている組織。例には、企業、慈善団体、政府や教会が含まれます。"@ja ;
  rdfs:isDefinedBy <http://www.w3.org/ns/org> ;
  rdfs:label "Formal Organization"@en ;
  rdfs:label "Organisation Formelle"@fr ;
  rdfs:label "Organizzazione formale"@it ;
  rdfs:label "organización formal"@es ;
  rdfs:subClassOf org:Organization ;
  rdfs:subClassOf foaf:Organization ;
.
org:Head
  rdf:type org:Role ;
  rdfs:comment "A role corresponding to the `org:headOf` property"@en ;
  rdfs:comment "Actividad correspondiente a la propiedad `org:headOf`."@es ;
  rdfs:comment "Un ruolo corrispondente alla proprietà `org:headOf`."@it ;
  rdfs:comment "Un rôle correspondant à la propriété `org:headOf`"@fr ;
  rdfs:isDefinedBy <http://www.w3.org/ns/org> ;
  rdfs:label "director ejecutivo"@es ;
  rdfs:label "directora ejecutiva"@es ;
  rdfs:label "head"@en ;
  rdfs:label "responsabile"@it ;
  rdfs:label "responsable"@fr ;
  skos:prefLabel "head"@en ;
  skos:prefLabel "responsabile"@it ;
  skos:prefLabel "responsable"@fr ;
  org:roleProperty org:headOf ;
.
org:Membership
  rdf:type rdfs:Class ;
  rdf:type owl:Class ;
  rdfs:comment "Indica la natura della relazione di appartenenza di un Agent in un'organizzazione. Rappresenta una relazione n-aria tra un'Agent, un Organization e un Role. È possibile indicare direttamente la membership, indipendentemente dallo specifico Role, attraverso l'uso della proprietà `org:memberOf`"@it ;
  rdfs:comment "Indicates the nature of an Agent's membership of an organization. Represents an n-ary relation between an Agent, an Organization and a Role. It is possible to directly indicate membership, independent of the specific Role, through use of the `org:memberOf` property."@en ;
  rdfs:comment "Indique la nature de l'engagement d'un Agent dans une Organisation. Représente une relation n-aire entre un Agent, une Organisation et un Role. Il est possible d'indiquer directement l'appartenance à une organisation, independemment d'un rôle spécifique, à travers l'usage de la propriété `org:memberOf`."@fr ;
  rdfs:comment "Pertenencia o afiliación de un agente a una organización. Es una relación n-aria entre un agente, una organización y una actividad. Es posible indicar pertenencia mediante el uso de la propiedad `org:memberOf`, independientemente de la actividad específica que se desempeñe."@es ;
  rdfs:comment "組織のエージェントの構成員の本質を示します。"@ja ;
  rdfs:isDefinedBy <http://www.w3.org/ns/org> ;
  rdfs:label "Appartenenza"@it ;
  rdfs:label "Engagement"@fr ;
  rdfs:label "Membership"@en ;
  rdfs:label "membresía"@es ;
  rdfs:subClassOf owl:Thing ;
  owl:disjointWith org:ChangeEvent ;
  owl:disjointWith org:Site ;
.
org:Organization
  rdf:type rdfs:Class ;
  rdf:type owl:Class ;
  rdfs:comment "Grupo de personas que se organiza en una comunidad u otro tipo de estructura social, comercial o política. Dicho grupo tiene un objetivo o motivo común para su existencia que va más allá del conjunto de personas que lo forman y que puede actuar como “agente”. A menudo las organizaciones se pueden agrupar en estructuras jerárquicas. Se recomienda el uso de etiquetas de SKOS para denominar a cada “organización”. En concreto, `skos:prefLabel` para la denominación principal o recomendada (aquella reconocida legalmente, siempre que sea posible), `skos:altLabel` para denominaciones alternativas (nombre comercial, sigla, denominación por la que se conoce a la organización coloquialmente) y `skos:notation` para referirse al código que identifique a la organización en una lista de códigos. Denominaciones alternativas: _colectivo_ _corporación_ _grupo_"@es ;
  rdfs:comment "Rappresenta una collezione di persone organizzate all'interno di una communità o di una qualche struttura sociale, commerciale o politica. Il gruppo condivide un obiettivo o una ragione d'essere che va oltre gli stessi membri appartenenti al gruppo e  può agire come un Agent. Le organizzazioni si possono spesso suddividere in strutture gerarchiche. Si raccomanda di usare le label per l'Organization mediante le proprietà di SKOS. In particolare, `skos:prefLabel` per il nome principale (possibilmente un nome legalmente riconosciuto)”, `skos:altLabel` come nome alternativo (denominazione commerciale, denominazione colloquiale) e `skos:notation` per indicare un codice di una lista di codici."@it ;
  rdfs:comment "Represents a collection of people organized together into a community or other social, commercial or political structure. The group has some common purpose or reason for existence which goes beyond the set of people belonging to it and can act as an Agent. Organizations are often decomposable into hierarchical structures.  It is recommended that SKOS lexical labels should be used to label the Organization. In particular `skos:prefLabel` for the primary (possibly legally recognized name), `skos:altLabel` for alternative names (trading names, colloquial names) and `skos:notation` to denote a code from a code list. Alternative names: _Collective_ _Body_ _Org_ _Group_"@en ;
  rdfs:comment "Représente un groupe de personnes organisées en communauté où tout autre forme de structure sociale, commerciale ou politique. Le groupe a un but commun ou une raison d'être qui va au-delà de la somme des personnes qui en font partie et peut agir en tant que \"Agent\". Les organisations sont souvent décomposables en structures hiérarchisées. Il est recommandé que des labels lexicaux SKOS soient utilisés pour nommer l'Organisation. En particulier `skos:prefLabel` pour le nom principal (en général le nom légal), `skos:altLabel` pour les noms alternatifs (marques, sigles, appellations familières) et `skos:notation` pour indiquer un code provenant d'une liste de code."@fr ;
  rdfs:comment "コミュニティー、その他の社会、商業、政治的な構造に共に編入された人々の集合を表わします。グループには、そこに属する人々を超えた、存在に対するある共通の目的や理由があり、エージェント（代理）を務めることができます。組織は、多くの場合、階層構造に分割できます。"@ja ;
  rdfs:isDefinedBy <http://www.w3.org/ns/org> ;
  rdfs:label "Organisation"@fr ;
  rdfs:label "Organization"@en ;
  rdfs:label "Organizzazione"@it ;
  rdfs:label "organización"@es ;
  rdfs:subClassOf owl:Thing ;
  rdfs:subClassOf foaf:Agent ;
  owl:disjointWith org:ChangeEvent ;
  owl:disjointWith org:Membership ;
  owl:disjointWith org:Role ;
  owl:disjointWith org:Site ;
  owl:equivalentClass foaf:Organization ;
  owl:hasKey (
      org:identifier
    ) ;
.
org:OrganizationalCollaboration
  rdf:type rdfs:Class ;
  rdf:type owl:Class ;
  rdfs:comment "A collaboration between two or more Organizations such as a project. It meets the criteria for being an Organization in that it has an identity and defining purpose independent of its particular members but is neither a formally recognized legal entity nor a sub-unit within some larger organization. Might typically have a shorter lifetime than the Organizations within it, but not necessarily. All members are `org:Organization`s rather than individuals and those Organizations can play particular roles within the venture. Alternative names: _Project_ _Venture_  _Endeavour_ _Consortium_ _Endeavour_"@en ;
  rdfs:comment "Colaboración determinada entre dos o más organizaciones, como en el caso de un proyecto común. Cumple con los criterios de ser una organización en sí misma, en la medida en que tiene una identidad y un propósito definido independiente de sus miembros en particular, pero no es una entidad legal formalmente reconocida ni una sub-unidad dentro de una organización más grande. La duración suele ser más corta que la de las organizaciones que lo componen, pero no necesariamente. Todos sus miembros son de tipo `org:Organization` en vez de individuos, y desempeñan una actividad concreta en el marco del proyecto de cooperación."@es ;
  rdfs:comment "Une collaboration entre deux ou plusieurs Organisations, telle qu'un projet commun. Un partenariat peut être considéré comme Organisation dans le sens ou il possède une identité et un But propre indépendant de ceux de ses membres, mais ce n'est ni une entité légale ni une sous-unité d'une Organisation plus grande. Typiquement, elle peut avoir une durée de vie plus courte que les Organisations qui la composent, mais pas nécessairement. Tous les membres sont des `org:Organization`s plutôt que des individus et ces Organisations peuvent jouer des Rôles particuliers au sein du Partenariat. "@fr ;
  rdfs:comment "È una collaborazione tra due o più Organization come ad esempio un progetto. Consente di rappresentare alcune identità dell'Organization che sono fuori dallo scopo principale e non sono formalmente riconosciute. Potrebbe anche avere un ciclo di vita limitato."@it ;
  rdfs:comment "プロジェクトなどの2つ以上の組織間のコラボレーション。それは、アイデンティティを有し、その特定のメンバーとは無関係に目的を定めているという点で、組織としての基準を満たしますが、正式に認識された法的実体でも、あるより大きな組織内のサブユニットでもありません。一般的には、その内部の組織よりも存続期間が短いかもしれませんが、必ずしもそうとは限りません。"@ja ;
  rdfs:isDefinedBy <http://www.w3.org/ns/org> ;
  rdfs:label "Collaborazione"@it ;
  rdfs:label "Endeavour"@en ;
  rdfs:label "Partenariat"@fr ;
  rdfs:label "proyecto de cooperación empresarial"@es ;
  rdfs:subClassOf org:Organization ;
  owl:equivalentClass [
      rdf:type owl:Class ;
      owl:intersectionOf (
          org:Organization
          [
            rdf:type owl:Restriction ;
            owl:allValuesFrom org:Organization ;
            owl:onProperty org:hasMember ;
          ]
        ) ;
    ] ;
.
org:OrganizationalUnit
  rdf:type rdfs:Class ;
  rdf:type owl:Class ;
  rdfs:comment "An Organization such as a University Support Unit which is part of some larger FormalOrganization and only has full recognition within the context of that FormalOrganization, it is not a Legal Entity in its own right. Units can be large and complex containing other Units and even FormalOrganizations. Alternative names: _OU_ _Unit_ _Department_"@en ;
  rdfs:comment "Organización que forma parte de una organización formal más amplia, como el servicio de informática o centro de cálculo de una universidad, y que sólo tiene reconocimiento pleno en el contexto de dicha organización formal, pero que no es una entidad legal propiamente dicha. Estas unidades pueden ser amplias y complejas, e incluir a otras unidades o incluso a otras organizaciones formales. Denominaciones alternativas: departamento."@es ;
  rdfs:comment "Un'organizzazione come ad esempio l'unità dei sistemi informativi che è parte di una più grande FormalOrganization e che, pur essendo riconosciuta nel contesto della propria organizzazione di riferimento, non è legalmente riconosciuta come entità a sé stante. Le unità possono essere ampie e complesse e contenere al loro interno sia altre unità che addirittura FormalOrganization."@it ;
  rdfs:comment "Une organisation telle que le support informatique d'une université, qui fait partie d'une Organisation Formelle plus importante et qui ne peut être reconnue qu'en tant que membre de cette organisation supérieure, ce n'est pas une entité légale en elle-même. Les unités opérationnelles peuvent être étendues, complexes et inclure elles-mêmes d'autres branches ou Unités Opérationnelles, voire des Organisations Formelles."@fr ;
  rdfs:comment "あるより大きな組織の一部であり、その組織の中においてのみ完全に認識される部局や支援部署などの組織です。特に、その単位はそれ自体では法的実体と見なされません。"@ja ;
  rdfs:isDefinedBy <http://www.w3.org/ns/org> ;
  rdfs:label "OrganizationalUnit"@en ;
  rdfs:label "Unità Organizzativa"@it ;
  rdfs:label "Unité opérationnelle"@fr ;
  rdfs:label "unidad organizativa"@es ;
  rdfs:subClassOf org:Organization ;
.
org:Post
  rdf:type rdfs:Class ;
  rdf:type owl:Class ;
  rdfs:comment "A Post represents some position within an organization that exists independently of the person or persons filling it. Posts may be used to represent situations where a person is a member of an organization ex officio (for example the Secretary of State for Scotland is part of UK Cabinet by virtue of being Secretary of State for Scotland, not as an individual person). A post can be held by multiple people and hence can be treated as a organization in its own right."@en ;
  rdfs:comment "Puesto o posición que representa algún tipo de empleo dentro de una organización, que existe independientemente de la persona o personas que lo desempeñan. Esta clase puede utilizarse para representar situaciones en las que una persona es miembro de una organización ex oficio (por ejemplo, el Secretario de Estado escocés es parte del Gabinete del gobierno británico por virtud de ser Secretario de Estado en Escocia, y no como individuo). Un puesto puede ser desempeñado por múltiples individuos y de aquí que sea tratado como una organización en sí misma."@es ;
  rdfs:comment "Un Impiego rappresenta una posizione all'interno dell'organizzazione che esiste indipendentemente dalla persona che la ricopre. Gli impieghi possono essere utilizzati per le situazioni in cui una persona è membro di un'organizzazione o di un ufficio (ad esempio un segretario di stato). Un Impiego può essere ricoperto da più persone."@it ;
  rdfs:comment "Un Poste représente une position au sein d'une Organisation qui existe indépendamment de la personne ou des personnes qui le remplissent. Les postes peuvent être utilisés pour représenter des situations où une personne est membre d'une Organisation d'office (par exemple, le Secrétaire d'Etat pour l'Ecosse fait partie du Cabinet du Royaume-Uni du fait d'être Secrétaire d'Etat pour l'Ecosse, non pas comme une personne physique). Un poste après peut être occupé par plusieurs personnes et peut donc être considéré comme une Organisation à part entière."@fr ;
  rdfs:comment "ポストは、それを埋める人（人々）とは無関係に存在する組織内のある位置を表わします。ポストは、人が職権上、組織のメンバーである状況を表わすために使用できます（例えば、スコットランド大臣は、個人としてではなく、スコットランド大臣であることにより、英国内閣の一部です）。ポストは、複数の人々によって保持されることが可能だあるため、それ自体を組織として扱うことができます。"@ja ;
  rdfs:isDefinedBy <http://www.w3.org/ns/org> ;
  rdfs:label "Impiego"@it ;
  rdfs:label "Post"@en ;
  rdfs:label "Poste"@fr ;
  rdfs:label "puesto"@es ;
  rdfs:subClassOf owl:Thing ;
.
org:Role
  rdf:type rdfs:Class ;
  rdf:type owl:Class ;
  rdfs:comment "Denotes a role that a Person or other Agent can take in an organization. Instances of this class describe the abstract role; to denote a specific instance of a person playing that role in a specific organization use an instance of `org:Membership`. It is common for roles to be arranged in some taxonomic structure and we use SKOS to represent that. The normal SKOS lexical properties should be used when labelling the Role. Additional descriptive properties for the Role, such as a Salary band, may be added by extension vocabularies."@en ;
  rdfs:comment "Función que una persona o agente desempeña en el seno de una organización. Las instancias de esta clase describen la actividad en abstracto; si lo que se pretende es incluir una instancia que refleje la función o actividad que desempeña una persona en concreto en una organización específica, se indica el uso de instancias de la clase `org:Membership`. Es común que dichas actividades se representen en una estructura taxonómica mediante SKOS. Las propiedades léxicas de SKOS deberían utilizarse a la hora de denominar o etiquetar la actividad desempeñada. Para añadir propiedades descriptivas adicionales, como rango salarial, se tendrá que recurrir a vocabularios externos."@es ;
  rdfs:comment "Indica il ruolo che una Person o un altro Agent può assumere in un'organizzazione. Le istanze di questa classe descrivono un ruolo astratto; per esprimere il ruolo che una precisa persona ricopre in un'organizzazione si usi un'istanza di `org:Membership`. È comune organizzare i ruoli in una qualche struttura tassonomica e quindi si raccomanda SKOS per questo. Altre proprietà descrittive per il Role, come salario, possono essere aggiunte mediante l'uso di altri vocabolari."@it ;
  rdfs:comment "Indique le rôle qu'une Personne ou un autre Agent peut avoir dans une Organisation. Les instances de cette classe décrivent le rôle dans l'absolu; pour indiquer une personne ayant ce rôle spécifique dans une Organisation, utilisez une instance de `org:Membership`. Il est courant que les rôles soient organisés dans une sorte de taxonomie, ce qui peut être représenté avec SKOS. Les propriétés de libellés standards de SKOS devraient être utilisées pour libeller le Rôle. D'autres propriétés additionnelles pour ce rôle, comme une fourchette de Salaire peuvent être ajoutées par une extension de ce vocabulaire."@fr ;
  rdfs:comment "人またはその他のエージェントが組織で担うことができる役割を表わします。この種のインスタンスは、抽象的な役割を記述します。特定の組織でその役割を担っている人の特定のインスタンスを示すためには、org:Membershipのインスタンスを使用します。"@ja ;
  rdfs:isDefinedBy <http://www.w3.org/ns/org> ;
  rdfs:label "Role"@en ;
  rdfs:label "Ruolo"@it ;
  rdfs:label "Rôle"@fr ;
  rdfs:label "actividad"@es ;
  rdfs:subClassOf skos:Concept ;
  owl:disjointWith org:ChangeEvent ;
  owl:disjointWith org:Membership ;
  owl:disjointWith org:Site ;
.
org:Site
  rdf:type rdfs:Class ;
  rdf:type owl:Class ;
  rdfs:comment "An office or other premise at which the organization is located. Many organizations are spread across multiple sites and many sites will host multiple locations. In most cases a Site will be a physical location. However, we don't exclude the possibility of non-physical sites such as a virtual office with an associated post box and phone reception service. Extensions may provide subclasses to denote particular types of site."@en ;
  rdfs:comment "Oficina, local o cualquier otro lugar en el que se encuentra una organización. Muchas organizaciones están distribuidas en varias sedes, que a su vez están repartidas en distintas ubicaciones. En muchos casos una sede será un sitio o local físico. Sin embargo, no se excluye la posibilidad de lugares no físicos como oficinas virtuales con los correspondientes apartados de correo y servicio de atención telefónica. Se pueden añadir más subtipos mediante extensiones para incluir tipos especiales de lugares."@es ;
  rdfs:comment "Un ufficio o altra sede dovei l'organizzazione è situata. Molte organizzazione sono distribuite su più sedi e molte sedi ospitano più ubicazioni. Nella maggior parte dei casi un Site è una locazione fisica. Non si esclude la possibilità di indicare sedi non fisiche come ad esempio gli uffici virtuali. Le estensioni dell'ontologia potrebbero usare delle sottoclassi per rappresentare i tipi particolari di sede."@it ;
  rdfs:comment "Un établissement ou tout autre lieu dans lequel une Organisation est localisé. Beaucoup d'organisations sont dispersées à travers plusieurs sites. Dans la plupart des cas un Site sera un lieu physique. Toutefois, nous n'excluons pas la possibilité de sites non-physiques comme un bureau virtuel avec une boîte postale et un service de secrétariat mutualisé. Des extensions pourraient fournir des sous-classes pour décrire des types de sites particuliers."@fr ;
  rdfs:comment "組織が位置するオフィスやその他の敷地。多くの組織が複数のサイトに散在しており、多くのサイトが多数の場所を持つでしょう。"@ja ;
  rdfs:isDefinedBy <http://www.w3.org/ns/org> ;
  rdfs:label "Sede"@it ;
  rdfs:label "Site"@en ;
  rdfs:label "Site"@fr ;
  rdfs:label "sede"@es ;
  rdfs:subClassOf owl:Thing ;
  owl:disjointWith org:ChangeEvent ;
.
org:basedAt
  rdf:type rdf:Property ;
  rdf:type owl:ObjectProperty ;
  rdfs:comment "Indica la sede in cui una è stabilita una persona. Non esclude la possibilità che una persona sia allocata su più sedi."@it ;
  rdfs:comment "Indicates the site at which a person is based. We do not restrict the possibility that a person is based at multiple sites."@en ;
  rdfs:comment "Indique le site sur lequel une personne est basée. Nous ne limitons pas le nombre de sites sur lesquels une personne peut être basée."@fr ;
  rdfs:comment "Lugar en el que trabaja una persona. No se restringe el hecho de que una persona pueda estar adscrita a múltiples ubicaciones."@es ;
  rdfs:comment "人が基礎としているサイトを示します。人が複数のサイトを基礎としている可能性を制限しません。"@ja ;
  rdfs:domain foaf:Person ;
  rdfs:isDefinedBy <http://www.w3.org/ns/org> ;
  rdfs:label "basata a"@it ;
  rdfs:label "based At"@en ;
  rdfs:label "basé à"@fr ;
  rdfs:label "trabaja en la sede"@es ;
  rdfs:range org:Site ;
.
org:changedBy
  rdf:type rdf:Property ;
  rdf:type owl:ObjectProperty ;
  rdfs:comment "Evento de cambio que resulta en una modificación en la organización. Dependiendo del evento, la organización puede dejar de existir tras el cambio. Es la relación inversa de `org:originalOrganization`."@es ;
  rdfs:comment "Indica un evento che ha contribuito al cambiamento di questa organizzazione. A seconda dell'evento, l'organizzazione potrebbe essere esistente dopo l'evento o aver cessato la propria esistenza. È l'inverso di `org:originalOrganization`."@it ;
  rdfs:comment "Indicates a change event which resulted in a change to this organization. Depending on the event the organization may or may not have continued to exist after the event. Inverse of `org:originalOrganization`."@en ;
  rdfs:comment "Indique un évènement qui a impliqué un changement dans l'Organisation. Selon l'évènement, l'Organisation a continué à exister après l'évènement, ou pas. Inverse de `org:originalOrganization`."@fr ;
  rdfs:comment "この組織の変更のきっかけとなった出来事を示します。"@ja ;
  rdfs:domain org:Organization ;
  rdfs:isDefinedBy <http://www.w3.org/ns/org> ;
  rdfs:label "cambiata da"@it ;
  rdfs:label "changed by"@en ;
  rdfs:label "es modificada por"@es ;
  rdfs:label "es modificado por"@es ;
  rdfs:label "modifiée par"@fr ;
  rdfs:range org:ChangeEvent ;
  owl:inverseOf org:originalOrganization ;
.
org:classification
  rdf:type rdf:Property ;
  rdf:type owl:ObjectProperty ;
  rdfs:comment "Indica una classificazione per questa Organization all'interno di un qualche schema di classificazione. Alcuni vocabolari potrebbero voler specializzare questa proprietà per avere un codominio corrispondente a uno specifico `skos:ConceptScheme`. Si noti che la presenza di questa proprietà è ancora in fase di discussione e potrebbe  essere revisionata o rimossa."@it ;
  rdfs:comment "Indicates a classification for this Organization within some classification scheme. Extension vocabularies may wish to specialize this property to have a range corresponding to a specific `skos:ConceptScheme`. This property is under discussion and may be revised or removed - in many cases organizations are best categorized by defining a sub-class hierarchy in an extension vocabulary."@en ;
  rdfs:comment "Indique une classification pour cette Organisation dans le cadre d'un schéma de classification. Il est possible de spécialiser cette propriété en utilisant un vocabulaire spécialisé pour que le champ corresponde à un concept spécifique `skos:ConceptScheme`. Cette propriété est en discussion est pourrait être révisée ou supprimée - dans de nombreux cas, les organisations sont mieux catégorisées par une hiérarchie de sous-classe dans un vocabulaire externe."@fr ;
  rdfs:comment "Ordenación jerárquica que se hace de una organización dentro de un esquema de clasificación. Es posible que algunos vocabularios especifiquen esta propiedad de forma que el rango se corresponda con un `skos:ConceptScheme` específico. La conveniencia de incluir esta propiedad se está debatiendo y puede que se revise o elimine (en muchos casos las organizaciones se clasifican mejor si se define una jerarquía de subclases en un vocabulario aparte)"@es ;
  rdfs:comment """ある分類表内のこの組織に対する分類を示します。
アプリケーションがorg:Organizationのサブクラスを組織的なカテゴリーを表わす手段として定義することも許容されることに注意してください。"""@ja ;
  rdfs:domain org:Organization ;
  rdfs:isDefinedBy <http://www.w3.org/ns/org> ;
  rdfs:label "classification"@en ;
  rdfs:label "classification"@fr ;
  rdfs:label "classificazione"@it ;
  rdfs:label "pertenece a la clasificación"@es ;
  rdfs:range skos:Concept ;
.
org:hasMember
  rdf:type rdf:Property ;
  rdf:type owl:ObjectProperty ;
  rdfs:comment "Indica una persona che è membro della data Organization. È l'inverso di `org:memberOf` ed è fornita per  compatibilità con `foaf:member`."@it ;
  rdfs:comment "Indicates a person who is a member of the subject Organization. Inverse of `org:memberOf`, see that property for further clarification. Provided for compatibility with `foaf:member`."@en ;
  rdfs:comment "Indique une personne membre de l'Organisation sujet. Inverse de `org:memberOf`, voyez la description de cette propriété pour plus de précisions. Fourni pour la compatibilité avec `foaf:member`."@fr ;
  rdfs:comment "Persona que es miembro de la organización en cuestión. Es la relación inversa de `org:memberOf`, véase la descripción de esa propiedad para más detalles. Se prevé compatibilidad con foaf:member`."@es ;
  rdfs:comment "対象組織のメンバーであるエージェント（人または他の組織）を示します。org:memberOfの逆。さらに明確な説明については、そのプロパティーを参照してください。"@ja ;
  rdfs:domain org:Organization ;
  rdfs:isDefinedBy <http://www.w3.org/ns/org> ;
  rdfs:label "ha membro"@it ;
  rdfs:label "has member"@en ;
  rdfs:label "possède un membre"@fr ;
  rdfs:label "tiene miembro"@es ;
  rdfs:range foaf:Agent ;
  owl:equivalentProperty foaf:member ;
  owl:inverseOf org:memberOf ;
.
org:hasMembership
  rdf:type rdf:Property ;
  rdf:type owl:ObjectProperty ;
  rdfs:comment "Indica una relazione di appartenenza che coinvolge un Agent. È l'inverso di `org:member`."@it ;
  rdfs:comment "Indicates a membership relationship that the Agent plays. Inverse of `org:member`."@en ;
  rdfs:comment "Indique pour cet Agent un engagement dans une Organisation. Inverse de `org:member`."@fr ;
  rdfs:comment "Relación de pertenencia o afiliación a una organización en la que el agente desempeña un cargo o función. Es la relación inversa de `org:member`."@es ;
  rdfs:comment "エージェントが担う構成員関係を示します。"@ja ;
  rdfs:domain foaf:Agent ;
  rdfs:isDefinedBy <http://www.w3.org/ns/org> ;
  rdfs:label "appartenenza"@it ;
  rdfs:label "engagement"@fr ;
  rdfs:label "membership"@en ;
  rdfs:label "tiene membresía"@es ;
  rdfs:range org:Membership ;
  owl:inverseOf org:member ;
.
org:hasPost
  rdf:type rdf:Property ;
  rdf:type owl:ObjectProperty ;
  rdfs:comment "Indica il Post che è presente in una Organization."@it ;
  rdfs:comment "Indicate un Poste qui existe dans l'Organisation."@fr ;
  rdfs:comment "Indicates a Post which exists within the Organization."@en ;
  rdfs:comment "Posición que existe en una organización."@es ;
  rdfs:comment "組織内に存在するポストを示します。"@ja ;
  rdfs:domain org:Organization ;
  rdfs:isDefinedBy <http://www.w3.org/ns/org> ;
  rdfs:label "impiego"@it ;
  rdfs:label "possède un poste"@fr ;
  rdfs:label "post"@en ;
  rdfs:label "tiene puesto"@es ;
  rdfs:range org:Post ;
.
org:hasPrimarySite
  rdf:type rdf:Property ;
  rdf:type owl:ObjectProperty ;
  rdfs:comment "Indica la sede principale per l'Organization. È da considerarsi come la sede di default in cui l'Organization deve essere contattata pur non essendo necessariamente il quartier generale."@it ;
  rdfs:comment "Indicates a primary site for the Organization, this is the default means by which an Organization can be contacted and is not necessarily the formal headquarters."@en ;
  rdfs:comment "Indique le site principal d'une Organisation, le moyen par défaut par lequel l'Organisation peut être contactée et pas nécessairement le siège social légal."@fr ;
  rdfs:comment "Oficina principal de la organización, la opción por defecto para ponerse en contacto con una organización, aunque no corresponde necesariamente con las oficinas centrales de la organización."@es ;
  rdfs:comment "組織の主要サイトを示します。組織の窓口となりえるデフォルトの手段ですが、正式な本部とは限りません。"@ja ;
  rdfs:domain org:Organization ;
  rdfs:isDefinedBy <http://www.w3.org/ns/org> ;
  rdfs:label "primary Site"@en ;
  rdfs:label "sede principale"@it ;
  rdfs:label "site principal"@fr ;
  rdfs:label "tiene sede principal en"@es ;
  rdfs:range org:Site ;
  rdfs:subPropertyOf org:hasSite ;
.
org:hasRegisteredSite
  rdf:type rdf:Property ;
  rdf:type owl:ObjectProperty ;
  rdfs:comment "Indica la sede legale per l'Organization. In molte giurisdizioni è richiesto che una FormalOrganization abbia una sede di questo tipo."@it ;
  rdfs:comment "Indicates the legally registered site for the organization, in many legal jurisdictions there is a requirement that FormalOrganizations such as Companies or Charities have such a primary designed site. "@en ;
  rdfs:comment "Indique l'établissement principal légalement enregistré pour l'Organisation. Dans de nombreuses juridictions existe l'obligation pour une Organisation Formelle d'avoir un tel site principal. "@fr ;
  rdfs:comment "Oficina o sede legalmente registrada de la organización. En muchas jurisdicciones legales existe el requisito de que organizaciones formales tales como empresas u organizaciones de beneficencia tengan una sede principal de este tipo."@es ;
  rdfs:comment "組織の法律上登録されたサイトを示し、多くの法的管轄区域では、会社や慈善団体などのFormalOrganizations（正式な組織）がそのような主要サイトを持っているという要件があります。"@ja ;
  rdfs:domain org:FormalOrganization ;
  rdfs:isDefinedBy <http://www.w3.org/ns/org> ;
  rdfs:label "registered Site"@en ;
  rdfs:label "sede legale"@it ;
  rdfs:label "siège social"@fr ;
  rdfs:label "tiene sede registrada en"@es ;
  rdfs:range org:Site ;
  rdfs:subPropertyOf org:hasPrimarySite ;
.
org:hasSite
  rdf:type rdf:Property ;
  rdf:type owl:ObjectProperty ;
  rdfs:comment "Indica la sede in cui l'Organization ha una qualche presenza anche in modo indiretto (ad esempio un ufficio virtuale). È l'inverso di `org:siteOf`."@it ;
  rdfs:comment "Indicates a site at which the Organization has some presence even if only indirect (e.g. virtual office or a professional service which is acting as the registered address for a company). Inverse of `org:siteOf`."@en ;
  rdfs:comment "Indique un site sur lequel l'Organisation possède une présence, même indirecte (domiciliation, boite postale). Inverse de `org:siteOf`."@fr ;
  rdfs:comment "Lugar en donde la organización tiene algún tipo de presencia, incluso si es de forma indirecta (por ejemplo, una oficina virtual o servicio profesional que hagan la función de dirección registrada de la compañía). Es la relación inversa de `org:siteOf`."@es ;
  rdfs:comment "組織が、間接（例えば、会社の登録住所として機能しているバーチャル・オフィスやプロフェッショナル・サービス）のみであったとしても、ある存在感を持っているサイトを示します。"@ja ;
  rdfs:domain org:Organization ;
  rdfs:isDefinedBy <http://www.w3.org/ns/org> ;
  rdfs:label "a un site"@fr ;
  rdfs:label "ha sede"@it ;
  rdfs:label "has site"@en ;
  rdfs:label "tiene sede en"@es ;
  rdfs:range org:Site ;
  owl:inverseOf org:siteOf ;
.
org:hasSubOrganization
  rdf:type rdf:Property ;
  rdf:type owl:ObjectProperty ;
  rdfs:comment "Indique le statut de dépendance hiérarchique pour des Organisations ou des Unités Opérationnelles; indique une Organisation qui est une sous-partie ou une branche d'une Organisation plus large. C'est la propriété inverse de `org:subOrganizationOf`."@fr ;
  rdfs:comment "Organización jerárquica de organizaciones o unidades. Indica que una organización es parte de otra organización más amplia o pertenece a ella. Es la relación inversa de `org:subOrganizationOf`."@es ;
  rdfs:comment "Rappresenta un contenimento gerarchico di una Organization o di una OrganizationalUnit. Indica una organizzazione che è parte di una organizzazione più grande. È l'inverso di `org:subOrganizationOf`."@it ;
  rdfs:comment "Represents hierarchical containment of Organizations or Organizational Units; indicates an organization which is a sub-part or child of this organization.  Inverse of `org:subOrganizationOf`."@en ;
  rdfs:comment "組織または組織単位の階層的包含を表わします。この組織のサブパートまたは子である組織を示します。"@ja ;
  rdfs:domain org:Organization ;
  rdfs:isDefinedBy <http://www.w3.org/ns/org> ;
  rdfs:label "a une Sous-Organization"@fr ;
  rdfs:label "ha sotto-Organization"@it ;
  rdfs:label "has SubOrganization"@en ;
  rdfs:label "tiene suborganización"@es ;
  rdfs:range org:Organization ;
  owl:inverseOf org:subOrganizationOf ;
.
org:hasUnit
  rdf:type rdf:Property ;
  rdf:type owl:ObjectProperty ;
  rdfs:comment "Indica un'unità che è parte di questa Organization, come ad esempio un dipartimento facente parte di una più ampia FormalOrganization. È l'inverso di `org:unitOf`."@it ;
  rdfs:comment "Indicates a unit which is part of this Organization, e.g. a Department within a larger FormalOrganization. Inverse of `org:unitOf`."@en ;
  rdfs:comment "Indique une Unité qui fait partie d'une Organisation, par exemple un Départment au sein d'une Organisation Formelle plus large. Inverse de `org:unitOf`."@fr ;
  rdfs:comment "Unidad que es parte de la organización, como, por ejemplo, un departamento incluido en una organización formal más amplia."@es ;
  rdfs:comment "例えば、より大きな組織内の部局など、この組織の一部である単位を示します。"@ja ;
  rdfs:domain org:FormalOrganization ;
  rdfs:isDefinedBy <http://www.w3.org/ns/org> ;
  rdfs:label "contiene unidad"@es ;
  rdfs:label "ha Unit"@it ;
  rdfs:label "has Unit"@en ;
  rdfs:label "possède une Unité"@fr ;
  rdfs:range org:OrganizationalUnit ;
  rdfs:subPropertyOf org:hasSubOrganization ;
  owl:inverseOf org:unitOf ;
.
org:headOf
  rdf:type rdf:Property ;
  rdf:type owl:ObjectProperty ;
  rdfs:comment "Indica che una persona è leader o responsabile formale di una Organization. Questo significa che la persona è alla radice del grafo (aciclico) creato dalle `org:reportsTo`, sebbene un'organizzazione possa avere più di un responsabile."@it ;
  rdfs:comment "Indicates that a person is the leader or formal head of the Organization. This will normally mean that they are the root of the `org:reportsTo` (acyclic) graph, though an organization may have more than one head."@en ;
  rdfs:comment "Indique qu'une personne est le directeur ou le responsable formel d'une Organisation. Ceci indique souvent qu'il est au sommet de du graphe acyclique des `org:reportsTo`, même si une organisation peut avoir plus d'un responsable."@fr ;
  rdfs:comment "Persona que es jefe o jefa, representante ,,director o directora de la organización. Esto significa que dicha persona es el rango de la relación `org:reportsTo` en el organigrama de la organización (acíclico), aunque una organización puede tener más de un jefe."@es ;
  rdfs:comment "人（または他のエージェント）が組織のリーダーや正式なトップであることを示します。"@ja ;
  rdfs:domain foaf:Person ;
  rdfs:isDefinedBy <http://www.w3.org/ns/org> ;
  rdfs:label "es director ejecutivo de"@es ;
  rdfs:label "head of"@en ;
  rdfs:label "responsabile di"@it ;
  rdfs:label "responsable de"@fr ;
  rdfs:range org:Organization ;
  rdfs:subPropertyOf org:memberOf ;
.
org:heldBy
  rdf:type rdf:Property ;
  rdf:type owl:ObjectProperty ;
  rdfs:comment "Agente que ocupa un puesto."@es ;
  rdfs:comment "Indica un Agent che ricopre un Post."@it ;
  rdfs:comment "Indicate un Agent qui occupe le Poste."@fr ;
  rdfs:comment "Indicates an Agent which holds a Post."@en ;
  rdfs:comment "ポストを保持するエージェントを示します。"@ja ;
  rdfs:domain org:Post ;
  rdfs:isDefinedBy <http://www.w3.org/ns/org> ;
  rdfs:label "held by"@en ;
  rdfs:label "occupé par"@fr ;
  rdfs:label "ocupado por"@es ;
  rdfs:label "ricoperto da"@it ;
  rdfs:range foaf:Agent ;
.
org:holds
  rdf:type rdf:Property ;
  rdf:type owl:ObjectProperty ;
  rdfs:comment "Indica un Impiego ricoperto da un Agent."@it ;
  rdfs:comment "Indicate un Poste occupé par un Agent."@fr ;
  rdfs:comment "Indicates a Post held by some Agent."@en ;
  rdfs:comment "Puesto ocupado por algún agente."@es ;
  rdfs:comment "あるエージェントによって保持されているポストを示します。"@ja ;
  rdfs:domain foaf:Agent ;
  rdfs:isDefinedBy <http://www.w3.org/ns/org> ;
  rdfs:label "holds"@en ;
  rdfs:label "occupe"@fr ;
  rdfs:label "ocupa"@es ;
  rdfs:label "ricopre"@it ;
  rdfs:range org:Post ;
  owl:inverseOf org:heldBy ;
.
org:identifier
  rdf:type rdf:Property ;
  rdf:type owl:DatatypeProperty ;
  rdfs:comment "Código o identificador, como por ejemplo el CIF de una empresa, que permite identificar de forma inequívoca a una organización. Existen muchos códigos de identificación tanto nacionales como internacionales. Esta ontología no obliga al uso de ningún esquema en concreto. Los códigos de identificación utilizados en cada caso se deberían indicar mediante el uso de la propiedad “datatype” del valor del identificador. El uso de la propiedad “datatype” para especificar el esquema de notación utilizado está en consonancia con las buenas prácticas recomendadas para el uso de la propiedad `skos:notation`, de la que esta propiedad es una especialización."@es ;
  rdfs:comment "Donne un identifiant, comme par exemple le numéro d'enregistrement d'une entreprise, qui peut être utilisé comme identifiant unique pour l'Organisation. De nombreux schémas nationaux et internationaux sont disponibles. Cette ontologie reste neutre par rapport au schéma utilisé. Le schéma particulier utilisé devrait être indiqué par le `datatype` de la valeur de l'identifiant. Utiliser les datatypes pour distinguer les schémas de notation est cohérent avec les bonnes pratiques pour `skos:notation` dont cette propriété est une spécialisation."@fr ;
  rdfs:comment "Gives an identifier, such as a company registration number, that can be used to used to uniquely identify the organization. Many different national and international identier schemes are available. The org ontology is neutral to which schemes are used. The particular identifier scheme should be indicated by the datatype of the identifier value.  Using datatypes to distinguish the notation scheme used is consistent with recommended best practice for `skos:notation` of which this property is a specialization."@en ;
  rdfs:comment "Indica un identificatore univoco per l'organizzazione, come ad esempio la partita IVA di un'azienda. Molti schemi di identificazione a livello nazionale e internazionale sono disponibili allo scopo. L'ontologia ORG è neutrale rispetto allo schema da utilizzare. Lo schema di identificazione dovrebbe essere indicato dal datatype del valore dell'identificatore. L'uso del datatype per distinguere lo schema di identificazione è coerente con le best practice per `skos:notation`, di cui questa proprietà è una specializzazione."@it ;
  rdfs:comment "組織を一意に識別するために使用できる会社登録番号などの識別子を与えます。"@ja ;
  rdfs:domain org:Organization ;
  rdfs:isDefinedBy <http://www.w3.org/ns/org> ;
  rdfs:label "identifiant"@fr ;
  rdfs:label "identificatore"@it ;
  rdfs:label "identifier"@en ;
  rdfs:label "tiene identificador"@es ;
  rdfs:subPropertyOf skos:notation ;
.
org:linkedTo
  rdf:type rdf:Property ;
  rdf:type owl:ObjectProperty ;
  rdfs:comment "2つの組織の任意の関係を示します。"@ja ;
  rdfs:comment "Indica una relazione arbitraria tra due organizzazioni. Ad esempio, specializzazioni di questa proprietà possono essere usate per denotare relazioni particolari tipo il finanziamento o la fornitura."@it ;
  rdfs:comment "Indicates an arbitrary relationship between two organizations. Specializations of this can be used to, for example, denote funding or supply chain relationships."@en ;
  rdfs:comment "Indique une relation arbitraire entre deux Organisations. Des spécialisations peuvent être utilisées pour, par exemple, qualifier une relation de fournisseur ou de financeur."@fr ;
  rdfs:comment "Relación arbitraria entre dos organizaciones. Las especializaciones de esta relación se pueden utilizar para denotar relaciones de financiación o suministro, entre otras."@es ;
  rdfs:domain org:Organization ;
  rdfs:isDefinedBy <http://www.w3.org/ns/org> ;
  rdfs:label "collegato a"@it ;
  rdfs:label "está relacionada con"@es ;
  rdfs:label "está relacionado con"@es ;
  rdfs:label "linked to"@en ;
  rdfs:label "relié à"@fr ;
  rdfs:range org:Organization ;
.
org:location
  rdf:type rdf:Property ;
  rdf:type owl:DatatypeProperty ;
  rdfs:comment "Gives a location description for a person within the organization, for example a _Mail Stop_ for internal posting purposes."@en ;
  rdfs:comment "Indica la descrizione del luogo presso cui è possibile reperire una persona dell'organizzazione."@it ;
  rdfs:comment "Indique la description de l'endroit ou est basé une personne de l'Organisation, par exemple pour des besoins de messagerie interne (Bureau 42)."@fr ;
  rdfs:comment "Lugar o ubicación exacta de una persona en una organización con el objetivo de facilitar, por ejemplo, la entrega de correo."@es ;
  rdfs:comment "例えば、内部配送目的のメール・ストップ（Mail Stop）などの、組織内の人の位置記述を提供します。"@ja ;
  rdfs:domain foaf:Person ;
  rdfs:isDefinedBy <http://www.w3.org/ns/org> ;
  rdfs:label "está ubicada en"@es ;
  rdfs:label "está ubicado en"@es ;
  rdfs:label "localisation"@fr ;
  rdfs:label "location"@en ;
  rdfs:label "luogo"@it ;
  rdfs:range xsd:string ;
.
org:member
  rdf:type rdf:Property ;
  rdf:type owl:FunctionalProperty ;
  rdf:type owl:ObjectProperty ;
  rdfs:comment "Indica la Person (o un altro Agent) coinvolto in una relazione di Membership. È l'inverso di `org:hasMembership`."@it ;
  rdfs:comment "Indicates the Person (or other Agent including Organization) involved in the Membership relationship. Inverse of `org:hasMembership`"@en ;
  rdfs:comment "Indique une personne (ou tout autre Agent, y compris une Organisation) impliqué dans la relation d'Engagement. Inverse de `org:hasMembership`"@fr ;
  rdfs:comment "Persona (u otro agente, incluyendo una organización) que participa en la relación de membresía. Es la relación inversa de `org:hasMembership`."@es ;
  rdfs:comment "構成員関係に含まれている人（または、組織を含んでいる他のエージェント）を示します。"@ja ;
  rdfs:domain org:Membership ;
  rdfs:isDefinedBy <http://www.w3.org/ns/org> ;
  rdfs:label "es condición de miembro sobre agente"@es ;
  rdfs:label "member"@en ;
  rdfs:label "membre"@fr ;
  rdfs:label "membro"@it ;
  rdfs:range foaf:Agent ;
  owl:inverseOf org:hasMembership ;
.
org:memberDuring
  rdf:type rdf:Property ;
  rdf:type owl:ObjectProperty ;
  rdfs:comment "Optional property to indicate the interval for which the membership is/was valid."@en ;
  rdfs:comment "Propiedad opcional que indica el periodo durante el cual la relación de membresía o pertenencia a una organización se mantiene en vigencia."@es ;
  rdfs:comment "Proprietà opzionale per indicare l'intervallo per il quale l'appartenenza è/è stata valida."@it ;
  rdfs:comment "Propriété optionnelle pour indiquer l'intervalle durant lequel l'engagemnet est ou était valide."@fr ;
  rdfs:comment "構成員が有効である／であった期間を示すためのオプションのプロパティー。"@ja ;
  rdfs:domain org:Membership ;
  rdfs:isDefinedBy <http://www.w3.org/ns/org> ;
  rdfs:label "durée d'engagement"@fr ;
  rdfs:label "es miembro durante"@es ;
  rdfs:label "member During"@en ;
  rdfs:label "membro durante"@it ;
.
org:memberOf
  rdf:type rdf:Property ;
  rdf:type owl:ObjectProperty ;
  rdfs:comment "Indica che una persona è membro di una Organization senza una precisa indicazione sulla natura di questa appartenenza e sul suo ruolo. Si noti che la scelta del nome di questa proprietà non intende limitarla alla sola  rappresentazione formalmente di un'appartenenza. La proprietà può coprire anche altri coinvolgimenti nell'organizzazione. Questa proprietà può essere specializzata per indicare ruoli all'interno organizzazione o relazioni di diverse tipologie. Ha `org:hasmember` come proprietà inversa opzionale."@it ;
  rdfs:comment "Indicates that a person is a member of the Organization with no indication of the nature of that membership or the role played. Note that the choice of property name is not meant to limit the property to only formal membership arrangements, it is also indended to cover related concepts such as affilliation or other involvement in the organization. Extensions can specialize this relationship to indicate particular roles within the organization or more nuanced relationships to the organization. Has an optional inverse, `org:hasmember`."@en ;
  rdfs:comment "Indique qu'une personne est membre de l'Organisation sans précision sur la nature de cet engagement ou du rôle joué. Notez que le choix du nom de cette propriété ne vise pas à la limiter aux seuls engagements formels, elle peut également couvrir des concepts reliés comme l'affiliation ou le bénévolat. Des extensions peuvent spécialiser cette relation pour indiquer des rôles particuliers au sein de l'Organisation or des relations plus nuancées avec elle. Possède une propriété inverse optionnelle, `org:hasmember`."@fr ;
  rdfs:comment "Persona que pertenece a la organización o es miembro de la misma, sin que conste la naturaleza de dicha pertenencia o el papel que desempeña. Se debe tener en cuenta que la elección de una denominación para esta propiedad no significa que la propiedad esté limitada a ciertos tipos de pertenencia formales, sino que pretende cubrir conceptos relacionados como el de afiliación u otras formas de participación en la organización. Se puede hacer uso de extensiones para especializar esta relación de forma que incluya tipos específicos de pertenencia a las organizaciones o relaciones especiales con la organización."@es ;
  rdfs:comment "エージェント（人または他の組織）が組織のメンバーであることを示します。ただし、その構成員の本質や担う役割は示しません。プロパティー名の選択は、プロパティーを正式な構成員配置のみに制限することが目的ではないことに注意してください。所属や組織へのその他の関与などの関連する概念をカバーすることも意図されています。拡張により、この関係を特殊化し、組織内の特定の役割やよりニュアンスを含んだ組織との関係を示すことができます。"@ja ;
  rdfs:domain foaf:Agent ;
  rdfs:isDefinedBy <http://www.w3.org/ns/org> ;
  rdfs:label "es miembro de"@es ;
  rdfs:label "member of"@en ;
  rdfs:label "membre de"@fr ;
  rdfs:label "membro di"@it ;
  rdfs:range org:Organization ;
  owl:inverseOf org:hasMember ;
.
org:organization
  rdf:type rdf:Property ;
  rdf:type owl:FunctionalProperty ;
  rdf:type owl:ObjectProperty ;
  rdfs:comment "Indica l'Organization in cui l'Agent è un membro."@it ;
  rdfs:comment "Indicates Organization in which the Agent is a member."@en ;
  rdfs:comment "Indique l'Organization dont l'agent est membre."@fr ;
  rdfs:comment "Organización a la que pertenece el agente en calidad de miembro."@es ;
  rdfs:comment "エージェントがメンバーである組織を示します。"@ja ;
  rdfs:domain org:Membership ;
  rdfs:isDefinedBy <http://www.w3.org/ns/org> ;
  rdfs:label "es condición de miembro sobre organización"@es ;
  rdfs:label "organisation"@fr ;
  rdfs:label "organization"@en ;
  rdfs:label "organizzazione"@it ;
  rdfs:range org:Organization ;
.
org:originalOrganization
  rdf:type rdf:Property ;
  rdf:type owl:ObjectProperty ;
  rdfs:comment "Indica una o più organizzazioni pregresse rispetto a un evento di cambiamento. A seconda dell'evento, queste organizzazioni potrebbero essere esistenti dopo l'evento o  aver cessato la loro esistenza. È l'inverso di `org:changedBy`."@it ;
  rdfs:comment "Indicates one or more organizations that existed before the change event. Depending on the event they may or may not have continued to exist after the event. Inverse of `org:changedBy`."@en ;
  rdfs:comment "Indique une ou plusieurs organisations qui ont existé avant un évènement de changement. Selon l'évènement, ces organisations ont pu continuer à exister ou non. Inverse de `org:changedBy`. "@fr ;
  rdfs:comment "Una o más organizaciones que existían antes de que sucediera el cambio en la organización. Dependiendo del tipo de cambio, dichas organizaciones pueden haber dejado de existir o no. Es la relación inversa de `org:changedBy`."@es ;
  rdfs:comment "変更のきっかけとなった出来事以前に存在した1つ以上の組織を示します。出来事によって、出来事の後にそれらは存在し続けたかも、存在し続けなかったかもしれません。"@ja ;
  rdfs:domain org:ChangeEvent ;
  rdfs:isDefinedBy <http://www.w3.org/ns/org> ;
  rdfs:label "es organización original"@es ;
  rdfs:label "organisation originelle"@fr ;
  rdfs:label "organizzazione originale"@it ;
  rdfs:label "original organization"@en ;
  rdfs:range org:Organization ;
  rdfs:subPropertyOf prov:used ;
  owl:inverseOf org:changedBy ;
.
org:postIn
  rdf:type rdf:Property ;
  rdf:type owl:ObjectProperty ;
  rdfs:comment "Indica l'Organization in cui il Post è presente."@it ;
  rdfs:comment "Indicate l'Organisation dans laquelle le Poste existe."@fr ;
  rdfs:comment "Indicates the Organization in which the Post exists."@en ;
  rdfs:comment "Organización en la que existe el puesto."@es ;
  rdfs:comment "ポストが存在する組織を示します。"@ja ;
  rdfs:domain org:Post ;
  rdfs:isDefinedBy <http://www.w3.org/ns/org> ;
  rdfs:label "es un puesto en"@es ;
  rdfs:label "impiego in"@it ;
  rdfs:label "post in"@en ;
  rdfs:label "poste chez"@fr ;
  rdfs:range org:Organization ;
  owl:inverseOf org:hasPost ;
.
org:purpose
  rdf:type rdf:Property ;
  rdfs:comment "Finalidad u objetivo de la organización. La organización puede tener muchos objetivos a diferentes niveles de abstracción, pero en la naturaleza de las organizaciones está el tener una razón para existir, y la finalidad de esta propiedad es documentar dicha razón. La organización podrá tener más de un objetivo. Se recomienda el uso de vocabularios controlados o listas de códigos para indicar el objetivo, preferentemente mediante el uso de un `skos:Concept`. Sin embargo, el rango no está predeterminado, de forma que otros tipos de esquemas descriptivos tiene cabida. Se espera que ciertas especializaciones de este vocabulario o ciertos perfiles de aplicaciones restrinjan el rango del objetivo. Denominaciones alternativas: área_ _jurisdicción_ _ responsabilidad _ (especialmente cuando se aplica a unidades tales como ministerios o divisiones administrativas de los gobiernos)"@es ;
  rdfs:comment "Indica l'obiettivo di questa Organization. In generale, si possono esprimere gli obiettivi di un'organizzazione secondo diversi livelli di astrazione, ma la natura stessa dell'organizzazione ha una ragione d'essere ed è proprio questa che deve essere catturata con tale proprietà. Inoltre, un'Organization può avere obiettivi multipli. È raccomandabile che l'obiettivo faccia parte di una code list, e che sia preferibilmente un `skos:Concept`. Ad ogni modo, il codominio della proprietà è lasciato aperto per consentire altri tipi di di descrizione. Conseguentemente, eventuali specializzazioni o profili applicativi possono utilizzare quel vocabolario come codominio della proprietà."@it ;
  rdfs:comment "Indicates the purpose of this Organization. There can be many purposes at different levels of abstraction but the nature of an organization is to have a reason for existence and this property is a means to document that reason. An Organization may have multiple purposes. It is recommended that the purpose be denoted by a controlled term or code list, ideally a `skos:Concept`. However, the range is left open to allow for other types of descriptive schemes. It is expected that specializations or application profiles of this vocabulary will constrain the range of the purpose. Alternative names: _remit_ _responsibility_ (esp. if applied to OrganizationalUnits such as Government Departments)."@en ;
  rdfs:comment "Indique le but de cette Organisation. Il peut exister plusieurs buts à différents niveaux d'abstraction mais la nature d'une organisation est d'avoir une raison d'exister et cette propriété doit servir à documenter cette raison d'être. Une Organisation peut avoir plusieurs Buts. Il est recommandé que le but soit libellé à l'aide d'un vocabulaire contrôlé ou autre code établi, idéalement avec un concept `skos:Concept`. Toutefois, le champ de cette propriété est laissé ouvert et pourrait accepter d'autres schémas de description. Il est préférable que les spécialisations ou les profils d'applications de ce vocabulaire contraignent le champ de cette propriété."@fr ;
  rdfs:comment "この組織の目的を示します。異なる抽象レベルの多くの目的がありえますが、組織の本質は存在理由を持つことであり、このプロパティーはその理由をドキュメント化する手段です。組織は、複数の目的を持っている可能性があります。"@ja ;
  rdfs:domain org:Organization ;
  rdfs:isDefinedBy <http://www.w3.org/ns/org> ;
  rdfs:label "but"@fr ;
  rdfs:label "obiettivo"@it ;
  rdfs:label "purpose"@en ;
  rdfs:label "tiene objetivo"@es ;
.
org:remuneration
  rdf:type rdf:Property ;
  rdf:type owl:ObjectProperty ;
  rdfs:comment "Indica il salario o altra forma di remunerazione associata al ruolo. In genere, questo si denota usando uno schema di rappresentazione esistente come il `gr:PriceSpecification` ma il codominio è lasciato libero di essere specializzato a seconda delle applicazioni."@it ;
  rdfs:comment "Indicates a salary or other reward associated with the role. Typically this will be denoted using an existing representation scheme such as `gr:PriceSpecification` but the range is left open to allow applications to specialize it (e.g. to remunerationInGBP)."@en ;
  rdfs:comment "Indique un salaire ou tout autre compensation associée au Rôle. Typiquement, ceci sera annoté en utilisant un schéma existant comme  `gr:PriceSpecification` mais le champ de cette propriété est laissé ouvert afin de permettre aux applications de la spécialiser (par exemple remunerationEuro)."@fr ;
  rdfs:comment "Salario o cualquier otra remuneración asociada con la actividad. La forma usual de referirse a dicha remuneración será utilizando un esquema de representación como el propuesto en la ontología GoodRelations `gr:PriceSpecification`, pero el rango se deja abierto a que las distintas aplicaciones lo especialicen (por ejemplo, remunerationInGBP)"@es ;
  rdfs:comment "役割に関係する給料やその他の報酬を示します。"@ja ;
  rdfs:domain org:Role ;
  rdfs:isDefinedBy <http://www.w3.org/ns/org> ;
  rdfs:label "recibe remuneración"@es ;
  rdfs:label "remuneration"@en ;
  rdfs:label "remunerazione"@it ;
  rdfs:label "rémuneration"@fr ;
.
org:reportsTo
  rdf:type rdf:Property ;
  rdf:type owl:ObjectProperty ;
  rdfs:comment "Indica una relazione di subordinazione all'interno dell'organigramma. La semantica precisa può variare a seconda dell'organizzazione, per esempio può essere usata per rappresentare la proprietà di supervisione oppure per le relazioni di rendicontazione."@it ;
  rdfs:comment "Indicates a reporting relationship as might be depicted on an organizational chart. The precise semantics of the reporting relationship will vary by organization but is intended to encompass both direct supervisory relationships (e.g. carrying objective and salary setting authority) and more general reporting or accountability relationships (e.g. so called _dotted line_ reporting)."@en ;
  rdfs:comment "Indique une relation de subordination comme elle pourrait figurer dans un organigramme. La sémantique précise de cette subordination pourra varier selon l'Organisation mais vise à englober aussi bien les relations hiérarchiques directes (définition d'objectifs, montant du salaire) que des relations plus générales ou organisationnelles (les liens en pointillés dans les organigrammes)."@fr ;
  rdfs:comment "Relación de subordinación que se representa en los organigramas de las organizaciones. La semántica de la relación de subordinación varía según las organizaciones, pero su intención es abarcar tanto a las relaciones de supervisión directa (por ejemplo, aquellas en las que la autoridad determina los objetivos o el salario) como a las relaciones de subordinación más generales (por ejemplo, las llamadas líneas de autoridad o de mando (y responsabilidad) (http://www.promonegocios.net/organigramas/tipos-de-organigramas.html))."@es ;
  rdfs:comment "組織図で描かれるかもしれないような上下関係を示します。エージェント間またはエージェントが就くことができるポスト間の上下関係を直接的に示すために使用できます。"@ja ;
  rdfs:domain [
      rdf:type owl:Class ;
      owl:unionOf (
          foaf:Agent
          org:Post
        ) ;
    ] ;
  rdfs:isDefinedBy <http://www.w3.org/ns/org> ;
  rdfs:label "est subordonné à"@fr ;
  rdfs:label "reports to"@en ;
  rdfs:label "responde ante"@es ;
  rdfs:label "riporta a"@it ;
  rdfs:range [
      rdf:type owl:Class ;
      owl:unionOf (
          foaf:Agent
          org:Post
        ) ;
    ] ;
.
org:resultedFrom
  rdf:type rdf:Property ;
  rdf:type owl:ObjectProperty ;
  rdfs:comment "Evento que tiene como resultado la creación de una organización."@es ;
  rdfs:comment "Indica l'evento che ha permesso all'organizzazione di instaurarsi. È l'inverso di `org:resultingOrganization`."@it ;
  rdfs:comment "Indicates an event which resulted in this organization. Inverse of `org:resultingOrganization`."@en ;
  rdfs:comment "Indique un évènement dont est issue l'Organisation. Inverse de `org:resultingOrganization`."@fr ;
  rdfs:comment "この組織になった（導いた、作成された）きっかけとなった出来事を示します。"@ja ;
  rdfs:domain org:Organization ;
  rdfs:isDefinedBy <http://www.w3.org/ns/org> ;
  rdfs:label "es el resultado de"@es ;
  rdfs:label "issue de"@fr ;
  rdfs:label "resulted from"@en ;
  rdfs:label "risultato da"@it ;
  rdfs:range org:ChangeEvent ;
  rdfs:subPropertyOf prov:wasGeneratedBy ;
  owl:inverseOf org:resultingOrganization ;
.
org:resultingOrganization
  rdf:type rdf:Property ;
  rdf:type owl:ObjectProperty ;
  rdfs:comment "Indica l'organizzazione che è stata creata o mutata a seguito dell'evento. È l'inverso di `org:resultedFrom`."@it ;
  rdfs:comment "Indicates an organization which was created or changed as a result of the event. Inverse of `org:resultedFrom`."@en ;
  rdfs:comment "Indique une organisation qui a été créée ou a été modifiée à la suite d'un Évènement de changement. Inverse de `org:resultedFrom`."@fr ;
  rdfs:comment "Organización que ha sido creada o modificada tras un evento específico.  Es la relación inversa de `org:resultedFrom`."@es ;
  rdfs:comment "出来事の結果、作成、変更された組織を示します。"@ja ;
  rdfs:domain org:ChangeEvent ;
  rdfs:isDefinedBy <http://www.w3.org/ns/org> ;
  rdfs:label "a donné naissance à"@fr ;
  rdfs:label "resulta en"@es ;
  rdfs:label "resulted in"@en ;
  rdfs:label "risultato in"@it ;
  rdfs:range org:Organization ;
  owl:inverseOf org:resultedFrom ;
.
org:role
  rdf:type rdf:Property ;
  rdf:type owl:ObjectProperty ;
  rdfs:comment "Actividad que el agente desempeña en una relación de pertenencia a una organización."@es ;
  rdfs:comment "Indica il Role che un Agent ricopre in una relazione di Membership con una Organization"@it ;
  rdfs:comment "Indicates the Role that the Agent plays in a Membership relationship with an Organization."@en ;
  rdfs:comment "Indique le Rôle de l'Agent dans son Engagement avec l'Organisation."@fr ;
  rdfs:comment "エージェントが組織との構成員関係において担う役割を示します。ポストの保持者が担う役割を示すためにorg:Postで用いることもできます。"@ja ;
  rdfs:domain [
      rdf:type owl:Class ;
      owl:unionOf (
          org:Membership
          org:Post
        ) ;
    ] ;
  rdfs:isDefinedBy <http://www.w3.org/ns/org> ;
  rdfs:label "desempeña la actividad de"@es ;
  rdfs:label "role"@en ;
  rdfs:label "ruolo"@it ;
  rdfs:label "rôle"@fr ;
  rdfs:range org:Role ;
.
org:roleProperty
  rdf:type rdf:Property ;
  rdf:type owl:AnnotationProperty ;
  rdfs:comment "Ceci est une méta-propriété utilisée pour annoter une instance de `org:Role` ayant une sous-propriété `org:memberOf` qui peut être utilisée pour indiquer directement le rôle et pouvoir faire des requêtes plus facilement. La sémantique visée est un Engagement impliquant l'existence d'une relation de propriété directe à travers d'une règle d'inférence de la forme:  `{ [] org:member ?p; org:organization ?o; org:role [org:roleProperty ?r] } -> {?p ?r ?o}`."@fr ;
  rdfs:comment "Meta-propiedad que se utiliza para anotar una instancia de `org:Role` con una sub-propiedad de `org:memberOf`, que puede ser utilizada para indicar directamente la actividad a fin de facilitar las consultas a los datos. The intended semantics is that a Membership relation involving the Role implies the existence of a direct property relationship through an inference rule of the form: { [] org:member ?a; org:organization ?o; org:role [org:roleProperty ?r] } -> {?a ?r ?o}"@es ;
  rdfs:comment "Questa è una meta-proprietà usata per annotare un'istanza di `org:Role` con una sotto-proprietà di `org:memberOf` e può essere usata per indicare direttamente il ruolo per facilitare un'interrogazione sui dati."@it ;
  rdfs:comment "This is a metalevel property which is used to annotate an `org:Role` instance with a sub-property of `org:memberOf` that can be used to directly indicate the role for easy of query. The intended semantics is a Membership relation involving the Role implies the existence of a direct property relationship through an inference rule of the form:  `{ [] org:member ?p; org:organization ?o; org:role [org:roleProperty ?r] } -> {?p ?r ?o}`."@en ;
  rdfs:comment "これは、クエリが容易になるように役割を直接的に示すために使用できるorg:memberOfのサブプロパティーでorg:Roleインスタンスを注釈するために用いられるメタレベルのプロパティーです。"@ja ;
  rdfs:domain org:Role ;
  rdfs:isDefinedBy <http://www.w3.org/ns/org> ;
  rdfs:label "desempeña la actividad de (propiedad)"@es ;
  rdfs:label "role (property)"@en ;
  rdfs:label "ruolo (proprietà)"@it ;
  rdfs:label "rôle (propriété)"@fr ;
  rdfs:range rdf:Property ;
.
org:siteAddress
  rdf:type rdf:Property ;
  rdf:type owl:ObjectProperty ;
  rdfs:comment "Dirección de la sede según una codificación adecuada. Se recomienda el uso de vCard (que utiliza el vocabulario en http://www.w3.org/TR/vcard-rdf/), pero el rango no se restringe únicamente al uso de este vocabulario sino que se permite el uso de otros códigos. La dirección puede constar de una dirección de correo electrónico, un número de teléfono o información de geo-localización, y no se limita a una dirección postal física."@es ;
  rdfs:comment "Indica un indirizzo per la sede in una codifica appropriata. Il codominio è lasciato libero ma è consigliabile l'uso del vocabolario vCard (http://www.w3.org/TR/vcard-rdf/). L'indirizzo può includere email, numero di telefono e informazioni di geolocalizzazione e non è vincolato ad essere un indirizzo fisico."@it ;
  rdfs:comment "Indicates an address for the site in a suitable encoding. Use of vCard (using the http://www.w3.org/TR/vcard-rdf/ vocabulary) is encouraged but the range is left open to allow other encodings to be used. The address may include email, telephone, and geo-location information and is not restricted to a physical address. "@en ;
  rdfs:comment "Indique une adresse pour le site dans un encodage approprié. L'usage du vocabulaire vCard ( http://www.w3.org/TR/vcard-rdf/) est encouragé, mais le range est ouvert pour permettre l'utilisation d'autres vocabulaires. L'adresse peut comporter le courriel, le téléphone, et l'information de géolocalisation; et n'est donc pas seulement limitée à une adresse physique. "@fr ;
  rdfs:comment "適切にコード化されたサイトのアドレスを示します。vCard[vcard-rdf]語彙などの有名なアドレスのコード化の使用が奨励されますが、他の符号化の使用を可能とするために値域はオープンのままにされます。アドレスには、電子メール、電話およびジオロケーション情報を含むことができ、物理的なアドレスに制限されません。"@ja ;
  rdfs:domain org:Site ;
  rdfs:isDefinedBy <http://www.w3.org/ns/org> ;
  rdfs:label "adresse du Site"@fr ;
  rdfs:label "es la dirección de la sede"@es ;
  rdfs:label "indirizzo della sede"@it ;
  rdfs:label "site Address"@en ;
.
org:siteOf
  rdf:type rdf:Property ;
  rdf:type owl:ObjectProperty ;
  rdfs:comment "Indica un'Organization che ha una qualche presenza nella data sede. È l'inverso di `org:hasSite`."@it ;
  rdfs:comment "Indicates an Organization which has some presence at the given site. This is the inverse of `org:hasSite`."@en ;
  rdfs:comment "Indique une Organisation qui a une présence sur le site en question. Inverse de `org:hasSite`."@fr ;
  rdfs:comment "Organización que tiene ubicación en un lugar. Es la relación inversa de `org:hasSite`."@es ;
  rdfs:comment "あるサイトである存在感を持っている組織を示します。"@ja ;
  rdfs:domain org:Site ;
  rdfs:isDefinedBy <http://www.w3.org/ns/org> ;
  rdfs:label "es sede de"@es ;
  rdfs:label "sede di"@it ;
  rdfs:label "site Of"@en ;
  rdfs:label "site de"@fr ;
  rdfs:range org:Organization ;
  owl:inverseOf org:hasSite ;
.
org:subOrganizationOf
  rdf:type rdf:Property ;
  rdf:type owl:ObjectProperty ;
  rdfs:comment "Distribución jerárquica de organizaciones o unidades. Indica que una organización contiene a otra organización. Es la relación inversa de `org:hasSubOrganization`"@es ;
  rdfs:comment "Rappresenta un contenimento gerarchico di una Organization o di una OrganizationalUnit. È l'inverso di `org:hasSubOrganization`. Ha nome come nome alternativo hasSubOrg."@it ;
  rdfs:comment "Represents hierarchical containment of Organizations or OrganizationalUnits; indicates an Organization which contains this Organization. Inverse of `org:hasSubOrganization`."@en ;
  rdfs:comment "Représente une relation hierarchique des Organisations ou des Unités Opérationnelles; indique une Organisation sujet qui contient cette Organisation. Inverse de `org:hasSubOrganization`."@fr ;
  rdfs:comment "組織または組織単位の階層的包含を表わします。この組織を含む組織を示します。"@ja ;
  rdfs:domain org:Organization ;
  rdfs:isDefinedBy <http://www.w3.org/ns/org> ;
  rdfs:label "es suborganización de"@es ;
  rdfs:label "sotto-Organization di"@it ;
  rdfs:label "sous-Organization de"@fr ;
  rdfs:label "subOrganization of"@en ;
  rdfs:range org:Organization ;
  rdfs:subPropertyOf org:transitiveSubOrganizationOf ;
  owl:inverseOf org:hasSubOrganization ;
.
org:transitiveSubOrganizationOf
  rdf:type rdf:Property ;
  rdf:type owl:ObjectProperty ;
  rdf:type owl:TransitiveProperty ;
  rdfs:comment "La version transitive de la propriété subOrganizationOf, renvoie une représentation de toutes les organisations qui contiennent celle-ci. Notez que ceci est une super-propriété de la relation transitive donc elle pourrait contenir des assertions additionnelles mais cet usage n'est pas recommandé."@fr ;
  rdfs:comment "La versión transitiva de la propiedad “subOrganizationOf”, es decir, la representación de todas las organizaciones en las que esta está contenida. Téngase en cuenta que desde el punto de vista técnico esta es una propiedad que contiene a todas las propiedades transitivas, de forma que podría contener afirmaciones adicionales, aunque su uso no está aconsejado."@es ;
  rdfs:comment "The transitive closure of subOrganizationOf, giving a representation of all organizations that contain this one. Note that technically this is a super property of the transitive closure so it could contain additional assertions but such usage is discouraged."@en ;
  rdfs:comment "subOrganizationOfの推移閉包で、これを含むすべての組織の表現を与える。技術的に、これが推移閉包のスーパープロパティーであるため、追加の言明を含むことができますが、そのような使用法はお勧めできないことに注意してください。"@ja ;
  rdfs:comment "È la chiusura transitiva di subOrganizationOf, quindi rappresenta tutte le organizzazioni che la contengono. Tecnicamente, essendo una chiusura transitiva, può contenere asserzioni che non la riguardano e quindi il suo uso è sconsigliato."@it ;
  rdfs:domain org:Organization ;
  rdfs:isDefinedBy <http://www.w3.org/ns/org> ;
  rdfs:label "es suborganización de (transitiva)"@es ;
  rdfs:label "es suborganización de manera transitiva de"@es ;
  rdfs:label "sotto-Organization transitiva"@it ;
  rdfs:label "sous-Organization transitive de"@fr ;
  rdfs:label "transitive sub-organization"@en ;
  rdfs:range org:Organization ;
.
org:unitOf
  rdf:type rdf:Property ;
  rdf:type owl:ObjectProperty ;
  rdfs:comment "Indica un Organization di cui questa Unit fa parte, come ad esempio un dipartimento all'interno di una più vasta FormalOrganization. È l'inverso di `org:hasUnit`."@it ;
  rdfs:comment "Indicates an Organization of which this Unit is a part, e.g. a Department within a larger FormalOrganization. This is the inverse of `org:hasUnit`."@en ;
  rdfs:comment "Indique l'Organisation dont cette Organisation ou Unité fait partie, par exemple un Départment au sein d'une Organisation Formelle plus large. Inverse de `org:hasUnit`."@fr ;
  rdfs:comment "Organización de la que es parte esta unidad, por ejemplo, un departamento incluido en una organización formal más amplia."@es ;
  rdfs:comment "例えば、より大きな組織内の部局など、この単位がその一部分である組織を示します。"@ja ;
  rdfs:domain org:OrganizationalUnit ;
  rdfs:isDefinedBy <http://www.w3.org/ns/org> ;
  rdfs:label "es unidad de"@es ;
  rdfs:label "unit Of"@en ;
  rdfs:label "unità di"@it ;
  rdfs:label "unité de"@fr ;
  rdfs:range org:FormalOrganization ;
  rdfs:subPropertyOf org:subOrganizationOf ;
  owl:inverseOf org:hasUnit ;
.
prov:Activity
  rdf:type owl:Class ;
  rdfs:isDefinedBy <http://www.w3.org/ns/prov-o#> ;
  rdfs:label "Activity" ;
  rdfs:subClassOf owl:Thing ;
  owl:disjointWith prov:Entity ;
  prov:category "starting-point" ;
  prov:component "entities-activities" ;
  prov:constraints "http://www.w3.org/TR/2013/REC-prov-constraints-20130430/#prov-dm-constraints-fig"^^xsd:anyURI ;
  prov:definition "An activity is something that occurs over a period of time and acts upon or with entities; it may include consuming, processing, transforming, modifying, relocating, using, or generating entities." ;
  prov:dm "http://www.w3.org/TR/2013/REC-prov-dm-20130430/#term-Activity"^^xsd:anyURI ;
  prov:n "http://www.w3.org/TR/2013/REC-prov-n-20130430/#expression-Activity"^^xsd:anyURI ;
.
prov:ActivityInfluence
  rdf:type owl:Class ;
  rdfs:comment "ActivityInfluence provides additional descriptions of an Activity's binary influence upon any other kind of resource. Instances of ActivityInfluence use the prov:activity property to cite the influencing Activity."@en ;
  rdfs:comment "It is not recommended that the type ActivityInfluence be asserted without also asserting one of its more specific subclasses."@en ;
  rdfs:isDefinedBy <http://www.w3.org/ns/prov-o#> ;
  rdfs:label "ActivityInfluence" ;
  rdfs:seeAlso prov:activity ;
  rdfs:subClassOf prov:Influence ;
  rdfs:subClassOf [
      rdf:type owl:Restriction ;
      owl:maxCardinality "0"^^xsd:nonNegativeInteger ;
      owl:onProperty prov:hadActivity ;
    ] ;
  owl:disjointWith prov:EntityInfluence ;
  prov:category "qualified" ;
  prov:editorsDefinition "ActivitiyInfluence is the capacity of an activity to have an effect on the character, development, or behavior of another by means of generation, invalidation, communication, or other."@en ;
.
prov:Agent
  rdf:type owl:Class ;
  rdfs:isDefinedBy <http://www.w3.org/ns/prov-o#> ;
  rdfs:label "Agent" ;
  rdfs:subClassOf owl:Thing ;
  owl:disjointWith prov:InstantaneousEvent ;
  prov:category "starting-point" ;
  prov:component "agents-responsibility" ;
  prov:definition "An agent is something that bears some form of responsibility for an activity taking place, for the existence of an entity, or for another agent's activity. "@en ;
  prov:dm "http://www.w3.org/TR/2013/REC-prov-dm-20130430/#term-agent"^^xsd:anyURI ;
  prov:n "http://www.w3.org/TR/2013/REC-prov-n-20130430/#expression-Agent"^^xsd:anyURI ;
.
prov:AgentInfluence
  rdf:type owl:Class ;
  rdfs:comment "AgentInfluence provides additional descriptions of an Agent's binary influence upon any other kind of resource. Instances of AgentInfluence use the prov:agent property to cite the influencing Agent."@en ;
  rdfs:comment "It is not recommended that the type AgentInfluence be asserted without also asserting one of its more specific subclasses."@en ;
  rdfs:isDefinedBy <http://www.w3.org/ns/prov-o#> ;
  rdfs:label "AgentInfluence" ;
  rdfs:seeAlso prov:agent ;
  rdfs:subClassOf prov:Influence ;
  prov:category "qualified" ;
  prov:editorsDefinition "AgentInfluence is the capacity of an agent to have an effect on the character, development, or behavior of another by means of attribution, association, delegation, or other."@en ;
.
prov:Association
  rdf:type owl:Class ;
  rdfs:comment "An instance of prov:Association provides additional descriptions about the binary prov:wasAssociatedWith relation from an prov:Activity to some prov:Agent that had some responsiblity for it. For example, :baking prov:wasAssociatedWith :baker; prov:qualifiedAssociation [ a prov:Association; prov:agent :baker; :foo :bar ]."@en ;
  rdfs:isDefinedBy <http://www.w3.org/ns/prov-o#> ;
  rdfs:label "Association" ;
  rdfs:subClassOf prov:AgentInfluence ;
  prov:category "qualified" ;
  prov:component "agents-responsibility" ;
  prov:definition "An activity association is an assignment of responsibility to an agent for an activity, indicating that the agent had a role in the activity. It further allows for a plan to be specified, which is the plan intended by the agent to achieve some goals in the context of this activity."@en ;
  prov:dm "http://www.w3.org/TR/2013/REC-prov-dm-20130430/#term-Association"^^xsd:anyURI ;
  prov:n "http://www.w3.org/TR/2013/REC-prov-n-20130430/#expression-Association"^^xsd:anyURI ;
  prov:unqualifiedForm prov:wasAssociatedWith ;
.
prov:Attribution
  rdf:type owl:Class ;
  rdfs:comment "An instance of prov:Attribution provides additional descriptions about the binary prov:wasAttributedTo relation from an prov:Entity to some prov:Agent that had some responsible for it. For example, :cake prov:wasAttributedTo :baker; prov:qualifiedAttribution [ a prov:Attribution; prov:entity :baker; :foo :bar ]."@en ;
  rdfs:isDefinedBy <http://www.w3.org/ns/prov-o#> ;
  rdfs:label "Attribution" ;
  rdfs:subClassOf prov:AgentInfluence ;
  prov:category "qualified" ;
  prov:component "agents-responsibility" ;
  prov:constraints "http://www.w3.org/TR/2013/REC-prov-constraints-20130430/#prov-dm-constraints-fig"^^xsd:anyURI ;
  prov:definition """Attribution is the ascribing of an entity to an agent.

When an entity e is attributed to agent ag, entity e was generated by some unspecified activity that in turn was associated to agent ag. Thus, this relation is useful when the activity is not known, or irrelevant."""@en ;
  prov:dm "http://www.w3.org/TR/2013/REC-prov-dm-20130430/#term-attribution"^^xsd:anyURI ;
  prov:n "http://www.w3.org/TR/2013/REC-prov-n-20130430/#expression-attribution"^^xsd:anyURI ;
  prov:unqualifiedForm prov:wasAttributedTo ;
.
prov:Bundle
  rdf:type owl:Class ;
  rdfs:comment "Note that there are kinds of bundles (e.g. handwritten letters, audio recordings, etc.) that are not expressed in PROV-O, but can be still be described by PROV-O."@en ;
  rdfs:isDefinedBy <http://www.w3.org/ns/prov-o#> ;
  rdfs:label "Bundle" ;
  rdfs:subClassOf prov:Entity ;
  prov:category "expanded" ;
  prov:definition "A bundle is a named set of provenance descriptions, and is itself an Entity, so allowing provenance of provenance to be expressed."@en ;
  prov:dm "http://www.w3.org/TR/2013/REC-prov-dm-20130430/#term-bundle-entity"^^xsd:anyURI ;
  prov:n "http://www.w3.org/TR/2013/REC-prov-n-20130430/#expression-bundle-declaration"^^xsd:anyURI ;
.
prov:Collection
  rdf:type owl:Class ;
  rdfs:isDefinedBy <http://www.w3.org/ns/prov-o#> ;
  rdfs:label "Collection" ;
  rdfs:subClassOf prov:Entity ;
  prov:category "expanded" ;
  prov:component "collections" ;
  prov:definition "A collection is an entity that provides a structure to some constituents, which are themselves entities. These constituents are said to be member of the collections."@en ;
  prov:dm "http://www.w3.org/TR/2013/REC-prov-dm-20130430/#term-collection"^^xsd:anyURI ;
.
prov:Communication
  rdf:type owl:Class ;
  rdfs:comment "An instance of prov:Communication provides additional descriptions about the binary prov:wasInformedBy relation from an informed prov:Activity to the prov:Activity that informed it. For example, :you_jumping_off_bridge prov:wasInformedBy :everyone_else_jumping_off_bridge; prov:qualifiedCommunication [ a prov:Communication; prov:activity :everyone_else_jumping_off_bridge; :foo :bar ]."@en ;
  rdfs:isDefinedBy <http://www.w3.org/ns/prov-o#> ;
  rdfs:label "Communication" ;
  rdfs:subClassOf prov:ActivityInfluence ;
  prov:category "qualified" ;
  prov:component "entities-activities" ;
  prov:constraints "http://www.w3.org/TR/2013/REC-prov-constraints-20130430/#prov-dm-constraints-fig"^^xsd:anyURI ;
  prov:definition "Communication is the exchange of an entity by two activities, one activity using the entity generated by the other." ;
  prov:dm "http://www.w3.org/TR/2013/REC-prov-dm-20130430/#term-Communication"^^xsd:anyURI ;
  prov:n "http://www.w3.org/TR/2013/REC-prov-n-20130430/#expression-wasInformedBy"^^xsd:anyURI ;
  prov:unqualifiedForm prov:wasInformedBy ;
.
prov:Delegation
  rdf:type owl:Class ;
  rdfs:comment "An instance of prov:Delegation provides additional descriptions about the binary prov:actedOnBehalfOf relation from a performing prov:Agent to some prov:Agent for whom it was performed. For example, :mixing prov:wasAssociatedWith :toddler . :toddler prov:actedOnBehalfOf :mother; prov:qualifiedDelegation [ a prov:Delegation; prov:entity :mother; :foo :bar ]."@en ;
  rdfs:isDefinedBy <http://www.w3.org/ns/prov-o#> ;
  rdfs:label "Delegation" ;
  rdfs:subClassOf prov:AgentInfluence ;
  prov:category "qualified" ;
  prov:component "agents-responsibility" ;
  prov:definition """Delegation is the assignment of authority and responsibility to an agent (by itself or by another agent) to carry out a specific activity as a delegate or representative, while the agent it acts on behalf of retains some responsibility for the outcome of the delegated work.

For example, a student acted on behalf of his supervisor, who acted on behalf of the department chair, who acted on behalf of the university; all those agents are responsible in some way for the activity that took place but we do not say explicitly who bears responsibility and to what degree."""@en ;
  prov:dm "http://www.w3.org/TR/2013/REC-prov-dm-20130430/#term-delegation"^^xsd:anyURI ;
  prov:n "http://www.w3.org/TR/2013/REC-prov-n-20130430/#expression-delegation"^^xsd:anyURI ;
  prov:unqualifiedForm prov:actedOnBehalfOf ;
.
prov:Derivation
  rdf:type owl:Class ;
  rdfs:comment "An instance of prov:Derivation provides additional descriptions about the binary prov:wasDerivedFrom relation from some derived prov:Entity to another prov:Entity from which it was derived. For example, :chewed_bubble_gum prov:wasDerivedFrom :unwrapped_bubble_gum; prov:qualifiedDerivation [ a prov:Derivation; prov:entity :unwrapped_bubble_gum; :foo :bar ]."@en ;
  rdfs:comment "The more specific forms of prov:Derivation (i.e., prov:Revision, prov:Quotation, prov:PrimarySource) should be asserted if they apply."@en ;
  rdfs:isDefinedBy <http://www.w3.org/ns/prov-o#> ;
  rdfs:label "Derivation" ;
  rdfs:subClassOf prov:EntityInfluence ;
  prov:category "qualified" ;
  prov:component "derivations" ;
  prov:constraints "http://www.w3.org/TR/2013/REC-prov-constraints-20130430/#prov-dm-constraints-fig"^^xsd:anyURI ;
  prov:definition "A derivation is a transformation of an entity into another, an update of an entity resulting in a new one, or the construction of a new entity based on a pre-existing entity."@en ;
  prov:dm "http://www.w3.org/TR/2013/REC-prov-dm-20130430/#term-Derivation"^^xsd:anyURI ;
  prov:n "http://www.w3.org/TR/2013/REC-prov-n-20130430/#Derivation-Relation"^^xsd:anyURI ;
  prov:unqualifiedForm prov:wasDerivedFrom ;
.
prov:EmptyCollection
  rdf:type owl:Class ;
  rdf:type owl:NamedIndividual ;
  rdfs:isDefinedBy <http://www.w3.org/ns/prov-o#> ;
  rdfs:label "EmptyCollection"@en ;
  rdfs:subClassOf prov:Collection ;
  prov:category "expanded" ;
  prov:component "collections" ;
  prov:definition "An empty collection is a collection without members."@en ;
.
prov:End
  rdf:type owl:Class ;
  rdfs:comment "An instance of prov:End provides additional descriptions about the binary prov:wasEndedBy relation from some ended prov:Activity to an prov:Entity that ended it. For example, :ball_game prov:wasEndedBy :buzzer; prov:qualifiedEnd [ a prov:End; prov:entity :buzzer; :foo :bar; prov:atTime '2012-03-09T08:05:08-05:00'^^xsd:dateTime ]."@en ;
  rdfs:isDefinedBy <http://www.w3.org/ns/prov-o#> ;
  rdfs:label "End" ;
  rdfs:subClassOf prov:EntityInfluence ;
  rdfs:subClassOf prov:InstantaneousEvent ;
  prov:category "qualified" ;
  prov:component "entities-activities" ;
  prov:constraints "http://www.w3.org/TR/2013/REC-prov-constraints-20130430/#prov-dm-constraints-fig"^^xsd:anyURI ;
  prov:definition "End is when an activity is deemed to have been ended by an entity, known as trigger. The activity no longer exists after its end. Any usage, generation, or invalidation involving an activity precedes the activity's end. An end may refer to a trigger entity that terminated the activity, or to an activity, known as ender that generated the trigger."@en ;
  prov:dm "http://www.w3.org/TR/2013/REC-prov-dm-20130430/#term-End"^^xsd:anyURI ;
  prov:n "http://www.w3.org/TR/2013/REC-prov-n-20130430/#expression-End"^^xsd:anyURI ;
  prov:unqualifiedForm prov:wasEndedBy ;
.
prov:Entity
  rdf:type owl:Class ;
  rdfs:isDefinedBy <http://www.w3.org/ns/prov-o#> ;
  rdfs:label "Entity" ;
  rdfs:subClassOf owl:Thing ;
  owl:disjointWith prov:InstantaneousEvent ;
  prov:category "starting-point" ;
  prov:component "entities-activities" ;
  prov:constraints "http://www.w3.org/TR/2013/REC-prov-constraints-20130430/#prov-dm-constraints-fig"^^xsd:anyURI ;
  prov:definition "An entity is a physical, digital, conceptual, or other kind of thing with some fixed aspects; entities may be real or imaginary. "@en ;
  prov:dm "http://www.w3.org/TR/2013/REC-prov-dm-20130430/#term-entity"^^xsd:anyURI ;
  prov:n "http://www.w3.org/TR/2013/REC-prov-n-20130430/#expression-Entity"^^xsd:anyURI ;
.
prov:EntityInfluence
  rdf:type owl:Class ;
  rdfs:comment "EntityInfluence provides additional descriptions of an Entity's binary influence upon any other kind of resource. Instances of EntityInfluence use the prov:entity property to cite the influencing Entity."@en ;
  rdfs:comment "It is not recommended that the type EntityInfluence be asserted without also asserting one of its more specific subclasses."@en ;
  rdfs:isDefinedBy <http://www.w3.org/ns/prov-o#> ;
  rdfs:label "EntityInfluence" ;
  rdfs:seeAlso prov:entity ;
  rdfs:subClassOf prov:Influence ;
  prov:category "qualified" ;
  prov:editorsDefinition "EntityInfluence is the capacity of an entity to have an effect on the character, development, or behavior of another by means of usage, start, end, derivation, or other. "@en ;
.
prov:Generation
  rdf:type owl:Class ;
  rdfs:comment "An instance of prov:Generation provides additional descriptions about the binary prov:wasGeneratedBy relation from a generated prov:Entity to the prov:Activity that generated it. For example, :cake prov:wasGeneratedBy :baking; prov:qualifiedGeneration [ a prov:Generation; prov:activity :baking; :foo :bar ]."@en ;
  rdfs:isDefinedBy <http://www.w3.org/ns/prov-o#> ;
  rdfs:label "Generation" ;
  rdfs:subClassOf prov:ActivityInfluence ;
  rdfs:subClassOf prov:InstantaneousEvent ;
  prov:category "qualified" ;
  prov:component "entities-activities" ;
  prov:constraints "http://www.w3.org/TR/2013/REC-prov-constraints-20130430/#prov-dm-constraints-fig"^^xsd:anyURI ;
  prov:definition "Generation is the completion of production of a new entity by an activity. This entity did not exist before generation and becomes available for usage after this generation."@en ;
  prov:dm "http://www.w3.org/TR/2013/REC-prov-dm-20130430/#term-Generation"^^xsd:anyURI ;
  prov:n "http://www.w3.org/TR/2013/REC-prov-n-20130430/#expression-Generation"^^xsd:anyURI ;
  prov:unqualifiedForm prov:wasGeneratedBy ;
.
prov:Influence
  rdf:type owl:Class ;
  rdfs:comment "An instance of prov:Influence provides additional descriptions about the binary prov:wasInfluencedBy relation from some influenced Activity, Entity, or Agent to the influencing Activity, Entity, or Agent. For example, :stomach_ache prov:wasInfluencedBy :spoon; prov:qualifiedInfluence [ a prov:Influence; prov:entity :spoon; :foo :bar ] . Because prov:Influence is a broad relation, the more specific relations (Communication, Delegation, End, etc.) should be used when applicable."@en ;
  rdfs:comment "Because prov:Influence is a broad relation, its most specific subclasses (e.g. prov:Communication, prov:Delegation, prov:End, prov:Revision, etc.) should be used when applicable."@en ;
  rdfs:isDefinedBy <http://www.w3.org/ns/prov-o#> ;
  rdfs:label "Influence" ;
  rdfs:subClassOf owl:Thing ;
  prov:category "qualified" ;
  prov:component "derivations" ;
  prov:definition "Influence is the capacity of an entity, activity, or agent to have an effect on the character, development, or behavior of another by means of usage, start, end, generation, invalidation, communication, derivation, attribution, association, or delegation."@en ;
  prov:dm "http://www.w3.org/TR/2013/REC-prov-dm-20130430/#term-influence"^^xsd:anyURI ;
  prov:n "http://www.w3.org/TR/2013/REC-prov-n-20130430/#expression-influence"^^xsd:anyURI ;
  prov:unqualifiedForm prov:wasInfluencedBy ;
.
prov:InstantaneousEvent
  rdf:type owl:Class ;
  rdfs:comment "An instantaneous event, or event for short, happens in the world and marks a change in the world, in its activities and in its entities. The term 'event' is commonly used in process algebra with a similar meaning. Events represent communications or interactions; they are assumed to be atomic and instantaneous."@en ;
  rdfs:isDefinedBy <http://www.w3.org/ns/prov-o#> ;
  rdfs:label "InstantaneousEvent" ;
  rdfs:subClassOf owl:Thing ;
  prov:category "qualified" ;
  prov:component "entities-activities" ;
  prov:constraints "http://www.w3.org/TR/2013/REC-prov-constraints-20130430/#dfn-event"^^xsd:anyURI ;
  prov:definition "The PROV data model is implicitly based on a notion of instantaneous events (or just events), that mark transitions in the world. Events include generation, usage, or invalidation of entities, as well as starting or ending of activities. This notion of event is not first-class in the data model, but it is useful for explaining its other concepts and its semantics."@en ;
.
prov:Invalidation
  rdf:type owl:Class ;
  rdfs:comment "An instance of prov:Invalidation provides additional descriptions about the binary prov:wasInvalidatedBy relation from an invalidated prov:Entity to the prov:Activity that invalidated it. For example, :uncracked_egg prov:wasInvalidatedBy :baking; prov:qualifiedInvalidation [ a prov:Invalidation; prov:activity :baking; :foo :bar ]."@en ;
  rdfs:isDefinedBy <http://www.w3.org/ns/prov-o#> ;
  rdfs:label "Invalidation" ;
  rdfs:subClassOf prov:ActivityInfluence ;
  rdfs:subClassOf prov:InstantaneousEvent ;
  prov:category "qualified" ;
  prov:component "entities-activities" ;
  prov:constraints "http://www.w3.org/TR/2013/REC-prov-constraints-20130430/#prov-dm-constraints-fig"^^xsd:anyURI ;
  prov:definition "Invalidation is the start of the destruction, cessation, or expiry of an existing entity by an activity. The entity is no longer available for use (or further invalidation) after invalidation. Any generation or usage of an entity precedes its invalidation." ;
  prov:dm "http://www.w3.org/TR/2013/REC-prov-dm-20130430/#term-Invalidation"^^xsd:anyURI ;
  prov:n "http://www.w3.org/TR/2013/REC-prov-n-20130430/#expression-Invalidation"^^xsd:anyURI ;
  prov:unqualifiedForm prov:wasInvalidatedBy ;
.
prov:Location
  rdf:type owl:Class ;
  rdfs:isDefinedBy <http://www.w3.org/ns/prov-o#> ;
  rdfs:label "Location" ;
  rdfs:seeAlso prov:atLocation ;
  rdfs:subClassOf owl:Thing ;
  prov:category "expanded" ;
  prov:definition "A location can be an identifiable geographic place (ISO 19112), but it can also be a non-geographic place such as a directory, row, or column. As such, there are numerous ways in which location can be expressed, such as by a coordinate, address, landmark, and so forth."@en ;
  prov:dm "http://www.w3.org/TR/2013/REC-prov-dm-20130430/#term-attribute-location"^^xsd:anyURI ;
  prov:n "http://www.w3.org/TR/2013/REC-prov-n-20130430/#expression-attribute"^^xsd:anyURI ;
.
prov:Organization
  rdf:type owl:Class ;
  rdfs:isDefinedBy <http://www.w3.org/ns/prov-o#> ;
  rdfs:label "Organization" ;
  rdfs:subClassOf prov:Agent ;
  prov:category "expanded" ;
  prov:component "agents-responsibility" ;
  prov:definition "An organization is a social or legal institution such as a company, society, etc." ;
  prov:dm "http://www.w3.org/TR/2013/REC-prov-dm-20130430/#term-agent"^^xsd:anyURI ;
  prov:n "http://www.w3.org/TR/2013/REC-prov-n-20130430/#expression-types"^^xsd:anyURI ;
.
prov:Person
  rdf:type owl:Class ;
  rdfs:isDefinedBy <http://www.w3.org/ns/prov-o#> ;
  rdfs:label "Person" ;
  rdfs:subClassOf prov:Agent ;
  prov:category "expanded" ;
  prov:component "agents-responsibility" ;
  prov:definition "Person agents are people."@en ;
  prov:dm "http://www.w3.org/TR/2013/REC-prov-dm-20130430/#term-agent"^^xsd:anyURI ;
  prov:n "http://www.w3.org/TR/2013/REC-prov-n-20130430/#expression-types"^^xsd:anyURI ;
.
prov:Plan
  rdf:type owl:Class ;
  rdfs:comment "There exist no prescriptive requirement on the nature of plans, their representation, the actions or steps they consist of, or their intended goals. Since plans may evolve over time, it may become necessary to track their provenance, so plans themselves are entities. Representing the plan explicitly in the provenance can be useful for various tasks: for example, to validate the execution as represented in the provenance record, to manage expectation failures, or to provide explanations."@en ;
  rdfs:isDefinedBy <http://www.w3.org/ns/prov-o#> ;
  rdfs:label "Plan" ;
  rdfs:subClassOf prov:Entity ;
  prov:category "expanded" ;
  prov:category "qualified" ;
  prov:component "agents-responsibility" ;
  prov:definition "A plan is an entity that represents a set of actions or steps intended by one or more agents to achieve some goals." ;
  prov:dm "http://www.w3.org/TR/2013/REC-prov-dm-20130430/#term-Association"^^xsd:anyURI ;
  prov:n "http://www.w3.org/TR/2013/REC-prov-n-20130430/#expression-Association"^^xsd:anyURI ;
.
prov:PrimarySource
  rdf:type owl:Class ;
  rdfs:comment "An instance of prov:PrimarySource provides additional descriptions about the binary prov:hadPrimarySource relation from some secondary prov:Entity to an earlier, primary prov:Entity. For example, :blog prov:hadPrimarySource :newsArticle; prov:qualifiedPrimarySource [ a prov:PrimarySource; prov:entity :newsArticle; :foo :bar ] ."@en ;
  rdfs:isDefinedBy <http://www.w3.org/ns/prov-o#> ;
  rdfs:label "PrimarySource" ;
  rdfs:subClassOf prov:Derivation ;
  prov:category "qualified" ;
  prov:component "derivations" ;
  prov:definition """A primary source for a topic refers to something produced by some agent with direct experience and knowledge about the topic, at the time of the topic's study, without benefit from hindsight.

Because of the directness of primary sources, they 'speak for themselves' in ways that cannot be captured through the filter of secondary sources. As such, it is important for secondary sources to reference those primary sources from which they were derived, so that their reliability can be investigated.

A primary source relation is a particular case of derivation of secondary materials from their primary sources. It is recognized that the determination of primary sources can be up to interpretation, and should be done according to conventions accepted within the application's domain."""@en ;
  prov:dm "http://www.w3.org/TR/2013/REC-prov-dm-20130430/#term-primary-source"^^xsd:anyURI ;
  prov:n "http://www.w3.org/TR/2013/REC-prov-n-20130430/#expression-original-source"^^xsd:anyURI ;
  prov:unqualifiedForm prov:hadPrimarySource ;
.
prov:Quotation
  rdf:type owl:Class ;
  rdfs:comment "An instance of prov:Quotation provides additional descriptions about the binary prov:wasQuotedFrom relation from some taken prov:Entity from an earlier, larger prov:Entity. For example, :here_is_looking_at_you_kid prov:wasQuotedFrom :casablanca_script; prov:qualifiedQuotation [ a prov:Quotation; prov:entity :casablanca_script; :foo :bar ]."@en ;
  rdfs:isDefinedBy <http://www.w3.org/ns/prov-o#> ;
  rdfs:label "Quotation" ;
  rdfs:subClassOf prov:Derivation ;
  prov:category "qualified" ;
  prov:component "derivations" ;
  prov:definition "A quotation is the repeat of (some or all of) an entity, such as text or image, by someone who may or may not be its original author. Quotation is a particular case of derivation."@en ;
  prov:dm "http://www.w3.org/TR/2013/REC-prov-dm-20130430/#term-quotation"^^xsd:anyURI ;
  prov:n "http://www.w3.org/TR/2013/REC-prov-n-20130430/#expression-quotation"^^xsd:anyURI ;
  prov:unqualifiedForm prov:wasQuotedFrom ;
.
prov:Revision
  rdf:type owl:Class ;
  rdfs:comment "An instance of prov:Revision provides additional descriptions about the binary prov:wasRevisionOf relation from some newer prov:Entity to an earlier prov:Entity. For example, :draft_2 prov:wasRevisionOf :draft_1; prov:qualifiedRevision [ a prov:Revision; prov:entity :draft_1; :foo :bar ]."@en ;
  rdfs:isDefinedBy <http://www.w3.org/ns/prov-o#> ;
  rdfs:label "Revision" ;
  rdfs:subClassOf prov:Derivation ;
  prov:category "qualified" ;
  prov:component "derivations" ;
  prov:definition "A revision is a derivation for which the resulting entity is a revised version of some original. The implication here is that the resulting entity contains substantial content from the original. Revision is a particular case of derivation."@en ;
  prov:dm "http://www.w3.org/TR/2013/REC-prov-dm-20130430/#term-revision"^^xsd:anyURI ;
  prov:n "http://www.w3.org/TR/2013/REC-prov-n-20130430/#expression-Revision"^^xsd:anyURI ;
  prov:unqualifiedForm prov:wasRevisionOf ;
.
prov:Role
  rdf:type owl:Class ;
  rdfs:isDefinedBy <http://www.w3.org/ns/prov-o#> ;
  rdfs:label "Role" ;
  rdfs:seeAlso prov:hadRole ;
  rdfs:subClassOf owl:Thing ;
  prov:category "qualified" ;
  prov:component "agents-responsibility" ;
  prov:definition "A role is the function of an entity or agent with respect to an activity, in the context of a usage, generation, invalidation, association, start, and end."@en ;
  prov:dm "http://www.w3.org/TR/2013/REC-prov-dm-20130430/#term-attribute-role"^^xsd:anyURI ;
  prov:n "http://www.w3.org/TR/2013/REC-prov-n-20130430/#expression-attribute"^^xsd:anyURI ;
.
prov:SoftwareAgent
  rdf:type owl:Class ;
  rdfs:isDefinedBy <http://www.w3.org/ns/prov-o#> ;
  rdfs:label "SoftwareAgent" ;
  rdfs:subClassOf prov:Agent ;
  prov:category "expanded" ;
  prov:component "agents-responsibility" ;
  prov:definition "A software agent is running software."@en ;
  prov:dm "http://www.w3.org/TR/2013/REC-prov-dm-20130430/#term-agent"^^xsd:anyURI ;
  prov:n "http://www.w3.org/TR/2013/REC-prov-n-20130430/#expression-types"^^xsd:anyURI ;
.
prov:Start
  rdf:type owl:Class ;
  rdfs:comment "An instance of prov:Start provides additional descriptions about the binary prov:wasStartedBy relation from some started prov:Activity to an prov:Entity that started it. For example, :foot_race prov:wasStartedBy :bang; prov:qualifiedStart [ a prov:Start; prov:entity :bang; :foo :bar; prov:atTime '2012-03-09T08:05:08-05:00'^^xsd:dateTime ] ."@en ;
  rdfs:isDefinedBy <http://www.w3.org/ns/prov-o#> ;
  rdfs:label "Start" ;
  rdfs:subClassOf prov:EntityInfluence ;
  rdfs:subClassOf prov:InstantaneousEvent ;
  prov:category "qualified" ;
  prov:component "entities-activities" ;
  prov:constraints "http://www.w3.org/TR/2013/REC-prov-constraints-20130430/#prov-dm-constraints-fig"^^xsd:anyURI ;
  prov:definition "Start is when an activity is deemed to have been started by an entity, known as trigger. The activity did not exist before its start. Any usage, generation, or invalidation involving an activity follows the activity's start. A start may refer to a trigger entity that set off the activity, or to an activity, known as starter, that generated the trigger."@en ;
  prov:dm "http://www.w3.org/TR/2013/REC-prov-dm-20130430/#term-Start"^^xsd:anyURI ;
  prov:n "http://www.w3.org/TR/2013/REC-prov-n-20130430/#expression-Start"^^xsd:anyURI ;
  prov:unqualifiedForm prov:wasStartedBy ;
.
prov:Usage
  rdf:type owl:Class ;
  rdfs:comment "An instance of prov:Usage provides additional descriptions about the binary prov:used relation from some prov:Activity to an prov:Entity that it used. For example, :keynote prov:used :podium; prov:qualifiedUsage [ a prov:Usage; prov:entity :podium; :foo :bar ]."@en ;
  rdfs:isDefinedBy <http://www.w3.org/ns/prov-o#> ;
  rdfs:label "Usage" ;
  rdfs:subClassOf prov:EntityInfluence ;
  rdfs:subClassOf prov:InstantaneousEvent ;
  prov:category "qualified" ;
  prov:component "entities-activities" ;
  prov:constraints "http://www.w3.org/TR/2013/REC-prov-constraints-20130430/#prov-dm-constraints-fig"^^xsd:anyURI ;
  prov:definition "Usage is the beginning of utilizing an entity by an activity. Before usage, the activity had not begun to utilize this entity and could not have been affected by the entity."@en ;
  prov:dm "http://www.w3.org/TR/2013/REC-prov-dm-20130430/#term-Usage"^^xsd:anyURI ;
  prov:n "http://www.w3.org/TR/2013/REC-prov-n-20130430/#expression-Usage"^^xsd:anyURI ;
  prov:unqualifiedForm prov:used ;
.
prov:actedOnBehalfOf
  rdf:type owl:ObjectProperty ;
  rdfs:comment "An object property to express the accountability of an agent towards another agent. The subordinate agent acted on behalf of the responsible agent in an actual activity. "@en ;
  rdfs:domain prov:Agent ;
  rdfs:isDefinedBy <http://www.w3.org/ns/prov-o#> ;
  rdfs:label "actedOnBehalfOf" ;
  rdfs:range prov:Agent ;
  rdfs:subPropertyOf prov:wasInfluencedBy ;
  owl:propertyChainAxiom (
      prov:qualifiedDelegation
      prov:agent
    ) ;
  prov:category "starting-point" ;
  prov:component "agents-responsibility" ;
  prov:inverse "hadDelegate" ;
  prov:qualifiedForm prov:Delegation ;
  prov:qualifiedForm prov:qualifiedDelegation ;
.
prov:activity
  rdf:type owl:ObjectProperty ;
  rdfs:domain prov:ActivityInfluence ;
  rdfs:isDefinedBy <http://www.w3.org/ns/prov-o#> ;
  rdfs:label "activity" ;
  rdfs:range prov:Activity ;
  rdfs:subPropertyOf prov:influencer ;
  prov:category "qualified" ;
  prov:editorialNote "This property behaves in spirit like rdf:object; it references the object of a prov:wasInfluencedBy triple."@en ;
  prov:editorsDefinition "The prov:activity property references an prov:Activity which influenced a resource. This property applies to an prov:ActivityInfluence, which is given by a subproperty of prov:qualifiedInfluence from the influenced prov:Entity, prov:Activity or prov:Agent." ;
  prov:inverse "activityOfInfluence" ;
.
prov:agent
  rdf:type owl:ObjectProperty ;
  rdfs:domain prov:AgentInfluence ;
  rdfs:isDefinedBy <http://www.w3.org/ns/prov-o#> ;
  rdfs:label "agent" ;
  rdfs:range prov:Agent ;
  rdfs:subPropertyOf prov:influencer ;
  prov:category "qualified" ;
  prov:editorialNote "This property behaves in spirit like rdf:object; it references the object of a prov:wasInfluencedBy triple."@en ;
  prov:editorsDefinition "The prov:agent property references an prov:Agent which influenced a resource. This property applies to an prov:AgentInfluence, which is given by a subproperty of prov:qualifiedInfluence from the influenced prov:Entity, prov:Activity or prov:Agent."@en ;
  prov:inverse "agentOfInfluence" ;
.
prov:alternateOf
  rdf:type owl:ObjectProperty ;
  rdfs:domain prov:Entity ;
  rdfs:isDefinedBy <http://www.w3.org/ns/prov-o#> ;
  rdfs:label "alternateOf" ;
  rdfs:range prov:Entity ;
  rdfs:seeAlso prov:specializationOf ;
  prov:category "expanded" ;
  prov:component "alternate" ;
  prov:constraints "http://www.w3.org/TR/2013/REC-prov-constraints-20130430/#prov-dm-constraints-fig"^^xsd:anyURI ;
  prov:definition "Two alternate entities present aspects of the same thing. These aspects may be the same or different, and the alternate entities may or may not overlap in time."@en ;
  prov:dm "http://www.w3.org/TR/2013/REC-prov-dm-20130430/#term-alternate"^^xsd:anyURI ;
  prov:inverse "alternateOf" ;
  prov:n "http://www.w3.org/TR/2013/REC-prov-n-20130430/#expression-alternate"^^xsd:anyURI ;
.
prov:aq
  rdf:type owl:AnnotationProperty ;
  rdfs:isDefinedBy <http://www.w3.org/ns/prov-o#> ;
  rdfs:subPropertyOf rdfs:seeAlso ;
.
prov:atLocation
  rdf:type owl:ObjectProperty ;
  rdfs:comment "The Location of any resource."@en ;
  rdfs:comment "This property has multiple RDFS domains to suit multiple OWL Profiles. See <a href=\"#owl-profile\">PROV-O OWL Profile</a>." ;
  rdfs:domain [
      rdf:type owl:Class ;
      owl:unionOf (
          prov:Activity
          prov:Agent
          prov:Entity
          prov:InstantaneousEvent
        ) ;
    ] ;
  rdfs:isDefinedBy <http://www.w3.org/ns/prov-o#> ;
  rdfs:label "atLocation" ;
  rdfs:range prov:Location ;
  prov:category "expanded" ;
  prov:editorialNote "The naming of prov:atLocation parallels prov:atTime, and is not named prov:hadLocation to avoid conflicting with the convention that prov:had* properties are used on prov:Influence classes."@en ;
  prov:editorialNote "This property is not functional because the many values could be at a variety of granularies (In this building, in this room, in that chair)."@en ;
  prov:inverse "locationOf" ;
  prov:sharesDefinitionWith prov:Location ;
.
prov:atTime
  rdf:type owl:DatatypeProperty ;
  rdfs:comment "The time at which an InstantaneousEvent occurred, in the form of xsd:dateTime."@en ;
  rdfs:domain prov:InstantaneousEvent ;
  rdfs:isDefinedBy <http://www.w3.org/ns/prov-o#> ;
  rdfs:label "atTime" ;
  rdfs:range xsd:dateTime ;
  prov:category "qualified" ;
  prov:component "entities-activities" ;
  prov:sharesDefinitionWith prov:InstantaneousEvent ;
  prov:unqualifiedForm prov:endedAtTime ;
  prov:unqualifiedForm prov:generatedAtTime ;
  prov:unqualifiedForm prov:invalidatedAtTime ;
  prov:unqualifiedForm prov:startedAtTime ;
.
prov:category
  rdf:type owl:AnnotationProperty ;
  rdfs:comment "Classify prov-o terms into three categories, including 'starting-point', 'qualifed', and 'extended'. This classification is used by the prov-o html document to gently introduce prov-o terms to its users. "@en ;
  rdfs:isDefinedBy <http://www.w3.org/ns/prov-o#> ;
.
prov:component
  rdf:type owl:AnnotationProperty ;
  rdfs:comment "Classify prov-o terms into six components according to prov-dm, including 'agents-responsibility', 'alternate', 'annotations', 'collections', 'derivations', and 'entities-activities'. This classification is used so that readers of prov-o specification can find its correspondence with the prov-dm specification."@en ;
  rdfs:isDefinedBy <http://www.w3.org/ns/prov-o#> ;
.
prov:constraints
  rdf:type owl:AnnotationProperty ;
  rdfs:comment "A reference to the principal section of the PROV-CONSTRAINTS document that describes this concept."@en ;
  rdfs:isDefinedBy <http://www.w3.org/ns/prov-o#> ;
  rdfs:subPropertyOf rdfs:seeAlso ;
.
prov:definition
  rdf:type owl:AnnotationProperty ;
  rdfs:comment "A definition quoted from PROV-DM or PROV-CONSTRAINTS that describes the concept expressed with this OWL term."@en ;
  rdfs:isDefinedBy <http://www.w3.org/ns/prov-o#> ;
.
prov:dm
  rdf:type owl:AnnotationProperty ;
  rdfs:comment "A reference to the principal section of the PROV-DM document that describes this concept."@en ;
  rdfs:isDefinedBy <http://www.w3.org/ns/prov-o#> ;
  rdfs:subPropertyOf rdfs:seeAlso ;
.
prov:editorialNote
  rdf:type owl:AnnotationProperty ;
  rdfs:comment "A note by the OWL development team about how this term expresses the PROV-DM concept, or how it should be used in context of semantic web or linked data."@en ;
  rdfs:isDefinedBy <http://www.w3.org/ns/prov-o#> ;
.
prov:editorsDefinition
  rdf:type owl:AnnotationProperty ;
  rdfs:comment "When the prov-o term does not have a definition drawn from prov-dm, and the prov-o editor provides one."@en ;
  rdfs:isDefinedBy <http://www.w3.org/ns/prov-o#> ;
  rdfs:subPropertyOf prov:definition ;
.
prov:endedAtTime
  rdf:type owl:DatatypeProperty ;
  rdfs:comment "The time at which an activity ended. See also prov:startedAtTime."@en ;
  rdfs:domain prov:Activity ;
  rdfs:isDefinedBy <http://www.w3.org/ns/prov-o#> ;
  rdfs:label "endedAtTime" ;
  rdfs:range xsd:dateTime ;
  prov:category "starting-point" ;
  prov:component "entities-activities" ;
  prov:editorialNote "It is the intent that the property chain holds: (prov:qualifiedEnd o prov:atTime) rdfs:subPropertyOf prov:endedAtTime."@en ;
  prov:qualifiedForm prov:End ;
  prov:qualifiedForm prov:atTime ;
.
prov:entity
  rdf:type owl:ObjectProperty ;
  rdfs:domain prov:EntityInfluence ;
  rdfs:isDefinedBy <http://www.w3.org/ns/prov-o#> ;
  rdfs:label "entity" ;
  rdfs:range prov:Entity ;
  rdfs:subPropertyOf prov:influencer ;
  prov:category "qualified" ;
  prov:editorialNote "This property behaves in spirit like rdf:object; it references the object of a prov:wasInfluencedBy triple."@en ;
  prov:editorsDefinition "The prov:entity property references an prov:Entity which influenced a resource. This property applies to an prov:EntityInfluence, which is given by a subproperty of prov:qualifiedInfluence from the influenced prov:Entity, prov:Activity or prov:Agent." ;
  prov:inverse "entityOfInfluence" ;
.
prov:generated
  rdf:type owl:ObjectProperty ;
  rdfs:domain prov:Activity ;
  rdfs:isDefinedBy <http://www.w3.org/ns/prov-o#> ;
  rdfs:label "generated" ;
  rdfs:range prov:Entity ;
  rdfs:subPropertyOf prov:influenced ;
  owl:inverseOf prov:wasGeneratedBy ;
  prov:category "expanded" ;
  prov:component "entities-activities" ;
  prov:editorialNote "prov:generated is one of few inverse property defined, to allow Activity-oriented assertions in addition to Entity-oriented assertions."@en ;
  prov:inverse "wasGeneratedBy" ;
  prov:sharesDefinitionWith prov:Generation ;
.
prov:generatedAtTime
  rdf:type owl:DatatypeProperty ;
  rdfs:comment "The time at which an entity was completely created and is available for use."@en ;
  rdfs:domain prov:Entity ;
  rdfs:isDefinedBy <http://www.w3.org/ns/prov-o#> ;
  rdfs:label "generatedAtTime" ;
  rdfs:range xsd:dateTime ;
  prov:category "expanded" ;
  prov:component "entities-activities" ;
  prov:editorialNote "It is the intent that the property chain holds: (prov:qualifiedGeneration o prov:atTime) rdfs:subPropertyOf prov:generatedAtTime."@en ;
  prov:qualifiedForm prov:Generation ;
  prov:qualifiedForm prov:atTime ;
.
prov:hadActivity
  rdf:type owl:ObjectProperty ;
  rdfs:comment "The _optional_ Activity of an Influence, which used, generated, invalidated, or was the responsibility of some Entity. This property is _not_ used by ActivityInfluence (use prov:activity instead)."@en ;
  rdfs:comment "This property has multiple RDFS domains to suit multiple OWL Profiles. See <a href=\"#owl-profile\">PROV-O OWL Profile</a>." ;
  rdfs:domain prov:Influence ;
  rdfs:domain [
      rdf:type owl:Class ;
      owl:unionOf (
          prov:Delegation
          prov:Derivation
          prov:End
          prov:Start
        ) ;
    ] ;
  rdfs:isDefinedBy <http://www.w3.org/ns/prov-o#> ;
  rdfs:label "hadActivity" ;
  rdfs:range prov:Activity ;
  prov:category "qualified" ;
  prov:component "derivations" ;
  prov:editorialNote "The multiple rdfs:domain assertions are intended. One is simpler and works for OWL-RL, the union is more specific but is not recognized by OWL-RL."@en ;
  prov:inverse "wasActivityOfInfluence" ;
  prov:sharesDefinitionWith prov:Activity ;
.
prov:hadGeneration
  rdf:type owl:ObjectProperty ;
  rdfs:comment "The _optional_ Generation involved in an Entity's Derivation."@en ;
  rdfs:domain prov:Derivation ;
  rdfs:isDefinedBy <http://www.w3.org/ns/prov-o#> ;
  rdfs:label "hadGeneration" ;
  rdfs:range prov:Generation ;
  prov:category "qualified" ;
  prov:component "derivations" ;
  prov:inverse "generatedAsDerivation" ;
  prov:sharesDefinitionWith prov:Generation ;
.
prov:hadMember
  rdf:type owl:ObjectProperty ;
  rdfs:domain prov:Collection ;
  rdfs:isDefinedBy <http://www.w3.org/ns/prov-o#> ;
  rdfs:label "hadMember" ;
  rdfs:range prov:Entity ;
  rdfs:subPropertyOf prov:wasInfluencedBy ;
  prov:category "expanded" ;
  prov:component "expanded" ;
  prov:inverse "wasMemberOf" ;
  prov:sharesDefinitionWith prov:Collection ;
.
prov:hadPlan
  rdf:type owl:ObjectProperty ;
  rdfs:comment "The _optional_ Plan adopted by an Agent in Association with some Activity. Plan specifications are out of the scope of this specification."@en ;
  rdfs:domain prov:Association ;
  rdfs:isDefinedBy <http://www.w3.org/ns/prov-o#> ;
  rdfs:label "hadPlan" ;
  rdfs:range prov:Plan ;
  prov:category "qualified" ;
  prov:component "agents-responsibility" ;
  prov:inverse "wasPlanOf" ;
  prov:sharesDefinitionWith prov:Plan ;
.
prov:hadPrimarySource
  rdf:type owl:ObjectProperty ;
  rdfs:domain prov:Entity ;
  rdfs:isDefinedBy <http://www.w3.org/ns/prov-o#> ;
  rdfs:label "hadPrimarySource" ;
  rdfs:range prov:Entity ;
  rdfs:subPropertyOf prov:wasDerivedFrom ;
  owl:propertyChainAxiom (
      prov:qualifiedPrimarySource
      prov:entity
    ) ;
  prov:category "expanded" ;
  prov:component "derivations" ;
  prov:inverse "wasPrimarySourceOf" ;
  prov:qualifiedForm prov:PrimarySource ;
  prov:qualifiedForm prov:qualifiedPrimarySource ;
.
prov:hadRole
  rdf:type owl:ObjectProperty ;
  rdfs:comment "The _optional_ Role that an Entity assumed in the context of an Activity. For example, :baking prov:used :spoon; prov:qualified [ a prov:Usage; prov:entity :spoon; prov:hadRole roles:mixing_implement ]."@en ;
  rdfs:comment "This property has multiple RDFS domains to suit multiple OWL Profiles. See <a href=\"#owl-profile\">PROV-O OWL Profile</a>." ;
  rdfs:domain prov:Influence ;
  rdfs:domain [
      rdf:type owl:Class ;
      owl:unionOf (
          prov:Association
          prov:InstantaneousEvent
        ) ;
    ] ;
  rdfs:isDefinedBy <http://www.w3.org/ns/prov-o#> ;
  rdfs:label "hadRole" ;
  rdfs:range prov:Role ;
  prov:category "qualified" ;
  prov:component "agents-responsibility" ;
  prov:editorsDefinition "prov:hadRole references the Role (i.e. the function of an entity with respect to an activity), in the context of an instantaneous usage, generation, association, start, and end."@en ;
  prov:inverse "wasRoleIn" ;
  prov:sharesDefinitionWith prov:Role ;
.
prov:hadUsage
  rdf:type owl:ObjectProperty ;
  rdfs:comment "The _optional_ Usage involved in an Entity's Derivation."@en ;
  rdfs:domain prov:Derivation ;
  rdfs:isDefinedBy <http://www.w3.org/ns/prov-o#> ;
  rdfs:label "hadUsage" ;
  rdfs:range prov:Usage ;
  prov:category "qualified" ;
  prov:component "derivations" ;
  prov:inverse "wasUsedInDerivation" ;
  prov:sharesDefinitionWith prov:Usage ;
.
prov:influenced
  rdf:type owl:ObjectProperty ;
  rdfs:isDefinedBy <http://www.w3.org/ns/prov-o#> ;
  rdfs:label "influenced" ;
  owl:inverseOf prov:wasInfluencedBy ;
  prov:category "expanded" ;
  prov:component "agents-responsibility" ;
  prov:inverse "wasInfluencedBy" ;
  prov:sharesDefinitionWith prov:Influence ;
.
prov:influencer
  rdf:type owl:ObjectProperty ;
  rdfs:comment "Subproperties of prov:influencer are used to cite the object of an unqualified PROV-O triple whose predicate is a subproperty of prov:wasInfluencedBy (e.g. prov:used, prov:wasGeneratedBy). prov:influencer is used much like rdf:object is used."@en ;
  rdfs:domain prov:Influence ;
  rdfs:isDefinedBy <http://www.w3.org/ns/prov-o#> ;
  rdfs:label "influencer" ;
  rdfs:range owl:Thing ;
  prov:category "qualified" ;
  prov:dm "http://www.w3.org/TR/2013/REC-prov-dm-20130430/#term-influence"^^xsd:anyURI ;
  prov:editorialNote "This property and its subproperties are used in the same way as the rdf:object property, i.e. to reference the object of an unqualified prov:wasInfluencedBy or prov:influenced triple."@en ;
  prov:editorsDefinition "This property is used as part of the qualified influence pattern. Subclasses of prov:Influence use these subproperties to reference the resource (Entity, Agent, or Activity) whose influence is being qualified."@en ;
  prov:inverse "hadInfluence" ;
.
prov:invalidated
  rdf:type owl:ObjectProperty ;
  rdfs:domain prov:Activity ;
  rdfs:isDefinedBy <http://www.w3.org/ns/prov-o#> ;
  rdfs:label "invalidated" ;
  rdfs:range prov:Entity ;
  rdfs:subPropertyOf prov:influenced ;
  owl:inverseOf prov:wasInvalidatedBy ;
  prov:category "expanded" ;
  prov:component "entities-activities" ;
  prov:editorialNote "prov:invalidated is one of few inverse property defined, to allow Activity-oriented assertions in addition to Entity-oriented assertions."@en ;
  prov:inverse "wasInvalidatedBy" ;
  prov:sharesDefinitionWith prov:Invalidation ;
.
prov:invalidatedAtTime
  rdf:type owl:DatatypeProperty ;
  rdfs:comment "The time at which an entity was invalidated (i.e., no longer usable)."@en ;
  rdfs:domain prov:Entity ;
  rdfs:isDefinedBy <http://www.w3.org/ns/prov-o#> ;
  rdfs:label "invalidatedAtTime" ;
  rdfs:range xsd:dateTime ;
  prov:category "expanded" ;
  prov:component "entities-activities" ;
  prov:editorialNote "It is the intent that the property chain holds: (prov:qualifiedInvalidation o prov:atTime) rdfs:subPropertyOf prov:invalidatedAtTime."@en ;
  prov:qualifiedForm prov:Invalidation ;
  prov:qualifiedForm prov:atTime ;
.
prov:inverse
  rdf:type owl:AnnotationProperty ;
  rdfs:comment "PROV-O does not define all property inverses. The directionalities defined in PROV-O should be given preference over those not defined. However, if users wish to name the inverse of a PROV-O property, the local name given by prov:inverse should be used."@en ;
  rdfs:isDefinedBy <http://www.w3.org/ns/prov-o#> ;
  rdfs:seeAlso <http://www.w3.org/TR/prov-o/#names-of-inverse-properties> ;
.
prov:n
  rdf:type owl:AnnotationProperty ;
  rdfs:comment "A reference to the principal section of the PROV-DM document that describes this concept."@en ;
  rdfs:isDefinedBy <http://www.w3.org/ns/prov-o#> ;
  rdfs:subPropertyOf rdfs:seeAlso ;
.
prov:order
  rdf:type owl:AnnotationProperty ;
  rdfs:comment "The position that this OWL term should be listed within documentation. The scope of the documentation (e.g., among all terms, among terms within a prov:category, among properties applying to a particular class, etc.) is unspecified."@en ;
  rdfs:isDefinedBy <http://www.w3.org/ns/prov-o#> ;
.
prov:qualifiedAssociation
  rdf:type owl:ObjectProperty ;
  rdfs:comment "If this Activity prov:wasAssociatedWith Agent :ag, then it can qualify the Association using prov:qualifiedAssociation [ a prov:Association;  prov:agent :ag; :foo :bar ]."@en ;
  rdfs:domain prov:Activity ;
  rdfs:isDefinedBy <http://www.w3.org/ns/prov-o#> ;
  rdfs:label "qualifiedAssociation" ;
  rdfs:range prov:Association ;
  rdfs:subPropertyOf prov:qualifiedInfluence ;
  prov:category "qualified" ;
  prov:component "agents-responsibility" ;
  prov:inverse "qualifiedAssociationOf" ;
  prov:sharesDefinitionWith prov:Association ;
  prov:unqualifiedForm prov:wasAssociatedWith ;
.
prov:qualifiedAttribution
  rdf:type owl:ObjectProperty ;
  rdfs:comment "If this Entity prov:wasAttributedTo Agent :ag, then it can qualify how it was influenced using prov:qualifiedAttribution [ a prov:Attribution;  prov:agent :ag; :foo :bar ]."@en ;
  rdfs:domain prov:Entity ;
  rdfs:isDefinedBy <http://www.w3.org/ns/prov-o#> ;
  rdfs:label "qualifiedAttribution" ;
  rdfs:range prov:Attribution ;
  rdfs:subPropertyOf prov:qualifiedInfluence ;
  prov:category "qualified" ;
  prov:component "agents-responsibility" ;
  prov:inverse "qualifiedAttributionOf" ;
  prov:sharesDefinitionWith prov:Attribution ;
  prov:unqualifiedForm prov:wasAttributedTo ;
.
prov:qualifiedCommunication
  rdf:type owl:ObjectProperty ;
  rdfs:comment "If this Activity prov:wasInformedBy Activity :a, then it can qualify how it was influenced using prov:qualifiedCommunication [ a prov:Communication;  prov:activity :a; :foo :bar ]."@en ;
  rdfs:domain prov:Activity ;
  rdfs:isDefinedBy <http://www.w3.org/ns/prov-o#> ;
  rdfs:label "qualifiedCommunication" ;
  rdfs:range prov:Communication ;
  rdfs:subPropertyOf prov:qualifiedInfluence ;
  prov:category "qualified" ;
  prov:component "entities-activities" ;
  prov:inverse "qualifiedCommunicationOf" ;
  prov:qualifiedForm prov:Communication ;
  prov:sharesDefinitionWith prov:Communication ;
.
prov:qualifiedDelegation
  rdf:type owl:ObjectProperty ;
  rdfs:comment "If this Agent prov:actedOnBehalfOf Agent :ag, then it can qualify how with prov:qualifiedResponsibility [ a prov:Responsibility;  prov:agent :ag; :foo :bar ]."@en ;
  rdfs:domain prov:Agent ;
  rdfs:isDefinedBy <http://www.w3.org/ns/prov-o#> ;
  rdfs:label "qualifiedDelegation" ;
  rdfs:range prov:Delegation ;
  rdfs:subPropertyOf prov:qualifiedInfluence ;
  prov:category "qualified" ;
  prov:component "agents-responsibility" ;
  prov:inverse "qualifiedDelegationOf" ;
  prov:sharesDefinitionWith prov:Delegation ;
  prov:unqualifiedForm prov:actedOnBehalfOf ;
.
prov:qualifiedDerivation
  rdf:type owl:ObjectProperty ;
  rdfs:comment "If this Entity prov:wasDerivedFrom Entity :e, then it can qualify how it was derived using prov:qualifiedDerivation [ a prov:Derivation;  prov:entity :e; :foo :bar ]."@en ;
  rdfs:domain prov:Entity ;
  rdfs:isDefinedBy <http://www.w3.org/ns/prov-o#> ;
  rdfs:label "qualifiedDerivation" ;
  rdfs:range prov:Derivation ;
  rdfs:subPropertyOf prov:qualifiedInfluence ;
  prov:category "qualified" ;
  prov:component "derivations" ;
  prov:inverse "qualifiedDerivationOf" ;
  prov:sharesDefinitionWith prov:Derivation ;
  prov:unqualifiedForm prov:wasDerivedFrom ;
.
prov:qualifiedEnd
  rdf:type owl:ObjectProperty ;
  rdfs:comment "If this Activity prov:wasEndedBy Entity :e1, then it can qualify how it was ended using prov:qualifiedEnd [ a prov:End;  prov:entity :e1; :foo :bar ]."@en ;
  rdfs:domain prov:Activity ;
  rdfs:isDefinedBy <http://www.w3.org/ns/prov-o#> ;
  rdfs:label "qualifiedEnd" ;
  rdfs:range prov:End ;
  rdfs:subPropertyOf prov:qualifiedInfluence ;
  prov:category "qualified" ;
  prov:component "entities-activities" ;
  prov:inverse "qualifiedEndOf" ;
  prov:sharesDefinitionWith prov:End ;
  prov:unqualifiedForm prov:wasEndedBy ;
.
prov:qualifiedForm
  rdf:type owl:AnnotationProperty ;
  rdfs:comment """This annotation property links a subproperty of prov:wasInfluencedBy with the subclass of prov:Influence and the qualifying property that are used to qualify it. 

Example annotation:

    prov:wasGeneratedBy prov:qualifiedForm prov:qualifiedGeneration, prov:Generation .

Then this unqualified assertion:

    :entity1 prov:wasGeneratedBy :activity1 .

can be qualified by adding:

   :entity1 prov:qualifiedGeneration :entity1Gen .
   :entity1Gen 
       a prov:Generation, prov:Influence;
       prov:activity :activity1;
       :customValue 1337 .

Note how the value of the unqualified influence (prov:wasGeneratedBy :activity1) is mirrored as the value of the prov:activity (or prov:entity, or prov:agent) property on the influence class."""@en ;
  rdfs:isDefinedBy <http://www.w3.org/ns/prov-o#> ;
  rdfs:subPropertyOf rdfs:seeAlso ;
.
prov:qualifiedGeneration
  rdf:type owl:ObjectProperty ;
  rdfs:comment "If this Activity prov:generated Entity :e, then it can qualify how it performed the Generation using prov:qualifiedGeneration [ a prov:Generation;  prov:entity :e; :foo :bar ]."@en ;
  rdfs:domain prov:Entity ;
  rdfs:isDefinedBy <http://www.w3.org/ns/prov-o#> ;
  rdfs:label "qualifiedGeneration" ;
  rdfs:range prov:Generation ;
  rdfs:subPropertyOf prov:qualifiedInfluence ;
  prov:category "qualified" ;
  prov:component "entities-activities" ;
  prov:inverse "qualifiedGenerationOf" ;
  prov:sharesDefinitionWith prov:Generation ;
  prov:unqualifiedForm prov:wasGeneratedBy ;
.
prov:qualifiedInfluence
  rdf:type owl:ObjectProperty ;
  rdfs:comment "Because prov:qualifiedInfluence is a broad relation, the more specific relations (qualifiedCommunication, qualifiedDelegation, qualifiedEnd, etc.) should be used when applicable."@en ;
  rdfs:domain [
      rdf:type owl:Class ;
      owl:unionOf (
          prov:Activity
          prov:Agent
          prov:Entity
        ) ;
    ] ;
  rdfs:isDefinedBy <http://www.w3.org/ns/prov-o#> ;
  rdfs:label "qualifiedInfluence" ;
  rdfs:range prov:Influence ;
  prov:category "qualified" ;
  prov:component "derivations" ;
  prov:inverse "qualifiedInfluenceOf" ;
  prov:sharesDefinitionWith prov:Influence ;
  prov:unqualifiedForm prov:wasInfluencedBy ;
.
prov:qualifiedInvalidation
  rdf:type owl:ObjectProperty ;
  rdfs:comment "If this Entity prov:wasInvalidatedBy Activity :a, then it can qualify how it was invalidated using prov:qualifiedInvalidation [ a prov:Invalidation;  prov:activity :a; :foo :bar ]."@en ;
  rdfs:domain prov:Entity ;
  rdfs:isDefinedBy <http://www.w3.org/ns/prov-o#> ;
  rdfs:label "qualifiedInvalidation" ;
  rdfs:range prov:Invalidation ;
  rdfs:subPropertyOf prov:qualifiedInfluence ;
  prov:category "qualified" ;
  prov:component "entities-activities" ;
  prov:inverse "qualifiedInvalidationOf" ;
  prov:sharesDefinitionWith prov:Invalidation ;
  prov:unqualifiedForm prov:wasInvalidatedBy ;
.
prov:qualifiedPrimarySource
  rdf:type owl:ObjectProperty ;
  rdfs:comment "If this Entity prov:hadPrimarySource Entity :e, then it can qualify how using prov:qualifiedPrimarySource [ a prov:PrimarySource; prov:entity :e; :foo :bar ]."@en ;
  rdfs:domain prov:Entity ;
  rdfs:isDefinedBy <http://www.w3.org/ns/prov-o#> ;
  rdfs:label "qualifiedPrimarySource" ;
  rdfs:range prov:PrimarySource ;
  rdfs:subPropertyOf prov:qualifiedInfluence ;
  prov:category "qualified" ;
  prov:component "derivations" ;
  prov:inverse "qualifiedSourceOf" ;
  prov:sharesDefinitionWith prov:PrimarySource ;
  prov:unqualifiedForm prov:hadPrimarySource ;
.
prov:qualifiedQuotation
  rdf:type owl:ObjectProperty ;
  rdfs:comment "If this Entity prov:wasQuotedFrom Entity :e, then it can qualify how using prov:qualifiedQuotation [ a prov:Quotation;  prov:entity :e; :foo :bar ]."@en ;
  rdfs:domain prov:Entity ;
  rdfs:isDefinedBy <http://www.w3.org/ns/prov-o#> ;
  rdfs:label "qualifiedQuotation" ;
  rdfs:range prov:Quotation ;
  rdfs:subPropertyOf prov:qualifiedInfluence ;
  prov:category "qualified" ;
  prov:component "derivations" ;
  prov:inverse "qualifiedQuotationOf" ;
  prov:sharesDefinitionWith prov:Quotation ;
  prov:unqualifiedForm prov:wasQuotedFrom ;
.
prov:qualifiedRevision
  rdf:type owl:ObjectProperty ;
  rdfs:comment "If this Entity prov:wasRevisionOf Entity :e, then it can qualify how it was revised using prov:qualifiedRevision [ a prov:Revision;  prov:entity :e; :foo :bar ]."@en ;
  rdfs:domain prov:Entity ;
  rdfs:isDefinedBy <http://www.w3.org/ns/prov-o#> ;
  rdfs:label "qualifiedRevision" ;
  rdfs:range prov:Revision ;
  rdfs:subPropertyOf prov:qualifiedInfluence ;
  prov:category "qualified" ;
  prov:component "derivations" ;
  prov:inverse "revisedEntity" ;
  prov:sharesDefinitionWith prov:Revision ;
  prov:unqualifiedForm prov:wasRevisionOf ;
.
prov:qualifiedStart
  rdf:type owl:ObjectProperty ;
  rdfs:comment "If this Activity prov:wasStartedBy Entity :e1, then it can qualify how it was started using prov:qualifiedStart [ a prov:Start;  prov:entity :e1; :foo :bar ]."@en ;
  rdfs:domain prov:Activity ;
  rdfs:isDefinedBy <http://www.w3.org/ns/prov-o#> ;
  rdfs:label "qualifiedStart" ;
  rdfs:range prov:Start ;
  rdfs:subPropertyOf prov:qualifiedInfluence ;
  prov:category "qualified" ;
  prov:component "entities-activities" ;
  prov:inverse "qualifiedStartOf" ;
  prov:sharesDefinitionWith prov:Start ;
  prov:unqualifiedForm prov:wasStartedBy ;
.
prov:qualifiedUsage
  rdf:type owl:ObjectProperty ;
  rdfs:comment "If this Activity prov:used Entity :e, then it can qualify how it used it using prov:qualifiedUsage [ a prov:Usage; prov:entity :e; :foo :bar ]."@en ;
  rdfs:domain prov:Activity ;
  rdfs:isDefinedBy <http://www.w3.org/ns/prov-o#> ;
  rdfs:label "qualifiedUsage" ;
  rdfs:range prov:Usage ;
  rdfs:subPropertyOf prov:qualifiedInfluence ;
  prov:category "qualified" ;
  prov:component "entities-activities" ;
  prov:inverse "qualifiedUsingActivity" ;
  prov:sharesDefinitionWith prov:Usage ;
  prov:unqualifiedForm prov:used ;
.
prov:sharesDefinitionWith
  rdf:type owl:AnnotationProperty ;
  rdfs:isDefinedBy <http://www.w3.org/ns/prov-o#> ;
  rdfs:subPropertyOf rdfs:seeAlso ;
.
prov:specializationOf
  rdf:type owl:AnnotationProperty ;
  rdf:type owl:ObjectProperty ;
  rdfs:domain prov:Entity ;
  rdfs:isDefinedBy <http://www.w3.org/ns/prov-o#> ;
  rdfs:label "specializationOf" ;
  rdfs:range prov:Entity ;
  rdfs:seeAlso prov:alternateOf ;
  rdfs:subPropertyOf prov:alternateOf ;
  prov:category "expanded" ;
  prov:component "alternate" ;
  prov:constraints "http://www.w3.org/TR/2013/REC-prov-constraints-20130430/#prov-dm-constraints-fig"^^xsd:anyURI ;
  prov:definition "An entity that is a specialization of another shares all aspects of the latter, and additionally presents more specific aspects of the same thing as the latter. In particular, the lifetime of the entity being specialized contains that of any specialization. Examples of aspects include a time period, an abstraction, and a context associated with the entity."@en ;
  prov:dm "http://www.w3.org/TR/2013/REC-prov-dm-20130430/#term-specialization"^^xsd:anyURI ;
  prov:inverse "generalizationOf" ;
  prov:n "http://www.w3.org/TR/2013/REC-prov-n-20130430/#expression-specialization"^^xsd:anyURI ;
.
prov:startedAtTime
  rdf:type owl:DatatypeProperty ;
  rdfs:comment "The time at which an activity started. See also prov:endedAtTime."@en ;
  rdfs:domain prov:Activity ;
  rdfs:isDefinedBy <http://www.w3.org/ns/prov-o#> ;
  rdfs:label "startedAtTime" ;
  rdfs:range xsd:dateTime ;
  prov:category "starting-point" ;
  prov:component "entities-activities" ;
  prov:editorialNote "It is the intent that the property chain holds: (prov:qualifiedStart o prov:atTime) rdfs:subPropertyOf prov:startedAtTime."@en ;
  prov:qualifiedForm prov:Start ;
  prov:qualifiedForm prov:atTime ;
.
prov:todo
  rdf:type owl:AnnotationProperty ;
.
prov:unqualifiedForm
  rdf:type owl:AnnotationProperty ;
  rdfs:comment "Classes and properties used to qualify relationships are annotated with prov:unqualifiedForm to indicate the property used to assert an unqualified provenance relation."@en ;
  rdfs:isDefinedBy <http://www.w3.org/ns/prov-o#> ;
  rdfs:subPropertyOf rdfs:seeAlso ;
.
prov:used
  rdf:type owl:ObjectProperty ;
  rdfs:comment "A prov:Entity that was used by this prov:Activity. For example, :baking prov:used :spoon, :egg, :oven ."@en ;
  rdfs:domain prov:Activity ;
  rdfs:isDefinedBy <http://www.w3.org/ns/prov-o#> ;
  rdfs:label "used" ;
  rdfs:range prov:Entity ;
  rdfs:subPropertyOf prov:wasInfluencedBy ;
  owl:propertyChainAxiom (
      prov:qualifiedUsage
      prov:entity
    ) ;
  prov:category "starting-point" ;
  prov:component "entities-activities" ;
  prov:inverse "wasUsedBy" ;
  prov:qualifiedForm prov:Usage ;
  prov:qualifiedForm prov:qualifiedUsage ;
.
prov:value
  rdf:type owl:DatatypeProperty ;
  rdfs:domain prov:Entity ;
  rdfs:isDefinedBy <http://www.w3.org/ns/prov-o#> ;
  rdfs:label "value" ;
  prov:category "expanded" ;
  prov:component "entities-activities" ;
  prov:definition "Provides a value that is a direct representation of an entity."@en ;
  prov:dm "http://www.w3.org/TR/2013/REC-prov-dm-20130430/#term-attribute-value"^^xsd:anyURI ;
  prov:editorialNote "The editor's definition comes from http://www.w3.org/TR/rdf-primer/#rdfvalue" ;
  prov:editorialNote "This property serves the same purpose as rdf:value, but has been reintroduced to avoid some of the definitional ambiguity in the RDF specification (specifically, 'may be used in describing structured values')."@en ;
.
prov:wasAssociatedWith
  rdf:type owl:ObjectProperty ;
  rdfs:comment "An prov:Agent that had some (unspecified) responsibility for the occurrence of this prov:Activity."@en ;
  rdfs:domain prov:Activity ;
  rdfs:isDefinedBy <http://www.w3.org/ns/prov-o#> ;
  rdfs:label "wasAssociatedWith" ;
  rdfs:range prov:Agent ;
  rdfs:subPropertyOf prov:wasInfluencedBy ;
  owl:propertyChainAxiom (
      prov:qualifiedAssociation
      prov:agent
    ) ;
  prov:category "starting-point" ;
  prov:component "agents-responsibility" ;
  prov:inverse "wasAssociateFor" ;
  prov:qualifiedForm prov:Association ;
  prov:qualifiedForm prov:qualifiedAssociation ;
.
prov:wasAttributedTo
  rdf:type owl:ObjectProperty ;
  rdfs:comment "Attribution is the ascribing of an entity to an agent."@en ;
  rdfs:domain prov:Entity ;
  rdfs:isDefinedBy <http://www.w3.org/ns/prov-o#> ;
  rdfs:label "wasAttributedTo" ;
  rdfs:range prov:Agent ;
  rdfs:subPropertyOf prov:wasInfluencedBy ;
  owl:propertyChainAxiom (
      prov:qualifiedAttribution
      prov:agent
    ) ;
  prov:category "starting-point" ;
  prov:component "agents-responsibility" ;
  prov:definition "Attribution is the ascribing of an entity to an agent."@en ;
  prov:inverse "contributed" ;
  prov:qualifiedForm prov:Attribution ;
  prov:qualifiedForm prov:qualifiedAttribution ;
.
prov:wasDerivedFrom
  rdf:type owl:ObjectProperty ;
  rdfs:comment "The more specific subproperties of prov:wasDerivedFrom (i.e., prov:wasQuotedFrom, prov:wasRevisionOf, prov:hadPrimarySource) should be used when applicable."@en ;
  rdfs:domain prov:Entity ;
  rdfs:isDefinedBy <http://www.w3.org/ns/prov-o#> ;
  rdfs:label "wasDerivedFrom" ;
  rdfs:range prov:Entity ;
  rdfs:subPropertyOf prov:wasInfluencedBy ;
  owl:propertyChainAxiom (
      org:resultedFrom
      org:originalOrganization
    ) ;
  owl:propertyChainAxiom (
      prov:qualifiedDerivation
      prov:entity
    ) ;
  prov:category "starting-point" ;
  prov:component "derivations" ;
  prov:definition "A derivation is a transformation of an entity into another, an update of an entity resulting in a new one, or the construction of a new entity based on a pre-existing entity."@en ;
  prov:inverse "hadDerivation" ;
  prov:qualifiedForm prov:Derivation ;
  prov:qualifiedForm prov:qualifiedDerivation ;
.
prov:wasEndedBy
  rdf:type owl:ObjectProperty ;
  rdfs:comment "End is when an activity is deemed to have ended. An end may refer to an entity, known as trigger, that terminated the activity."@en ;
  rdfs:domain prov:Activity ;
  rdfs:isDefinedBy <http://www.w3.org/ns/prov-o#> ;
  rdfs:label "wasEndedBy" ;
  rdfs:range prov:Entity ;
  rdfs:subPropertyOf prov:wasInfluencedBy ;
  owl:propertyChainAxiom (
      prov:qualifiedEnd
      prov:entity
    ) ;
  prov:category "expanded" ;
  prov:component "entities-activities" ;
  prov:inverse "ended" ;
  prov:qualifiedForm prov:End ;
  prov:qualifiedForm prov:qualifiedEnd ;
.
prov:wasGeneratedBy
  rdf:type owl:ObjectProperty ;
  rdfs:domain prov:Entity ;
  rdfs:isDefinedBy <http://www.w3.org/ns/prov-o#> ;
  rdfs:label "wasGeneratedBy" ;
  rdfs:range prov:Activity ;
  rdfs:subPropertyOf prov:wasInfluencedBy ;
  owl:propertyChainAxiom (
      prov:qualifiedGeneration
      prov:activity
    ) ;
  prov:category "starting-point" ;
  prov:component "entities-activities" ;
  prov:inverse "generated" ;
  prov:qualifiedForm prov:Generation ;
  prov:qualifiedForm prov:qualifiedGeneration ;
.
prov:wasInfluencedBy
  rdf:type owl:ObjectProperty ;
  rdfs:comment "Because prov:wasInfluencedBy is a broad relation, its more specific subproperties (e.g. prov:wasInformedBy, prov:actedOnBehalfOf, prov:wasEndedBy, etc.) should be used when applicable."@en ;
  rdfs:comment "This property has multiple RDFS domains to suit multiple OWL Profiles. See <a href=\"#owl-profile\">PROV-O OWL Profile</a>." ;
  rdfs:domain [
      rdf:type owl:Class ;
      owl:unionOf (
          prov:Activity
          prov:Agent
          prov:Entity
        ) ;
    ] ;
  rdfs:isDefinedBy <http://www.w3.org/ns/prov-o#> ;
  rdfs:label "wasInfluencedBy" ;
  rdfs:range [
      rdf:type owl:Class ;
      owl:unionOf (
          prov:Activity
          prov:Agent
          prov:Entity
        ) ;
    ] ;
  prov:category "qualified" ;
  prov:component "agents-responsibility" ;
  prov:editorialNote """The sub-properties of prov:wasInfluencedBy can be elaborated in more detail using the Qualification Pattern. For example, the binary relation :baking prov:used :spoon can be qualified by asserting :baking prov:qualifiedUsage [ a prov:Usage; prov:entity :spoon; prov:atLocation :kitchen ] .

Subproperties of prov:wasInfluencedBy may also be asserted directly without being qualified.

prov:wasInfluencedBy should not be used without also using one of its subproperties. 
"""@en ;
  prov:inverse "influenced" ;
  prov:qualifiedForm prov:Influence ;
  prov:qualifiedForm prov:qualifiedInfluence ;
  prov:sharesDefinitionWith prov:Influence ;
.
prov:wasInformedBy
  rdf:type owl:ObjectProperty ;
  rdfs:comment "An activity a2 is dependent on or informed by another activity a1, by way of some unspecified entity that is generated by a1 and used by a2."@en ;
  rdfs:domain prov:Activity ;
  rdfs:isDefinedBy <http://www.w3.org/ns/prov-o#> ;
  rdfs:label "wasInformedBy" ;
  rdfs:range prov:Activity ;
  rdfs:subPropertyOf prov:wasInfluencedBy ;
  owl:propertyChainAxiom (
      prov:qualifiedCommunication
      prov:activity
    ) ;
  prov:category "starting-point" ;
  prov:component "entities-activities" ;
  prov:inverse "informed" ;
  prov:qualifiedForm prov:Communication ;
  prov:qualifiedForm prov:qualifiedCommunication ;
.
prov:wasInvalidatedBy
  rdf:type owl:ObjectProperty ;
  rdfs:domain prov:Entity ;
  rdfs:isDefinedBy <http://www.w3.org/ns/prov-o#> ;
  rdfs:label "wasInvalidatedBy" ;
  rdfs:range prov:Activity ;
  rdfs:subPropertyOf prov:wasInfluencedBy ;
  owl:propertyChainAxiom (
      prov:qualifiedInvalidation
      prov:activity
    ) ;
  prov:category "expanded" ;
  prov:component "entities-activities" ;
  prov:inverse "invalidated" ;
  prov:qualifiedForm prov:Invalidation ;
  prov:qualifiedForm prov:qualifiedInvalidation ;
.
prov:wasQuotedFrom
  rdf:type owl:ObjectProperty ;
  rdfs:comment "An entity is derived from an original entity by copying, or 'quoting', some or all of it."@en ;
  rdfs:domain prov:Entity ;
  rdfs:isDefinedBy <http://www.w3.org/ns/prov-o#> ;
  rdfs:label "wasQuotedFrom" ;
  rdfs:range prov:Entity ;
  rdfs:subPropertyOf prov:wasDerivedFrom ;
  owl:propertyChainAxiom (
      prov:qualifiedQuotation
      prov:entity
    ) ;
  prov:category "expanded" ;
  prov:component "derivations" ;
  prov:inverse "quotedAs" ;
  prov:qualifiedForm prov:Quotation ;
  prov:qualifiedForm prov:qualifiedQuotation ;
.
prov:wasRevisionOf
  rdf:type owl:AnnotationProperty ;
  rdf:type owl:ObjectProperty ;
  rdfs:comment "A revision is a derivation that revises an entity into a revised version."@en ;
  rdfs:domain prov:Entity ;
  rdfs:isDefinedBy <http://www.w3.org/ns/prov-o#> ;
  rdfs:label "wasRevisionOf" ;
  rdfs:range prov:Entity ;
  rdfs:subPropertyOf prov:wasDerivedFrom ;
  owl:propertyChainAxiom (
      prov:qualifiedRevision
      prov:entity
    ) ;
  prov:category "expanded" ;
  prov:component "derivations" ;
  prov:inverse "hadRevision" ;
  prov:qualifiedForm prov:Revision ;
  prov:qualifiedForm prov:qualifiedRevision ;
.
prov:wasStartedBy
  rdf:type owl:ObjectProperty ;
  rdfs:comment "Start is when an activity is deemed to have started. A start may refer to an entity, known as trigger, that initiated the activity."@en ;
  rdfs:domain prov:Activity ;
  rdfs:isDefinedBy <http://www.w3.org/ns/prov-o#> ;
  rdfs:label "wasStartedBy" ;
  rdfs:range prov:Entity ;
  rdfs:subPropertyOf prov:wasInfluencedBy ;
  owl:propertyChainAxiom (
      prov:qualifiedStart
      prov:entity
    ) ;
  prov:category "expanded" ;
  prov:component "entities-activities" ;
  prov:inverse "started" ;
  prov:qualifiedForm prov:Start ;
  prov:qualifiedForm prov:qualifiedStart ;
.
<http://www.w3.org/ns/prov-o#>
  rdfs:comment """This document is published by the Provenance Working Group (http://www.w3.org/2011/prov/wiki/Main_Page). 

If you wish to make comments regarding this document, please send them to public-prov-comments@w3.org (subscribe public-prov-comments-request@w3.org, archives http://lists.w3.org/Archives/Public/public-prov-comments/). All feedback is welcome."""@en ;
  rdfs:label "W3C PROVenance Interchange Ontology (PROV-O)"@en ;
  rdfs:seeAlso <http://www.w3.org/TR/prov-o/> ;
  rdfs:seeAlso <http://www.w3.org/ns/prov> ;
  owl:versionIRI <http://www.w3.org/ns/prov-o-20130430> ;
  owl:versionInfo "Recommendation version 2013-04-30"@en ;
  prov:specializationOf <http://www.w3.org/ns/prov-o> ;
  prov:wasRevisionOf <http://www.w3.org/ns/prov-o-20130312> ;
.
<http://www.w3.org/ns/regorg>
  dcterms:abstract "The Registered Organization Vocabulary is a profile of the Organization Ontology for describing organizations that have gained legal entity status through a formal registration process, typically in a national or regional register." ;
  dcterms:creator [
      schema:affiliation [
          foaf:homepage <http://ies.jrc.ec.europa.eu/DE> ;
          foaf:name "European Commission, Joint Research Centre " ;
        ] ;
      rdfs:seeAlso <http://andrea-perego.name/foaf/#me> ;
      foaf:homepage <http://andrea-perego.name/> ;
      foaf:name "Andrea Perego" ;
    ] ;
  dcterms:creator [
      schema:affiliation [
          foaf:homepage <http://www.w3.org/> ;
          foaf:name "W3C/ERCIM" ;
        ] ;
      rdfs:seeAlso <http://philarcher.org/foaf.rdf#me> ;
      foaf:homepage <http://www.w3.org/People/all#phila> ;
      foaf:name "Phil Archer" ;
    ] ;
  dcterms:creator [
      rdfs:seeAlso <http://makxdekkers.com/makxdekkers.rdf#me> ;
      foaf:homepage <http://makxdekkers.com/> ;
      foaf:name "Makx Dekkers" ;
    ] ;
  dcterms:description "This is the RDF encoding of the Legal Entity vocabulary, originally developed under the European Commission's ISA Programme." ;
  dcterms:modified "2013-05-24"^^xsd:date ;
  vann:preferredNamespacePrefix "rov" ;
  vann:preferredNamespaceUri "http://www.w3.org/ns/regorg#" ;
  voaf:specializes <http://www.w3.org/org> ;
  rdfs:comment "This file specifies the set of RDF classes and properties used in the Registered Organization Vocabulary"@en ;
  rdfs:label "Registered Organization Vocabulary"@en ;
  owl:versionInfo "Second version in w3.org/ns"@en ;
  wdrs:describedby <http://www.w3.org/TR/2013/NOTE-vocab-regorg-20130528/> ;
  foaf:depiction <http://www.w3.org/TR/2013/NOTE-vocab-regorg-20130528/regorg20130508.png> ;
  foaf:maker [
      foaf:name "Government Linked Data WG, based on output from the ADMS Working Group" ;
      foaf:page <http://www.w3.org/2011/gld/> ;
    ] ;
.
rov:RegisteredOrganization
  rdf:type rdfs:Class ;
  rdf:type owl:Class ;
  dcterms:identifier "rov:RegisteredOrganization" ;
  rdfs:comment """<p xmlns=\"http://www.w3.org/ns/regorg#\">rov:RegisteredOrganization is the key class for the Registered Organization vocabulary and represents an organization that is legally registered. In many countries there is a single registry although in others, such as Spain and Germany, multiple registries exist. A Registered Organization is able to trade, is legally liable for its actions, accounts, tax affairs etc. Legal entity status is conferred by the act of registration cf. org:FormalOrganization that applies to any legal entity, including those created by other legal means.</p>
    <p xmlns=\"http://www.w3.org/ns/regorg#\">This makes registered organizations distinct from the broader concept of organizations, groups or, in some jurisdictions, sole traders. Many organizations exist that are not legal entities yet to the outside world they have staff, hierarchies, locations etc. Other organizations exist that are an umbrella for several legal entities (universities are often good examples of this). This vocabulary is concerned solely with registered organizations.</p>
    <p xmlns=\"http://www.w3.org/ns/regorg#\">In RDF, Registered Organization is a sub class of the Organization Ontology's org:FormalOrganization which is itself a sub class of the more general 'Agent' class found in FOAF and Dublin Core that does encompass organizations, natural persons, groups etc. - i.e. an Agent is any entity that is able to carry out actions.</p>"""^^rdf:XMLLiteral ;
  rdfs:isDefinedBy <http://www.w3.org/TR/vocab-regorg/> ;
  rdfs:label "Registered Organization"@en ;
  rdfs:subClassOf org:FormalOrganization ;
.
rov:hasRegisteredOrganization
  rdf:type rdf:Property ;
  rdf:type owl:ObjectProperty ;
  dcterms:identifier "rov:hasRegisteredOrganization" ;
  rdfs:comment """The has registered organization relationship can be used to link any dcterms:Agent (equivalent class foaf:Agent)
    to a Registered Organization that in some way acts as a registered legal entity for it. This is useful, for example, 
    where an organization includes one or more legal entities, or where a natural person is also registered as a legal entity.
    rov:hasRegisteredOrganization has a range of rov:RegisteredOrganization."""@en ;
  rdfs:domain dcterms:Agent ;
  rdfs:isDefinedBy <http://www.w3.org/TR/vocab-regorg/> ;
  rdfs:label "registered organization"@en ;
  rdfs:range rov:RegisteredOrganization ;
.
rov:legalName
  rdf:type rdf:Property ;
  rdf:type owl:DatatypeProperty ;
  dcterms:identifier "rov:legalName" ;
  rdfs:comment """The legal name of the business. A business might have more than one 
    legal name, particularly in countries with more than one official language. In such cases the 
    language of the string should be identified."""@en ;
  rdfs:domain org:FormalOrganization ;
  rdfs:isDefinedBy <http://www.w3.org/TR/vocab-regorg/> ;
  rdfs:label "legal name"@en ;
  rdfs:range rdfs:Literal ;
.
rov:orgActivity
  rdf:type rdf:Property ;
  rdf:type owl:ObjectProperty ;
  dcterms:identifier "rov:orgActivity" ;
  rdfs:comment """The activity of a company should be 
    recorded using a controlled vocabulary expressed as a SKOS concept scheme. Several such 
    vocabularies exist, many of which map to the UN's ISIC codes. Where a particular controlled vocabulary is in use 
    within a given context, such as SIC codes in the UK, it is acceptable to use these, however, the preferred 
    choice for European interoperability is NACE. rov:orgActivity is a sub class of org:classification which has a range of skos:Concept."""@en ;
  rdfs:isDefinedBy <http://www.w3.org/TR/vocab-regorg/> ;
  rdfs:label "company activity"@en ;
  rdfs:subPropertyOf org:classification ;
.
rov:orgStatus
  rdf:type rdf:Property ;
  rdf:type owl:ObjectProperty ;
  dcterms:identifier "rov:orgStatus" ;
  rdfs:comment """Terms like insolvent, bankrupt and in receivership are likely to have 
    different legal implications in different jurisdictions. Best Practice for recording various 
    other status levels is to use the relevant jurisdiction's terms and to do so in a 
    consistent manner using a SKOS Concept Scheme. rov:orgStatus is a sub class of org:classification
    which has a range of skos:Concept."""@en ;
  rdfs:isDefinedBy <http://www.w3.org/TR/vocab-regorg/> ;
  rdfs:label "company status"@en ;
  rdfs:subPropertyOf org:classification ;
.
rov:orgType
  rdf:type rdf:Property ;
  rdf:type owl:ObjectProperty ;
  dcterms:identifier "rov:orgType" ;
  rdfs:comment """This property records the type of organization. Familiar types are SA, PLC, LLC, GmbH etc. Each 
    jurisdiction will have a limited set of recognized company types and these should be used in a consistent manner
    using a SKOS Concept Scheme. rov:orgType is a sub class of org:classification which has a range of skos:Concept."""@en ;
  rdfs:isDefinedBy <http://www.w3.org/TR/vocab-regorg/> ;
  rdfs:label "company type"@en ;
  rdfs:subPropertyOf org:classification ;
.
rov:registration
  rdf:type rdf:Property ;
  rdf:type owl:ObjectProperty ;
  dcterms:identifier "rov:registration" ;
  rdfs:comment """The registration is a fundamental relationship between a legal entity and the 
    authority with which it is registered and that confers legal status upon it. rov:registration is 
    a sub property of adms:identifier which has a range of adms:Identifier. rov:registration has a domain of rov:RegisteredOrganization."""@en ;
  rdfs:domain rov:RegisteredOrganization ;
  rdfs:isDefinedBy <http://www.w3.org/TR/vocab-regorg/> ;
  rdfs:label "registration"@en ;
  rdfs:subPropertyOf adms:identifier ;
.
[
  rdf:type owl:Axiom ;
  rdfs:comment "A collection is an entity that provides a structure to some constituents, which are themselves entities. These constituents are said to be member of the collections."@en ;
  owl:annotatedProperty rdfs:range ;
  owl:annotatedSource prov:hadMember ;
  owl:annotatedTarget prov:Entity ;
  prov:dm "http://www.w3.org/TR/2013/REC-prov-dm-20130430/#term-collection" ;
].
[
  rdf:type owl:Axiom ;
  rdfs:comment "Attribution is a particular case of trace (see http://www.w3.org/TR/prov-dm/#concept-trace), in the sense that it links an entity to the agent that ascribed it." ;
  owl:annotatedProperty rdfs:subPropertyOf ;
  owl:annotatedSource prov:wasAttributedTo ;
  owl:annotatedTarget prov:wasInfluencedBy ;
  prov:definition "IF wasAttributedTo(e2,ag1,aAttr) holds, THEN wasInfluencedBy(e2,ag1) also holds. " ;
].
[
  rdf:type owl:Axiom ;
  rdfs:comment "Derivation is a particular case of trace (see http://www.w3.org/TR/prov-dm/#term-trace), since it links an entity to another entity that contributed to its existence." ;
  owl:annotatedProperty rdfs:subPropertyOf ;
  owl:annotatedSource prov:wasDerivedFrom ;
  owl:annotatedTarget prov:wasInfluencedBy ;
].
[
  rdf:type owl:Axiom ;
  rdfs:comment "Quotation is a particular case of derivation (see http://www.w3.org/TR/prov-dm/#term-quotation) in which an entity is derived from an original entity by copying, or \"quoting\", some or all of it. " ;
  owl:annotatedProperty rdfs:subPropertyOf ;
  owl:annotatedSource prov:wasQuotedFrom ;
  owl:annotatedTarget prov:wasDerivedFrom ;
].
[
  rdf:type owl:Axiom ;
  rdfs:comment """Revision is a derivation (see http://www.w3.org/TR/prov-dm/#term-Revision). Moreover, according to 
http://www.w3.org/TR/2013/REC-prov-constraints-20130430/#term-Revision 23 April 2012 'wasRevisionOf is a strict sub-relation of wasDerivedFrom since two entities e2 and e1 may satisfy wasDerivedFrom(e2,e1) without being a variant of each other.'""" ;
  owl:annotatedProperty rdfs:subPropertyOf ;
  owl:annotatedSource prov:wasRevisionOf ;
  owl:annotatedTarget prov:wasDerivedFrom ;
].
[
  rdf:type owl:Axiom ;
  rdfs:comment "hadPrimarySource property is a particular case of wasDerivedFrom (see http://www.w3.org/TR/prov-dm/#term-original-source) that aims to give credit to the source that originated some information." ;
  owl:annotatedProperty rdfs:subPropertyOf ;
  owl:annotatedSource prov:hadPrimarySource ;
  owl:annotatedTarget prov:wasDerivedFrom ;
].
[
  rdf:type owl:Axiom ;
  owl:annotatedProperty rdfs:domain ;
  owl:annotatedSource prov:wasInfluencedBy ;
  owl:annotatedTarget [
      rdf:type owl:Class ;
      owl:unionOf (
          prov:Activity
          prov:Agent
          prov:Entity
        ) ;
    ] ;
  prov:definition "influencee: an identifier (o2) for an entity, activity, or agent; " ;
  prov:dm "http://www.w3.org/TR/2013/REC-prov-dm-20130430/#term-influence" ;
].
[
  rdf:type owl:Axiom ;
  owl:annotatedProperty rdfs:range ;
  owl:annotatedSource prov:wasInfluencedBy ;
  owl:annotatedTarget [
      rdf:type owl:Class ;
      owl:unionOf (
          prov:Activity
          prov:Agent
          prov:Entity
        ) ;
    ] ;
  prov:definition "influencer: an identifier (o1) for an ancestor entity, activity, or agent that the former depends on;" ;
  prov:dm "http://www.w3.org/TR/2013/REC-prov-dm-20130430/#term-influence" ;
].
