# baseURI: http://toop.elo/elonia-business-register
# imports: http://www.w3.org/ns/adms.rdf
# imports: https://www.w3.org/2009/08/skos-reference/skos.rdf
# prefix: elobr

@prefix adms: <http://www.w3.org/ns/adms#> .
@prefix elobr: <http://toop.elo/elonia-business-register#> .
@prefix dcterms: <http://purl.org/dc/terms/> .
@prefix foaf: <http://xmlns.com/foaf/0.1/> .
@prefix owl: <http://www.w3.org/2002/07/owl#> .
@prefix rdf: <http://www.w3.org/1999/02/22-rdf-syntax-ns#> .
@prefix rdfs: <http://www.w3.org/2000/01/rdf-schema#> .
@prefix skos: <http://www.w3.org/2004/02/skos/core#> .
@prefix xsd: <http://www.w3.org/2001/XMLSchema#> .

<http://toop.elo/elonia-business-register>
  rdf:type owl:Ontology ;
  owl:imports <http://www.w3.org/ns/adms.rdf> ;
  owl:imports <https://www.w3.org/2009/08/skos-reference/skos.rdf> ;
  owl:versionInfo "Created with TopBraid Composer" ;
.
elobr:Repository
  rdf:type adms:AssetRepository ;
  dcterms:created "2018-04-05"^^xsd:date ;
  dcterms:description "This repository describes Elonia's business register in accordance to the defined ontological concepts"@en ;
  dcterms:publisher <http://toop.elo/ebr> ;
  dcterms:title "Elonia's Business Register"@en ;
.
elobr:Citizen
  rdf:type rdfs:Class ;
  rdf:type owl:Class ;
  rdfs:comment "A human person that can have a role in the context of a company."@en ;
  rdfs:subClassOf foaf:Person ;
  rdfs:subClassOf [
      rdf:type owl:Restriction ;
      owl:onDataRange xsd:date ;
      owl:onProperty elobr:birthday ;
      owl:qualifiedCardinality "1"^^xsd:nonNegativeInteger ;
    ] ;
  rdfs:subClassOf [
      rdf:type owl:Restriction ;
      owl:onDataRange xsd:string ;
      owl:onProperty elobr:givenName ;
      owl:qualifiedCardinality "1"^^xsd:nonNegativeInteger ;
    ] ;
  rdfs:subClassOf [
      rdf:type owl:Restriction ;
      owl:onDataRange xsd:string ;
      owl:onProperty elobr:surName ;
      owl:qualifiedCardinality "1"^^xsd:nonNegativeInteger ;
    ] ;
.
elobr:Company
  rdf:type owl:Class ;
  rdfs:comment "A company is an organisation with a business character with a goal to make profit by producing products or providing services."@en ;
  rdfs:label "Company"@en ;
  rdfs:subClassOf skos:Concept ;
  rdfs:subClassOf [
      rdf:type owl:Restriction ;
      owl:cardinality "1"^^xsd:nonNegativeInteger ;
      owl:onProperty elobr:EloniaCompanyName ;
    ] ;
  rdfs:subClassOf [
      rdf:type owl:Restriction ;
      owl:onDataRange elobr:EloniaBusinessCode ;
      owl:onProperty elobr:hasBusinessCode ;
      owl:qualifiedCardinality "1"^^xsd:nonNegativeInteger ;
    ] ;
  rdfs:subClassOf [
      rdf:type owl:Restriction ;
      owl:minQualifiedCardinality "1"^^xsd:nonNegativeInteger ;
      owl:onClass elobr:Citizen ;
      owl:onProperty elobr:hasLegalRepresentationBy ;
    ] ;
.
elobr:EloniaActivityDeclaration
  rdf:type owl:ObjectProperty ;
  rdfs:comment "The description of the main activity of the company as free text description recorded on the registry. This tag should be used to give a description of the company activity in the local language. This should be used in conjunction with the CompanyNaceCode."@en ;
  rdfs:label "Elonia activity declaration"@en ;
.
elobr:EloniaAddress
  rdf:type owl:Class ;
  rdfs:comment "The postal address and/or the visiting address of a physical site of the company, or, an virtual address, i.e., an URL."@en ;
  rdfs:label "Company address"@en ;
.
elobr:EloniaBusinessCode
  rdf:type rdfs:Class ;
  rdfs:comment "The unique official company identifier_"@en ;
  rdfs:label "Elonia business code"@en ;
  skos:prefLabel "Elonia business code" ;
.
elobr:EloniaCompanyNaceCode
  rdf:type owl:DatatypeProperty ;
  rdfs:comment "All companies have to provide an Elonia company NACE code upon registration at the Elonia business register." ;
  rdfs:domain elobr:Company ;
  rdfs:label "company nace code"@en ;
  rdfs:range xsd:string ;
  skos:prefLabel "company nace code"@en ;
.
elobr:EloniaCompanyName
  rdf:type owl:DatatypeProperty ;
  rdfs:comment "All companies have to provide an Elonia company name upon registration at the Elonia business register." ;
  rdfs:domain elobr:Company ;
  rdfs:label "company name"@en ;
  rdfs:range xsd:string ;
  skos:prefLabel "company name"@en ;
.
elobr:EloniaCompanyType
  rdf:type owl:ObjectProperty ;
  rdfs:comment "The legal type of the company_"@en ;
  rdfs:domain elobr:Company ;
  rdfs:label "company type"@en ;
.
elobr:EloniaLegalStatus
  rdf:type owl:ObjectProperty ;
  rdfs:comment "The legal status of the company"@en ;
  rdfs:domain elobr:Company ;
  rdfs:label "company legal status"@en ;
.
elobr:EloniaLegalStatusEffectiveDate
  rdf:type owl:ObjectProperty ;
  rdfs:comment "The date at which the current legal status became effective_"@en ;
  rdfs:domain elobr:Company ;
  rdfs:label "Elonia legal status effective date"@en ;
.
elobr:EloniaHasRegistrationAuthority
  rdf:type owl:ObjectProperty ;
  rdfs:comment "The reference to the official register that has registered the company"@en ;
  rdfs:domain elobr:EloniaBusinessCode ;
  rdfs:label "registration authority"@en ;
.
elobr:EloniaRegistrationDate
  rdf:type owl:DatatypeProperty ;
  rdfs:comment "Represents the date at which the company started."@en ;
  rdfs:label "Elonia registration date"@en ;
  rdfs:range xsd:date ;
.
elobr:EloniaRegistrationNumber
  rdf:type rdfs:Class ;
  rdfs:comment "The registration number of the company_"@en ;
  rdfs:label "Registration number"@en ;
.
elobr:EloniaSSNumber
  rdf:type rdfs:Class ;
  rdfs:comment "The social security number of the company_"@en ;
  rdfs:label "Social security number"@en ;
.
elobr:EloniaVATNumber
  rdf:type rdfs:Class ;
  rdfs:comment "The value added tax number of the company"@en ;
  rdfs:label "VAT number"@en ;
.
elobr:hasBusinessCode
  rdf:type owl:ObjectProperty ;
  rdfs:comment "All companies get an Elonia Business Code uponregistration at the Elonia business register." ;
  rdfs:domain elobr:Company ;
  rdfs:label "has business code"@en ;
  rdfs:range elobr:EloniaBusinessCode ;
  skos:prefLabel "has business code"@en ;
.
elobr:hasLegalRepresentationBy
  rdf:type owl:ObjectProperty ;
  rdfs:comment "The pointer to the person acting as legal representative of the company."@en ;
  rdfs:domain elobr:Company ;
  rdfs:label "has legal representative"@en ;
  rdfs:range elobr:Citizen ;
.
elobr:birthday
  rdf:type owl:DatatypeProperty ;
  rdfs:comment "The day of birth of a person"@en ;
  rdfs:domain elobr:Citizen ;
  rdfs:label "birthday"@en ;
  rdfs:range xsd:date ;
  rdfs:subPropertyOf foaf:birthday ;
.
elobr:givenName
  rdf:type owl:DatatypeProperty ;
  rdfs:comment "The given name of a person"@en ;
  rdfs:domain elobr:Citizen ;
  rdfs:label "given name"@en ;
  rdfs:range xsd:string ;
  rdfs:subPropertyOf foaf:givenName ;
.
elobr:surName
  rdf:type owl:DatatypeProperty ;
  rdfs:comment "The family name of a person"@en ;
  rdfs:domain elobr:Citizen ;
  rdfs:label "family name"@en ;
  rdfs:range xsd:string ;
  rdfs:subPropertyOf foaf:familyName ;
.
elobr:Company_1
  rdf:type elobr:Company ;
  elobr:EloniaCompanyName "A of Elonia" ;
  elobr:hasLegalRepresentationBy elobr:Citizen_1 ;
  rdfs:comment "The A-company, pride of Elonia"@en ;
  rdfs:label "Company 1_"@en ;
  skos:prefLabel "Company 1" ;
.
elobr:Citizen_1
  rdf:type elobr:Citizen ;
  elobr:birthday "1994-03-24"^^xsd:date ;
  elobr:givenName "Czitekiniosis Jehoin" ;
  elobr:surName "din Aldest" ;
  rdfs:comment "A brave citizen of Elonia"@en ;
  rdfs:label "Citizen 1_"@en ;
  skos:prefLabel "Czitek din Aldest" ;
.
